Cleanup.

theories/persistent/pstore_1.v
@@ -2,23 +2,36 @@
    https://gitlab.com/basile.clement/store/-/blob/main/src/store.ml?ref_type=heads
 *)
 
-From iris.base_logic Require Import
-  lib.ghost_map.
+From iris.algebra Require Import
+  gmap.
 
 From zebre Require Import
   prelude.
+From zebre.iris.base_logic Require Import
+  lib.mono_map.
 From zebre.language Require Import
   notations
   diaframe.
+From zebre.std Require Import
+  assert
+  lst.
 From zebre.persistent Require Export
   base.
 From zebre Require Import
   options.
 
-Implicit Types l r root : loc.
-Implicit Types v t : val.
+Implicit Types l : loc.
+Implicit Types v t s : val.
 Implicit Types σ : gmap loc val.
-Implicit Types map : gmap loc (gmap loc val).
+
+#[local] Notation "'snap_store'" := (
+  in_type "snap" 0
+)(in custom zebre_proj
+).
+#[local] Notation "'snap_root'" := (
+  in_type "snap" 1
+)(in custom zebre_proj
+).
 
 #[local] Notation "'Root'" := (
   in_type "descr" 0
@@ -29,45 +42,611 @@ Implicit Types map : gmap loc (gmap loc val).
 )(in custom zebre_tag
 ).
 
+(* ------------------------------------------------------------------------ *)
+(* Code. *)
+
 Definition pstore_create : val :=
   λ: <>,
-    ref §Root.
+    ref (ref §Root).
 
 Definition pstore_ref : val :=
   λ: "v",
     ref "v".
 
-#[local] Definition pstore_reroot : val :=
-  rec: "pstore_reroot" "t" :=
-    match: !"t" with
-    | Root =>
-        ()
-    | Diff "r" "v" "t'" =>
-        "pstore_reroot" "t'" ;;
-        "t'" <- ‘Diff{ "r", !"r", "t" } ;;
-        "r" <- "v" ;;
-        "t" <- §Root
-    end.
-
 Definition pstore_get : val :=
   λ: "t" "r",
-    pstore_reroot "t" ;;
     !"r".
 
 Definition pstore_set : val :=
   λ: "t" "r" "v",
-    pstore_reroot "t" ;;
-    let: "t'" := ref §Root in
-    "t" <- ‘Diff{ "r", !"r", "t'" } ;;
+    let: "root" := ref §Root in
+    !"t" <- ‘Diff{ "r", !"r", "root" } ;;
     "r" <- "v" ;;
-    "t'".
+    "t" <- "root".
+
+Definition pstore_capture : val :=
+  λ: "t",
+    ("t", !"t").
+
+Definition pstore_collect : val :=
+  rec: "pstore_collect" "node" "acc" :=
+    match: !"node" with
+    | Root =>
+        ("node", "acc")
+    | Diff <> <> "node'" =>
+        "pstore_collect" "node'" ‘Cons{ "node", "acc" }
+    end.
+Definition pstore_revert : val :=
+  rec: "pstore_revert" "node" "seg" :=
+    match: "seg" with
+    | Nil =>
+        "node" <- §Root
+    | Cons "node'" "seg" =>
+        match: !"node'" with
+        | Root =>
+            Fail
+        | Diff "r" "v" "node_" =>
+            assert ("node_" = "node") ;;
+            "node" <- ‘Diff{ "r", !"r", "node'" } ;;
+            "r" <- "v" ;;
+            "pstore_revert" "node'" "seg"
+        end
+    end.
+Definition pstore_reroot : val :=
+  λ: "node",
+    let: "root", "nodes" := pstore_collect "node" §Nil in
+    pstore_revert "root" "nodes".
+
+Definition pstore_restore : val :=
+  λ: "t" "s",
+    if: "t" ≠ "s".<snap_store> then (
+      Fail
+    ) else (
+      let: "root" := "s".<snap_root> in
+      match: !"root" with
+      | Root =>
+          ()
+      | Diff <> <> <> =>
+          pstore_reroot "root" ;;
+          "t" <- "root"
+      end
+    ).
+
+(* ------------------------------------------------------------------------ *)
+(* Lemmas on maps and lists. *)
+
+Section map.
+  Context `{Countable K}.
+  Context {V : Type}.
+
+  Lemma gmap_included_insert (σ1 σ2:gmap K V) (l:K) (v:V) :
+    σ1 ⊆ σ2 ->
+    <[l:=v]>σ1 ⊆ <[l:=v]>σ2.
+  Proof.
+    intros ? l'. destruct_decide (decide (l=l')).
+    { subst. rewrite !lookup_insert //. }
+    { rewrite !lookup_insert_ne //. }
+  Qed.
+
+  Lemma gmap_included_insert_notin (σ1 σ2:gmap K V) (l:K) (v:V) :
+    l ∉ dom σ1 ->
+    σ1 ⊆ σ2 ->
+    σ1 ⊆ <[l:=v]>σ2.
+  Proof.
+    intros ?? l'. destruct_decide (decide (l=l')).
+    { subst. rewrite lookup_insert // not_elem_of_dom_1 //. }
+    { rewrite !lookup_insert_ne //. }
+  Qed.
+
+  Lemma incl_dom_incl (σ1 σ2:gmap K V)  :
+    σ1 ⊆ σ2 ->
+    dom σ1 ⊆ dom σ2.
+  Proof.
+    intros X1.
+    intros l Hl. apply elem_of_dom in Hl. destruct Hl as (?&Hl).
+    eapply map_subseteq_spec in X1; last done. by eapply elem_of_dom.
+  Qed.
+End map.
+
+Section list.
+  Context {A : Type}.
+
+  Lemma list_case_r (l:list A) :
+    l = nil \/ exists (l':list A) x, l = l' ++ [x].
+  Proof.
+    induction l using rev_ind.
+    naive_solver. right.
+    destruct IHl as [-> | (?&?&->)]; eauto.
+  Qed.
+
+  Lemma elem_of_middle (x:A) (xs:list A) :
+    x ∈ xs ->
+    exists (l1 l2:list A), xs = l1 ++ x::l2.
+  Proof.
+    intros Hx. apply elem_of_list_lookup_1 in Hx.
+    destruct Hx as (?&?).
+    eexists _,_. symmetry. eapply take_drop_middle. done.
+  Qed.
+End list.
+
+(* ------------------------------------------------------------------------ *)
+(* Define a labeled graph as a set of edges. *)
+
+Section graph.
+  Definition graph (A B : Type) `{Countable A} `{Countable B} :=
+    gset (A * B * A).
+
+  Context `{Countable A} `{Countable B}.
+  Definition vertices (g:graph A B) : gset A :=
+    set_fold (fun '(x,_,y) acc => {[x;y]} ∪ acc) ∅ g.
+
+  Lemma vertices_empty :
+    vertices ∅ = ∅.
+  Proof.
+    compute_done.
+  Qed.
+
+  Definition proj1 {A B C:Type} (x:(A*B*C)) : A :=
+    match x with (x,_,_) => x end.
+  Definition proj2 {A B C:Type} (x:(A*B*C)) : B :=
+    match x with (_,x,_) => x end.
+  Definition proj3 {A B C:Type} (x:(A*B*C)) : C :=
+    match x with (_,_,x) => x end.
+
+  Lemma elem_of_vertices x (g:graph A B) :
+    x ∈ vertices g <-> exists b y, ((x,b,y) ∈ g \/ (y,b,x) ∈ g).
+  Proof.
+    apply set_fold_ind_L with (P := fun f g => x ∈ f  <-> exists b y, ((x,b,y) ∈ g \/ (y,b,x) ∈ g)).
+    set_solver.
+    intros ((?,?),?). set_solver.
+  Qed.
+
+  Lemma vertices_singleton (x:(A*B*A)) :
+    vertices {[x]} = {[proj1 x; proj3 x]}.
+  Proof.
+    rewrite /vertices set_fold_singleton. destruct x as ((?&?)&?); set_solver.
+  Qed.
+
+  Lemma vertices_union (g1 g2:graph A B) :
+    vertices (g1 ∪ g2) = vertices g1 ∪ vertices g2.
+  Proof.
+    revert g2. induction g1 using set_ind_L; intros g2.
+    { rewrite /vertices set_fold_empty !left_id_L //. }
+    replace ({[x]} ∪ X ∪ g2) with (X ∪ ({[x]} ∪ g2)) by set_solver.
+    rewrite (union_comm_L _  X).
+    rewrite !IHg1. rewrite -union_assoc_L. f_equal.
+    destruct_decide (decide (x ∈ g2)).
+    { replace ({[x]} ∪ g2) with g2 by set_solver.
+      rewrite vertices_singleton.
+      assert ({[proj1 x; proj3 x]} ⊆ vertices g2); last by set_solver.
+      intros l Hl. apply elem_of_vertices.
+      rewrite elem_of_union !elem_of_singleton in Hl. destruct x as ((?,?),?). set_solver. }
+    rewrite {1}/vertices /set_fold. simpl.
+    rewrite (foldr_permutation _ _ _ _ (x::elements g2)).
+    { intros. destruct a1 as ((?,?),?),a2 as ((?,?),?); set_solver. }
+    { by apply elements_union_singleton. }
+    { simpl. rewrite vertices_singleton. destruct x as ((?,?),?). set_solver. }
+  Qed.
+
+  Definition edge (g:graph A B) x c y :=
+    (x,c,y) ∈ g.
+
+  Inductive path (g:graph A B) : A -> list (A*B*A) -> A -> Prop :=
+  | path_nil : forall a, path g a [] a
+  | path_cons : forall a1 b a2 bs a3,
+      (a1,b,a2) ∈ g ->
+      path g a2 bs a3 ->
+      path g a1 ((a1,b,a2)::bs) a3.
+
+  Lemma path_app_inv g a1 a2 xs ys :
+    path g a1 (xs ++ ys) a2 ->
+    exists a, path g a1 xs a /\ path g a ys a2.
+  Proof.
+    revert a1 ys a2. induction xs as [| ((?,?),?)].
+    { eauto using path_nil. }
+    { intros. rewrite -app_comm_cons in H1. inversion H1. subst.
+      apply IHxs in H9. destruct H9 as (?&?&?).
+      eauto using path_cons. }
+  Qed.
+
+  Lemma path_snoc_inv g a1 a2 a3 a4 b xs :
+    path g a1 (xs ++ [(a2,b,a3)]) a4 ->
+    path g a1 xs a2 /\ a3 = a4 /\ (a2,b,a3) ∈ g.
+  Proof.
+    intros Hpath. apply path_app_inv in Hpath. destruct Hpath as (?&?&Hpath).
+    inversion Hpath. subst. inversion H9. naive_solver.
+  Qed.
+
+  Definition acyclic g := forall a xs, path g a xs a -> xs = nil.
+
+  Record rooted_dag g (r:A) :=
+    { ti1 : forall a, a ∈ vertices g -> exists xs, path g a xs r;
+      ti2 : acyclic g
+    }.
+
+  Definition unaliased (g:graph A B) :=
+      forall r x1 r1 x2 r2,
+      (r,x1,r1) ∈ g ->
+      (r,x2,r2) ∈ g ->
+      x1 = x2 /\ r1 = r2.
+
+  Lemma path_app (g:graph A B) x3 x1 xs ys x2 :
+    path g x1 xs x3 ->
+    path g x3 ys x2 ->
+    path g x1 (xs++ys) x2.
+  Proof.
+    intros Hp.
+    revert x2 ys. induction Hp. eauto.
+    intros. rewrite -app_comm_cons. apply path_cons. set_solver.
+    eauto.
+  Qed.
+
+  Definition all_uniq_path g :=
+    forall a1 a2 xs ys, path g a1 xs a2 -> path g a1 ys a2 -> xs = ys.
+
+  Lemma rooted_tree_impl_acyclic_unaliased g r :
+    (forall a, a ∈ vertices g -> exists xs, path g a xs r) -> (* If every vertex can reach the root, *)
+    all_uniq_path g -> (* then the property of uniq path *)
+    acyclic g /\ unaliased g. (* implies acyclicity + unalising *)
+  Proof.
+    intros Hroot  Huniq. split.
+    { intros ?? Hpath.
+      assert (path g a (xs++xs) a) as Hloop.
+      { by eapply path_app. }
+      specialize (Huniq a a xs (xs++xs) Hpath Hloop).
+      apply (@f_equal _ _ length) in Huniq. rewrite app_length in Huniq.
+      assert (length xs = 0) by lia. destruct xs; simpl in *; try done; lia. }
+    { intros ????? X1 X2.
+      destruct (Hroot r1) as (xs1&Hxs1).
+      { eapply elem_of_vertices. eauto. }
+      destruct (Hroot r2) as (xs2&Hxs2).
+      { eapply elem_of_vertices. eauto. }
+      assert (path g r0 ((r0,x1,r1)::xs1) r) as Hp1. by eapply path_cons.
+      assert (path g r0 ((r0,x2,r2)::xs2) r) as Hp2. by eapply path_cons.
+      specialize (Huniq _ _ _ _ Hp1 Hp2). naive_solver. }
+  Qed.
+
+  Lemma acyclic_unaliased_impl_uniq_path g :
+    acyclic g ->
+    unaliased g ->
+    all_uniq_path g.
+  Proof.
+    intros Hacy Hinj. intros ???? Hpath.
+    revert ys. induction Hpath; intros ys.
+    { intros Hpath. apply Hacy in Hpath. done. }
+    { inversion 1; subst.
+      { exfalso.
+        assert (path g a3 ((a3, b, a2)::bs) a3) as Z.
+        { apply path_cons. done. eauto. }
+        apply Hacy in Z. congruence. }
+      destruct (Hinj _ _ _ _ _ H1 H3). subst.
+      f_equal. eapply IHHpath. done. }
+  Qed.
+
+  Lemma rooted_dag_empty (r:A) :
+      rooted_dag (∅ : graph A B) r.
+  Proof.
+    constructor.
+    { intros ?. rewrite vertices_empty. set_solver. }
+    { intros ??. inversion 1; set_solver. }
+  Qed.
+
+  Lemma path_cycle_end_inv_aux g (r r':A) b ds x1 x2 :
+    r ≠ r' ->
+    x2 ≠ r' ->
+    r' ∉ vertices g ->
+    path ({[(r, b, r')]} ∪ g) x1 ds x2 ->
+    path g x1 ds x2.
+  Proof.
+    induction 4.
+    { apply path_nil. }
+    { eapply path_cons.
+      { rewrite /edge elem_of_union elem_of_singleton in H4.
+        destruct H4 as [|]; last done.
+        inversion H4. subst. inversion H5. congruence. subst.
+        exfalso. apply H3. apply elem_of_vertices. set_solver. }
+      by eapply IHpath. }
+  Qed.
+
+  Lemma path_cycle_end_inv g (r r':A) b ds x :
+    r ≠ r' ->
+    r' ∉ vertices g ->
+    path ({[(r, b, r')]} ∪ g) x ds x ->
+    path g x ds x.
+  Proof.
+    intros.
+    destruct_decide (decide (x=r')).
+    { subst. inversion H3. apply path_nil. subst. exfalso. apply H2. apply elem_of_vertices. set_solver. }
+    eapply path_cycle_end_inv_aux; last done. all:done.
+  Qed.
+
+  Lemma path_snoc g a1 b a2 bs a3 :
+    path g a1 bs a2 ->
+    (a2,b,a3) ∈ g ->
+    path g a1 (bs++[(a2,b,a3)]) a3.
+  Proof.
+    induction 1.
+    { intros. apply path_cons. done. apply path_nil. }
+    { intros. rewrite -app_comm_cons. eauto using path_cons. }
+  Qed.
+
+  Lemma path_weak g1 g2 x bs y :
+    path g1 x bs y ->
+    g1 ⊆ g2 ->
+    path g2 x bs y.
+  Proof.
+    induction 1; intros Hi. apply path_nil. eapply path_cons.
+    by apply Hi. by apply IHpath.
+  Qed.
+
+  Lemma rooted_dag_add (r r':A) g x:
+    r ≠ r' ->
+    r' ∉ vertices g ->
+    rooted_dag g r ->
+    rooted_dag ({[(r, x, r')]} ∪ g) r'.
+  Proof.
+    intros Hne Hg Hroot. inversion Hroot as [X1 X2].
+    constructor.
+    { rewrite vertices_union vertices_singleton. intros a.
+      rewrite !elem_of_union !elem_of_singleton.
+      intros [[-> | ->] | Hx].
+      { exists [(r, x, r')]. simpl. eapply path_cons. set_solver. apply path_nil. }
+      { exists nil. apply path_nil. }
+      { apply X1 in Hx. destruct Hx as (ds,Hx). exists (ds++[(r, x, r')]).
+        eapply path_snoc.
+        { eapply path_weak; eauto. set_solver. }
+        { set_solver. } } }
+    { intros ?? Hpath. apply  path_cycle_end_inv in Hpath; eauto. }
+  Qed.
+
+  Lemma acyclic_weak (g1 g2:graph A B) :
+    acyclic g1 ->
+    g2 ⊆ g1 ->
+    acyclic g2.
+  Proof.
+    intros Hacy ? ???. eapply Hacy. by eapply path_weak.
+  Qed.
+
+  Lemma path_all_in (g:graph A B) a1 xs a2 :
+    path g a1 xs a2 ->
+    list_to_set xs ⊆ g.
+  Proof.
+    induction 1; simpl; set_solver.
+  Qed.
+
+  Lemma path_restrict (g:graph A B) r xs r' :
+    path g r xs r' ->
+    path (list_to_set xs) r xs r'.
+  Proof.
+    induction 1; eauto using path_nil.
+    apply path_cons. set_solver.
+    eapply path_weak. done. set_solver.
+  Qed.
+
+  Lemma path_inv_r (g:graph A B) x bs z :
+    path g x bs z ->
+    (x = z /\ bs = nil) ∨ ∃ bs' b y, bs = bs' ++ [(y,b,z)] /\ path g x bs' y ∧ (y,b,z) ∈ g.
+  Proof.
+    induction 1.
+    { naive_solver.  }
+    right. destruct IHpath as [(->&->)|(bs'&b'&y&->&?&?)].
+    { exists nil. eexists _,_. split; first done. split. eauto using path_nil. naive_solver. }
+    { exists ((a1, b, a2) :: bs'). eexists _,_. rewrite app_comm_cons //. split_and !; try done.
+      apply path_cons; eauto. }
+  Qed.
+
+  Lemma path_add_inv_r (r r':A) b x xs g :
+    r ≠ r' ->
+    r' ∉ vertices g ->
+    path ({[(r, b, r')]} ∪ g) x xs r' ->
+    (xs = nil /\ x = r') \/ (exists xs', xs = xs' ++ [(r, b, r')] /\ path g x xs' r).
+  Proof.
+    intros Hrr' Hr' Hreach. apply path_inv_r in Hreach.
+    destruct Hreach as [(->&->)|(bs'&b0&y&->&Hreach&Hedge)].
+    { eauto. }
+    right.
+    assert (b0=b /\ y=r) as (->&->).
+    { rewrite /edge elem_of_union elem_of_singleton in Hedge.
+      destruct Hedge. naive_solver. exfalso. apply Hr', elem_of_vertices. eauto. }
+    eexists. split; first done.
+    eauto using path_cycle_end_inv_aux.
+  Qed.
+
+  (* [mirror xs ys] asserts that, up-to labels, the path xs is the reverse of ys *)
+  Inductive mirror :
+    list (A*B*A) -> list (A*B*A) -> Prop :=
+  | mirror_nil :
+    mirror [] []
+  | mirror_cons :
+    forall r x x' r' xs ys,
+      mirror xs ys  ->
+      mirror (xs++[(r,x,r')]) ((r',x',r)::ys).
+
+  Lemma mirror_snoc ys xs a a' x x' :
+    mirror ys xs ->
+    mirror ((a,x,a') :: ys) (xs ++ [(a',x',a)]).
+  Proof.
+    induction 1.
+    { apply (mirror_cons _ _ _ _ nil nil). apply mirror_nil. }
+    rewrite -!app_comm_cons app_comm_cons. by apply mirror_cons.
+  Qed.
+
+  Lemma mirror_symm xs ys :
+    mirror xs ys -> mirror ys xs.
+  Proof.
+    induction 1. eauto using mirror_nil.
+    apply mirror_snoc; eauto.
+  Qed.
+
+  Lemma use_mirror xs ys (g:graph A B) r y :
+    mirror xs ys ->
+    path g r xs y ->
+    path (list_to_set ys) y ys r.
+  Proof.
+    intros Hu. revert r y. induction Hu; intros r0 y.
+    { inversion 1. subst. apply path_nil. }
+    intros Hp. apply path_snoc_inv in Hp. destruct Hp as (?&?&?). subst.
+    apply path_cons. set_solver. eapply path_weak. apply IHHu; eauto. set_solver.
+  Qed.
+
+  Lemma mirror_vertices (xs ys:list (A*B*A)) :
+    mirror xs ys ->
+    vertices (list_to_set ys) = vertices (list_to_set xs).
+  Proof.
+    revert xs. induction ys; intros xs; inversion 1; subst. done.
+    simpl. rewrite list_to_set_app_L !vertices_union !vertices_singleton. simpl.
+    erewrite IHys; last done. rewrite vertices_empty. set_solver.
+  Qed.
+
+  Lemma mirror_same_length (xs ys:list (A*B*A)):
+    mirror xs ys ->
+    length xs = length ys.
+  Proof. induction 1. done. rewrite app_length. simpl. lia. Qed.
+
+  Lemma mirror_mirrored_edges xs ys r x r' :
+    mirror xs ys ->
+    (r,x,r') ∈ xs -> exists x', (r',x',r) ∈ ys.
+  Proof.
+    induction 1. intros ?. set_solver.
+    rewrite elem_of_app elem_of_list_singleton.
+    intros [X|X].
+    { apply IHmirror in X. set_solver. }
+    { set_solver. }
+  Qed.
+
+  Lemma path_middle (g:graph A B) x xs ys z :
+    path g x (xs ++ ys) z ->
+    exists y, path g x xs y /\ path g y ys z.
+  Proof.
+    revert g x ys z. induction xs; intros g x ys z.
+    { simpl. eauto using path_nil. }
+    inversion 1; simpl in *; subst.
+    apply IHxs in H7. destruct H7 as (y,(?&?)).
+    exists y. split; last done. eauto using path_cons.
+  Qed.
+
+  Lemma use_mirror_subset xs ys xs' g r y :
+    xs' ⊆ xs ->
+    mirror xs ys ->
+    path g r xs' y ->
+    exists zs, path (list_to_set ys) y zs r /\ length xs' = length zs.
+  Proof.
+    intros Hincl Hundo Hpath.
+    induction Hpath.
+    { exists nil. split. apply path_nil. done. }
+    { destruct IHHpath as (zs&Hzs&?).
+      { set_solver. }
+      eapply (mirror_mirrored_edges _ _ a1 b a2) in Hundo. 2:set_solver.
+      destruct Hundo as (b'&?).
+      exists (zs ++ [(a2, b', a1)]). split.
+      { eapply path_app. done.
+        apply path_cons.  set_solver. apply path_nil. }
+      { rewrite app_length. simpl. lia. } }
+  Qed.
+
+  Definition pathlike (ys:list (A*B*A)) r :=
+    forall a b a', (a,b,a') ∈ ys -> a' = r \/ exists b' a'', (a',b',a'') ∈ ys.
+
+  Lemma path_pathlike g r ys y :
+    path g y ys r ->
+    pathlike ys r.
+  Proof.
+    intros Hpath a b a' Hedge.
+    apply elem_of_middle in Hedge. destruct Hedge as (?&?&->).
+    rewrite cons_middle assoc_L in Hpath.
+    apply path_app_inv in Hpath. destruct Hpath as (?&Hpath&Hp').
+    apply path_snoc_inv in Hpath. destruct Hpath as (?&?&?). subst.
+    inversion Hp'; set_solver.
+  Qed.
+
+  Lemma same_path g (xs:list (A*B*A)) a1 a2 a3 a4 :
+    path g a1 xs a2 ->
+    path g a3 xs a4 ->
+    xs ≠ nil ->
+    a1 = a3 /\ a2=a4.
+  Proof.
+    intros Hp1. revert a3 a4. induction Hp1.
+    { intros. congruence. }
+    intros a3' a4'. inversion 1. subst. intros _. destruct bs.
+    { inversion Hp1; inversion H10. subst. done. }
+    apply IHHp1 in H10. 2:done. naive_solver.
+  Qed.
+
+  Lemma path_ends_vertices g x1 xs x2 :
+    path g x1 xs x2 ->
+    (x1 = x2) \/ (x1 ∈ vertices g /\ x2 ∈ vertices g).
+  Proof.
+     inversion 1. eauto. subst. right.
+     split. apply elem_of_vertices. eauto.
+     apply path_inv_r in H3. destruct H3 as [(->&->)|(?&?&?&->&?&?)].
+     all:apply elem_of_vertices; eauto.
+  Qed.
+End graph.
+
+(* ------------------------------------------------------------------------ *)
+(* Define apply_diffl, a function applying a list of diff. *)
+
+Section adiffl.
+  Notation diff := (
+    (* loc and its old value *)
+    loc*val
+  )%type.
+
+  Definition apply_diffl (ds:list diff) (σ:gmap loc val) : gmap loc val :=
+    foldr (fun '(l,v) σ => <[l:=v]> σ) σ ds.
+
+  Lemma dom_apply_diffl ds σ :
+    dom (apply_diffl ds σ) = dom σ ∪ (list_to_set ds.*1).
+  Proof.
+    induction ds as [|(?&?)]; set_solver.
+  Qed.
+
+  Lemma apply_diffl_insert_ne ds l v σ :
+    l ∉ ds.*1 ->
+    apply_diffl ds (<[l:=v]> σ) = <[l:=v]> (apply_diffl ds σ).
+  Proof.
+    induction ds as [|(?&?)].
+    { intros ?. reflexivity. }
+    { intros. simpl. rewrite IHds. set_solver.
+      rewrite insert_commute //. set_solver. }
+  Qed.
+
+  Lemma apply_diffl_app ds ds' σ :
+    apply_diffl (ds++ds') σ = apply_diffl ds (apply_diffl ds' σ).
+  Proof.
+    rewrite /apply_diffl foldr_app //.
+  Qed.
+
+  Lemma apply_diffl_snoc xs l v σ :
+    apply_diffl (xs ++ [(l,v)]) σ = apply_diffl xs (<[l:=v]> σ).
+  Proof.
+    rewrite apply_diffl_app //.
+  Qed.
+
+  Lemma apply_diffl_cons l v xs σ :
+    apply_diffl ((l,v)::xs) σ = <[l:=v]> (apply_diffl xs σ).
+  Proof.
+    done.
+  Qed.
+
+  Lemma apply_diffl_included xs σ1 σ2 :
+    σ1 ⊆ σ2 ->
+    apply_diffl xs σ1 ⊆ apply_diffl xs σ2.
+  Proof.
+    revert σ1 σ2. induction xs as [|(?,?)]; intros;
+      [ done | eauto using gmap_included_insert ].
+  Qed.
+End adiffl.
+
+(* ------------------------------------------------------------------------ *)
+(* Proof. *)
 
 Class PstoreG Σ `{zebre_G : !ZebreG Σ} := {
-  pstore_G_map_G : ghost_mapG Σ loc (gmap loc val) ;
+  #[local] pstore_G_map_G :: MonoMapG Σ nat (loc * gmap loc val)%type ;
 }.
 
 Definition pstore_Σ := #[
-  ghost_mapΣ loc (gmap loc val)
+  mono_map_Σ nat (loc * gmap loc val)%type
 ].
 #[global] Instance subG_pstore_Σ Σ `{zebre_G : !ZebreG Σ} :
   subG pstore_Σ Σ →
@@ -79,105 +658,90 @@ Qed.
 Section pstore_G.
   Context `{pstore_G : PstoreG Σ}.
 
-  Definition pstore_name :=
-    gname.
-  Implicit Types γ : pstore_name.
+  Notation diff := (
+    (* loc and its old value. *)
+    loc*val
+  )%type.
+  Notation graph_store := (
+    graph loc diff
+  ).
+  Notation map_model := (
+    gmap loc (gmap loc val)
+  ).
+
+  Definition correct_path_diff (M:map_model) (g:graph_store) :=
+    forall r1 ds r2 σ1 σ2,
+      path g r1 ds r2 -> M !! r1 = Some σ1 -> M !! r2 = Some σ2 ->
+      σ1 = (apply_diffl (proj2 <$> ds) σ2).
+
+  Record store_inv (M:map_model) (g:graph_store) (r:loc) (σ σ0:gmap loc val) :=
+    { si1 : dom M = vertices g ∪ {[r]};
+      si2 : σ ⊆ σ0;
+      si3 : M !! r = Some σ0 ;
+      si4 : correct_path_diff M g
+    }.
+
+  Definition locs_of_edges_in g (X:gset loc) :=
+    forall (r:loc) l v r', edge g r (l,v) r' -> l ∈ X.
+
+  Record coherent (M:map_model) (σ0:gmap loc val) (g:graph_store) :=
+    { coh1 : forall r σ, M !! r = Some σ -> dom σ = dom σ0;
+      coh2 : locs_of_edges_in g (dom σ0);
+    }.
+
+  Definition snap_inv (M:map_model) (C:gmap nat (loc * gmap loc val)) :=
+    forall n l σ, C !! n = Some (l,σ) -> exists σ', M !! l = Some σ' /\ σ ⊆ σ'.
 
   #[local] Definition pstore_map_auth γ map :=
-    @ghost_map_auth _ _ _ _ _ pstore_G_map_G γ 1 map.
-  #[local] Definition pstore_map_elem γ l σ :=
-    @ghost_map_elem _ _ _ _ _ pstore_G_map_G γ l DfracDiscarded σ.
+    mono_map_auth γ map.
+  #[local] Definition pstore_map_elem γ n l σ :=
+    mono_map_elem γ n (l, σ).
 
-  Definition pstore_store σ0 σ :=
-    union_with (λ _, Some) σ0 σ.
+  Lemma extract_unaliased (g : graph_store) :
+    ([∗ set] '(r, (l, v), r') ∈ g, r ↦ ’Diff{ #(l : loc), v, #(r' : loc) }) -∗
+    ⌜unaliased g⌝.
+  Proof.
+    iIntros "Hg" (???????).
+    destruct_decide (decide (a0 = a2 ∧ a1 = a3)). done.
+    rewrite (big_sepS_delete _ _ (a, a0, a1)). set_solver.
+    rewrite (big_sepS_delete _ _ (a, a2, a3)). set_solver.
+    iDestruct "Hg" as "(?&?&_)". destruct a0,a2.
+    iDestruct (pointsto_ne with "[$][$]") as "%". congruence.
+  Qed.
 
-  #[local] Definition pstore_inv_inner γ σ0 map root : iProp Σ :=
-    ∃ σ_root,
-    ⌜map !! root = Some σ_root⌝ ∗
-    ⌜map_Forall (λ _ σ, dom σ ⊆ dom σ0) map⌝ ∗
-    pstore_map_auth γ map ∗
-    root ↦ §Root ∗
-    ( [∗ map] r ↦ v ∈ pstore_store σ0 σ_root,
-      r ↦ v
-    ) ∗
-    ( [∗ map] l ↦ σ ∈ delete root map,
-      ∃ r v l' σ',
-      ⌜map !! l' = Some σ'⌝ ∗
-      ⌜pstore_store σ0 σ = <[r := v]> (pstore_store σ0 σ')⌝ ∗
-      l ↦ ’Diff{ #r, v, #l' }
-    ).
-  Definition pstore_inv γ σ0 : iProp Σ :=
-    ∃ map root,
-    pstore_inv_inner γ σ0 map root.
+  (* NB our invariant asserts that g is indeed a rooted tree: a rooted DAG
+     with unicity of paths. Indeed, from the set of pointsto we can extract [unaliased],
+     (see [extract_unaliased]), and a DAG with unaliased guarantees unicity of paths
+     (see [acyclic_unaliased_impl_uniq_path] ) *)
 
-  Definition pstore_model t γ σ : iProp Σ :=
-    ∃ l,
-    ⌜t = #l⌝ ∗
-    pstore_map_elem γ l σ.
+  #[local] Definition pstore (γ:gname) (t:val) (σ:gmap loc val) : iProp Σ :=
+    ∃ (t0 r:loc)
+      (σ0:gmap loc val) (* the global map, with all the points-to ever allocated *)
+      (g:graph_store) (* the global graph *)
+      (M:map_model) (* the map model, associating to each node its model *)
+      (C:gmap nat (loc * gmap loc val)), (* the model of snapshots *)
+    ⌜t=#t0 /\ store_inv M g r σ σ0 /\ coherent M σ0 g /\ rooted_dag g r /\ snap_inv M C⌝ ∗
+    t0 ↦ #r ∗
+    r ↦ §Root ∗
+    pstore_map_auth γ C ∗
+    ([∗ map] l ↦ v ∈ σ0, l ↦ v) ∗
+    ([∗ set] x ∈ g, let '(r,(l,v),r') := x in r ↦ ’Diff{ #(l : loc), v, #(r' : loc) }) .
 
-  #[local] Instance pstore_inv_inner_timeless γ σ0 map root :
-    Timeless (pstore_inv_inner γ σ0 map root).
+  Definition open_inv : string :=
+    "[%t0 [%r [%σ0 [%g [%M [%C ((->&%Hinv&%Hcoh&%Hgraph&%Hsnap)&Ht0&Hr&HC&Hσ0&Hg)]]]]]]".
+
+  Definition pstore_snapshot γ t s σ : iProp Σ :=
+    ∃ l n, ⌜s=ValTuple [t;#l]⌝ ∗ pstore_map_elem γ n l σ.
+
+  #[global] Instance pstore_snapshot_timeless γ t s σ :
+    Timeless (pstore_snapshot γ t s σ).
   Proof.
     apply _.
   Qed.
-  #[global] Instance pstore_inv_timeless γ σ0 :
-    Timeless (pstore_inv γ σ0).
+  #[global] Instance pstore_snapshot_persistent γ t s σ :
+    Persistent (pstore_snapshot γ t s σ).
   Proof.
     apply _.
-  Qed.
-  #[global] Instance pstore_model_persistent t γ σ :
-    Persistent (pstore_model t γ σ).
-  Proof.
-    apply _.
-  Qed.
-
-  #[local] Lemma pstore_map_alloc root :
-    ⊢ |==>
-      ∃ γ,
-      pstore_map_auth γ {[root := ∅]} ∗
-      pstore_map_elem γ root ∅.
-  Proof.
-    iMod (@ghost_map_alloc _ _ _ _ _ pstore_G_map_G {[root := ∅]}) as "(%γ_map & Hmap_auth & Hmap_elem)".
-    setoid_rewrite big_sepM_singleton.
-    iMod (ghost_map_elem_persist with "Hmap_elem") as "Hmap_elem".
-    iSteps.
-  Qed.
-  #[local] Lemma pstore_map_lookup γ map l σ :
-    pstore_map_auth γ map -∗
-    pstore_map_elem γ l σ -∗
-    ⌜map !! l = Some σ⌝.
-  Proof.
-    apply ghost_map_lookup.
-  Qed.
-  #[local] Lemma pstore_map_insert {γ map} l σ :
-    map !! l = None →
-    pstore_map_auth γ map ⊢ |==>
-      pstore_map_auth γ (<[l := σ]> map) ∗
-      pstore_map_elem γ l σ.
-  Proof.
-    iIntros "%Hlookup Hmap_auth".
-    iMod (ghost_map_insert with "Hmap_auth") as "(Hmap_auth & Hmap_elem)"; first done.
-    iMod (ghost_map_elem_persist with "Hmap_elem") as "Hmap_elem".
-    iSteps.
-  Qed.
-
-  #[local] Lemma pstore_store_dom σ0 σ :
-    dom σ ⊆ dom σ0 →
-    dom (pstore_store σ0 σ) ≡ dom σ0.
-  Proof.
-    rewrite set_equiv => Hσ_dom r. rewrite !elem_of_dom lookup_union_with.
-    destruct (σ0 !! r) eqn:Hσ0_lookup, (σ !! r) eqn:Hσ_lookup; try done.
-    apply not_elem_of_dom_2 in Hσ0_lookup. apply elem_of_dom_2 in Hσ_lookup. set_solver.
-  Qed.
-  #[local] Lemma pstore_store_insert r v σ0 σ :
-    dom σ ⊆ dom σ0 →
-    σ0 !! r = None →
-    pstore_store (<[r := v]> σ0) σ = <[r := v]> (pstore_store σ0 σ).
-  Proof.
-    intros Hσ_dom Hσ0_lookup.
-    rewrite insert_union_with_l // -not_elem_of_dom.
-    rewrite -not_elem_of_dom in Hσ0_lookup.
-    set_solver.
   Qed.
 
   Lemma pstore_create_spec :
@@ -185,114 +749,972 @@ Section pstore_G.
       pstore_create ()
     {{{ t γ,
       RET t;
-      pstore_inv γ ∅ ∗
-      pstore_model t γ ∅
+        pstore γ t ∅
     }}}.
   Proof.
     iIntros "%Φ _ HΦ".
     wp_rec.
-    wp_alloc root as "Hroot".
-    iMod (pstore_map_alloc root) as "(%γ & Hmap_auth & Hmap_elem)".
-    iApply "HΦ".
-    iSplitR "Hmap_elem"; last iSteps.
-    iExists {[root := ∅]}, root. iFrame. iExists ∅.
-    iSplitR. { rewrite lookup_singleton //. }
-    iSplitR. { rewrite map_Forall_singleton //. }
-    iSplitR. { rewrite /pstore_store left_id big_sepM_empty //. }
-    rewrite delete_singleton big_sepM_empty //.
+    wp_alloc r as "Hroot".
+    wp_alloc t0 as "Ht0".
+    iMod (mono_map_alloc ∅) as "[%γ ?]".
+    iApply "HΦ". iModIntro.
+    iExists t0,r,∅,∅,{[r := ∅]},∅. iFrame.
+    rewrite !big_sepM_empty big_sepS_empty !right_id.
+    iPureIntro. split_and!; first done.
+    { constructor.
+      { rewrite dom_singleton_L vertices_empty //. set_solver. }
+      { set_solver. }
+      { rewrite lookup_insert //. }
+      { intros ????? Hr.
+        rewrite !lookup_singleton_Some.
+        inversion Hr; set_solver. } }
+    { constructor.
+      { intros ??. rewrite lookup_singleton_Some. intros (->&->). reflexivity. }
+      { intros ????. set_solver. } }
+    { eauto using rooted_dag_empty. }
+    { intros ??. set_solver. }
   Qed.
 
-  Lemma pstore_ref_spec γ σ0 v :
+  Lemma use_locs_of_edges_in g r xs r' X :
+    locs_of_edges_in g X ->
+    path g r xs r' ->
+    (list_to_set (proj2 <$> xs).*1) ⊆ X.
+  Proof.
+    intros He.
+    induction 1. set_solver.
+    apply He in H. set_solver.
+  Qed.
+
+  Lemma pstore_ref_spec γ t σ v :
     {{{
-      pstore_inv γ σ0
+      pstore γ t σ
     }}}
       pstore_ref v
-    {{{ r,
-      RET #r;
-      ⌜σ0 !! r = None⌝ ∗
-      pstore_inv γ (<[r := v]> σ0)
+    {{{ l,
+      RET #l;
+      ⌜l ∉ dom σ⌝ ∗
+      pstore γ t (<[l := v]> σ)
     }}}.
   Proof.
-    iIntros "%Φ (%map & %root & %σ_root & %Hmap_lookup_root & %Hmap & Hmap_auth & Hroot & Hσ_root & Hmap) HΦ".
-    assert (dom σ_root ⊆ dom σ0) as Hσ_root_dom.
-    { rewrite map_Forall_lookup in Hmap. naive_solver. }
-    wp_rec. wp_alloc r as "Hr".
+    iIntros (ϕ) open_inv. iIntros "HΦ".
+
+    wp_rec. wp_alloc l as "Hl".
     iApply "HΦ".
-    iAssert ⌜σ0 !! r = None⌝%I as %Hσ0_lookup.
-    { rewrite -not_elem_of_dom. iIntros "%Hr".
-      assert (∃ w, pstore_store σ0 σ_root !! r = Some w) as (w & Hunion_lookup).
-      { eexists. apply lookup_lookup_total_dom. rewrite pstore_store_dom //. }
-      iDestruct (big_sepM_lookup with "Hσ_root") as "Hr_"; first done.
-      iDestruct (pointsto_ne with "Hr Hr_") as %[]. done.
-    }
-    assert (σ_root !! r = None).
-    { rewrite -!not_elem_of_dom in Hσ0_lookup |- *. set_solver. }
-    iModIntro. iStep. iExists map, root. iFrame. iExists σ_root.
-    iSplit. { iPureIntro. set_solver. }
-    iSplit. { iPureIntro. eapply map_Forall_impl; first done. set_solver. }
-    iSplitR "Hmap".
-    { setoid_rewrite <- insert_union_with_l; last done.
-      iApply (big_sepM_insert_2 with "[Hr] Hσ_root").
-      iSteps.
-    }
-    iApply (big_sepM_impl with "Hmap"). iIntros "!> %l %σ %Hdelete_map_lookup (%r' & %v' & %l' & %σ' & %Hmap_lookup' & %Hdiff & Hl & Hmap_elem)".
-    iExists r', v', l', σ'. iSteps.
-    assert (dom σ ⊆ dom σ0) as Hσ_dom.
-    { rewrite map_Forall_lookup in Hmap. rewrite lookup_delete_Some in Hdelete_map_lookup. naive_solver. }
-    assert (σ !! r = None).
-    { rewrite -!not_elem_of_dom in Hσ0_lookup |- *. set_solver. }
-    assert (dom σ' ⊆ dom σ0) as Hσ'_dom.
-    { rewrite map_Forall_lookup in Hmap. naive_solver. }
-    rewrite pstore_store_insert // Hdiff pstore_store_insert // insert_commute //.
-  Abort.
 
-  #[local] Lemma pstore_reroot_spec γ σ0 map root l σ :
-    {{{
-      pstore_inv_inner γ σ0 map root ∗
-      pstore_map_elem γ l σ
-    }}}
-      pstore_reroot #l
-    {{{
-      RET ();
-      pstore_inv_inner γ σ0 map l
-    }}}.
-  Proof.
-  Abort.
+    iAssert ⌜σ0 !! l = None⌝%I as %Hl0.
+    { rewrite -not_elem_of_dom. iIntros (Hl).
+      apply elem_of_dom in Hl. destruct Hl.
+      iDestruct (big_sepM_lookup with "Hσ0") as "Hl_"; first done.
+      iDestruct (pointsto_ne with "Hl Hl_") as %?. done. }
+    assert (σ !! l = None).
+    { eapply not_elem_of_dom. apply not_elem_of_dom in Hl0.  destruct Hinv as [_ X].
+      apply incl_dom_incl in X. set_solver. }
+    iDestruct (pointsto_ne with "Hl Hr") as %Hlr.
 
-  Lemma pstore_get_spec {γ σ0 t σ r} v :
-    pstore_store σ0 σ !! r = Some v →
+    iModIntro. iSplitR. iPureIntro. by eapply not_elem_of_dom.
+    iExists t0,r, (<[l:=v]>σ0),g,((fun σ => <[l:=v]>σ)<$> M),C.
+
+    rewrite big_sepM_insert //. iFrame.
+    iPureIntro. split_and !; eauto.
+    { destruct Hinv as [X1 X2 X3 X4].
+      constructor.
+      { rewrite dom_fmap_L; set_solver. }
+      { eauto using gmap_included_insert. }
+      { rewrite lookup_fmap X3 //. }
+      { intros r1 ds r2 σ1 σ2 Hr. rewrite !lookup_fmap. generalize Hr. intros Hreach.
+        intros Hr1 Hr2.
+        destruct (M !! r1) eqn:Hor1. 2:simpl in *; congruence.
+        inversion Hr1. subst.
+        destruct (M !! r2) eqn:Hor2. 2:simpl in *; congruence.
+        inversion Hr2. subst.
+        destruct Hcoh as [Z1 Z2].
+        eapply use_locs_of_edges_in in Z2. 2:done.
+        rewrite apply_diffl_insert_ne.
+        { apply not_elem_of_dom in Hl0. set_solver. }
+        { f_equal. eauto. } } }
+    { destruct Hcoh as [X1 X2].
+      constructor.
+      { intros r' ?. rewrite lookup_fmap. intros E.
+        destruct (M !! r') eqn:Hor. 2:simpl in *; congruence.
+        inversion E. subst. rewrite !dom_insert_L. set_solver. }
+      { intros. rewrite dom_insert_L. intros ??. set_solver. } }
+    { intros ? r' ? HC. apply Hsnap in HC. destruct HC as (x&Hx&?).
+      exists (<[l:=v]>x). rewrite lookup_fmap Hx. split. done.
+      apply gmap_included_insert_notin; last done.
+      apply incl_dom_incl in H0. intros X. apply H0 in X.
+      destruct Hcoh as [X1 X2]. apply X1 in Hx.
+      apply not_elem_of_dom in Hl0. set_solver. }
+  Qed.
+
+  Lemma pstore_get_spec {γ t σ l} v :
+    σ !! l = Some v →
     {{{
-      pstore_inv γ σ0 ∗
-      pstore_model t γ σ
+      pstore γ t σ
     }}}
-      pstore_get t #r
+      pstore_get t #l
     {{{
       RET v;
-      pstore_inv γ σ0
+      pstore γ t σ
     }}}.
   Proof.
-  Abort.
+    iIntros (Hl ϕ) open_inv. iIntros "HΦ".
+    wp_rec. iStep 4. iModIntro.
 
-  Lemma pstore_set_spec γ σ0 t σ r v :
-    r ∈ dom σ0 →
+    iDestruct (big_sepM_lookup_acc _ _ l v with "[$]") as "(?&Hσ0)".
+    { destruct Hinv as [_ Hincl _ _].
+      specialize (Hincl l). rewrite Hl in Hincl. destruct (σ0!!l); naive_solver. }
+
+    iSteps.
+  Qed.
+
+  Lemma pstore_set_spec γ t σ l v :
+    l ∈ dom σ →
     {{{
-      pstore_inv γ σ0 ∗
-      pstore_model t γ σ
+      pstore γ t σ
     }}}
-      pstore_set t #r v
-    {{{ t',
-      RET t';
-      pstore_inv γ σ0 ∗
-      pstore_model t' γ (<[r := v]> (pstore_store σ0 σ))
+      pstore_set t #l v
+    {{{
+      RET ();
+      pstore γ t (<[l := v]> σ)
     }}}.
   Proof.
-  Abort.
+    iIntros (Hl Φ) open_inv. iIntros "HΦ".
+    wp_rec. iStep 8. iModIntro.
+    wp_alloc r' as "Hr'".
+
+    assert (exists w, σ0 !! l = Some w) as (w&Hl0).
+    { apply elem_of_dom. destruct Hinv as [_ Hincl].
+      apply incl_dom_incl in Hincl.
+      set_solver. }
+
+    iDestruct (big_sepM_insert_acc with "Hσ0") as "(?&Hσ0)". done.
+    wp_load. wp_load. wp_store. iStep 4. iModIntro.
+    wp_store. wp_store. iApply "HΦ".
+
+    iSpecialize ("Hσ0" with "[$]").
+
+    iAssert ⌜r ≠ r'⌝%I as %?.
+    { iClear "Ht0". iDestruct (pointsto_ne with "[$][$]") as %?. done. }
+
+    iAssert ⌜r' ∉ vertices g⌝%I as %Hr'.
+    { iIntros (Hr'). destruct Hgraph as [X1 X2].
+      apply X1 in Hr'. destruct Hr' as (?&Hr'). inversion Hr'; subst.
+      { done. }
+      { destruct b. iDestruct (big_sepS_elem_of with "[$]") as "?". done.
+        iDestruct (pointsto_ne r' r' with "[$][$]") as %?. congruence. } }
+
+    iModIntro. iExists t0,r',(<[l:=v]> σ0),({[(r,(l,w),r')]} ∪ g), (<[r':=<[l:=v]> σ0]>M),C.
+    rewrite big_sepS_union.
+    { apply disjoint_singleton_l. intros ?. apply Hr'.
+      apply elem_of_vertices. eauto. }
+    rewrite big_sepS_singleton. iFrame. iPureIntro.
+    split_and!; first done.
+    { destruct Hinv as [X1 X2 X3 X4].
+      constructor.
+      { rewrite dom_insert_L vertices_union vertices_singleton //. set_solver. }
+      { apply gmap_included_insert. done. }
+      { rewrite lookup_insert //. }
+      { intros r1 ds r2 σ1 σ2 Hreach.
+        destruct_decide (decide (r'=r1)).
+        { subst. rewrite lookup_insert. inversion_clear 1.
+          inversion Hreach. subst.
+          2:{ exfalso. subst. rewrite /edge elem_of_union in H0.
+              destruct H0. set_solver. apply Hr'. apply elem_of_vertices. set_solver. }
+          rewrite lookup_insert. inversion 1. done. }
+        rewrite lookup_insert_ne //. intros E1.
+        destruct_decide (decide (r2=r')).
+        { subst. rewrite lookup_insert. inversion 1. subst.
+          apply path_add_inv_r in Hreach; try done.
+          destruct Hreach as [(->&->)|(ds'&->&Hreach)].
+          { congruence. }
+          specialize (X4 _ _ _ _ _ Hreach E1 X3).
+          rewrite fmap_app apply_diffl_snoc insert_insert insert_id //. }
+        { rewrite lookup_insert_ne //. intros. eapply X4; eauto.
+          apply path_cycle_end_inv_aux in Hreach; eauto. } } }
+    { destruct Hcoh as [X1 X2].
+      constructor.
+      { intros r0 ?. destruct_decide (decide (r0=r')).
+        { subst. rewrite lookup_insert. inversion 1. done. }
+        rewrite lookup_insert_ne //. intros HM.
+        apply X1 in HM. rewrite dom_insert_lookup_L //. }
+      { intros ?. set_solver. } }
+    { eauto using rooted_dag_add. }
+    { intros ? r0 ? HC. apply Hsnap in HC. destruct HC as (?&HC&?).
+      destruct_decide (decide (r0=r')).
+      { exfalso. subst. destruct Hinv as [X1 X2 X3].
+        assert (r' ∉ dom M) as F by set_solver. apply F. by eapply elem_of_dom. }
+      rewrite lookup_insert_ne //. eauto. }
+  Qed.
+
+  Lemma pstore_capture_spec γ t σ :
+    {{{
+      pstore γ t σ
+    }}}
+      pstore_capture t
+    {{{ s,
+      RET s;
+      pstore γ t σ ∗
+      pstore_snapshot γ t s σ
+    }}}.
+  Proof.
+    iIntros (Φ) open_inv. iIntros "HΦ".
+    wp_rec. wp_load. do 5 iStep.
+
+    iMod (mono_map_insert' (fresh (dom C)) (r,σ) with "HC") as "(HC&Hsnap)".
+    { apply not_elem_of_dom. apply is_fresh. }
+    iModIntro.
+    iSplitR "Hsnap". 2:iSteps.
+    iExists _,_,_,_,_,_. iFrame.
+    iPureIntro. split_and!; eauto.
+    intros ? r' ? HC.
+    destruct_decide (decide (n=fresh (dom C))).
+    { subst. rewrite lookup_insert in HC. inversion HC. subst.
+      destruct Hinv. eauto. }
+    { rewrite lookup_insert_ne // in HC. eauto. }
+  Qed.
+
+  Definition fsts  (ys:list (loc*(loc*val)*loc)) : list val :=
+    (fun '(x,_,_) => ValLoc x) <$> ys.
+
+  Lemma pstore_collect_spec_aux (r r':loc) t' (xs:list val) (ys:list (loc*(loc*val)*loc)) (g:graph_store) :
+    lst_model' t' xs ->
+    path g r ys r' ->
+    {{{
+      r' ↦ §Root ∗
+      ([∗ set] '(r, (l, v), r') ∈ g, r ↦ ’Diff{ #(l : loc), v, #(r' : loc) })
+    }}}
+      pstore_collect #r t'
+    {{{ t,
+      RET (#r',t);
+      r' ↦ §Root ∗
+      ([∗ set] '(r, (l, v), r') ∈ g, r ↦ ’Diff{ #(l : loc), v, #(r' : loc) }) ∗
+      lst_model t (rev_append (fsts ys) xs)
+    }}}.
+  Proof.
+    iIntros (-> Hpath Φ) "(Hr'&Hg) HΦ".
+    iInduction ys as [|] "IH" forall (r xs r' Hpath); wp_rec.
+    { inversion Hpath. subst. iSteps. }
+    { inversion Hpath. subst.
+      iDestruct (big_sepS_elem_of_acc _ _ (r,b,a2) with "[$]") as "(?&Hg)".
+      { set_solver. } destruct b.
+      wp_load.
+      iSpecialize ("Hg" with "[$]").
+      iSpecialize ("IH" with "[%//][$][$][$]").
+      iSteps.
+    }
+  Qed.
+
+  Lemma pstore_collect_spec (r r':loc) (ys:list (loc*(loc*val)*loc)) (g:graph_store) :
+    path g r ys r' ->
+    {{{
+      r' ↦ §Root ∗
+      ([∗ set] '(r, (l, v), r') ∈ g, r ↦ ’Diff{ #(l : loc), v, #(r' : loc) })
+    }}}
+      pstore_collect #r §Nil
+    {{{ t,
+      RET (#r',t);
+      r' ↦ §Root ∗
+      ([∗ set] '(r, (l, v), r') ∈ g, r ↦ ’Diff{ #(l : loc), v, #(r' : loc) }) ∗
+      lst_model t (rev (fsts ys))
+    }}}.
+  Proof.
+    iIntros (? Φ) "(?&?) HΦ".
+    iDestruct (pstore_collect_spec_aux with "[$]") as "Go"; [done.. |].
+    rewrite -lst_to_val_nil.
+    iApply "Go". rewrite -rev_alt //.
+  Qed.
+
+  Lemma use_path r g (xs:list (loc*(loc*val)*loc)) r0 x r1 r':
+    list_to_set xs ⊆ g ->
+    path g r (xs ++ [(r0, x, r1)]) r' ->
+    (r0, x, r1) ∈ (list_to_set xs : gset(loc*(loc*val)*loc) ) ->
+    exists ds, path g r0 ds r0 /\ ds ≠ nil.
+  Proof.
+    revert r r0 r1 r' x. induction xs; intros r r0 r1 r' x ?.
+    { set_solver. }
+    rewrite -app_comm_cons. inversion 1. subst.
+    rewrite list_to_set_cons.
+    destruct_decide (decide ((r0, x, r1) = (r, b, a2))) as X.
+    { inversion X. subst. intros _. clear IHxs.
+      rewrite app_comm_cons in H0. apply path_snoc_inv in H0.
+      destruct H0 as (?&?&?). subst a2.
+      exists (((r, b, r') :: xs)). done. }
+    { intros ?. apply IHxs in H6. 2,3:set_solver.
+      destruct H6 as (?&?&?). eexists. split; last done.
+      eapply path_weak. done. set_solver. }
+  Qed.
+
+  (* [undo xs ys σ] asserts [mirror xs ys] and that [σ = apply_diffl (proj2 <$> ys ++ xs) σ],
+     ie, ys undo the changes of xs *)
+  Inductive undo :
+    list (loc*(loc*val)*loc) -> list (loc*(loc*val)*loc) -> gmap loc val -> Prop :=
+  | undo_nil :
+    forall σ, undo [] [] σ
+  | undo_cons :
+    forall σ r l v v' r' xs ys,
+      σ !! l = Some v' ->
+      undo xs ys (<[l:=v]> σ) ->
+      undo (xs++[(r,(l,v),r')]) ((r',(l,v'),r)::ys) σ.
+
+  Lemma use_undo xs ys σ :
+    undo xs ys σ ->
+    σ = apply_diffl (proj2 <$> ys ++ xs) σ.
+  Proof.
+    induction 1.
+    { done. }
+    rewrite !assoc_L fmap_app apply_diffl_snoc.
+    rewrite -app_comm_cons fmap_cons apply_diffl_cons.
+    rewrite -IHundo insert_insert insert_id //.
+  Qed.
+
+  Lemma undo_mirror xs ys g :
+    undo xs ys g ->
+    mirror xs ys.
+  Proof.
+    induction 1; eauto using mirror_cons,mirror_nil.
+  Qed.
+
+  Lemma pstore_revert_spec_aux g g1 r t g2 xs r' w σ σ0 :
+    lst_model' t (fsts (rev xs)) ->
+    locs_of_edges_in g2 (dom σ) ->
+    g2 = list_to_set xs ->
+    acyclic g ->
+    g2 ⊆ g ->
+    path g r xs r' ->
+    {{{
+      r' ↦ w ∗
+      ([∗ map] l0↦v0 ∈ σ, l0 ↦ v0) ∗
+      ([∗ set] '(r, (l, v), r') ∈ g1, r ↦ ’Diff{ #(l : loc), v, #(r' : loc) }) ∗
+      ([∗ set] '(r, (l, v), r') ∈ g2, r ↦ ’Diff{ #(l : loc), v, #(r' : loc) })
+    }}}
+      pstore_revert #r' t
+    {{{
+      RET ();
+      ∃ ys,
+      ⌜undo xs ys σ⌝ ∗
+      r ↦ §Root ∗
+      ([∗ set] '(r, (l, v), r') ∈ (g1 ∪ list_to_set ys), r ↦ ’Diff{ #(l : loc), v, #(r' : loc) }) ∗
+      ([∗ map] l0↦v0 ∈ (apply_diffl (proj2 <$> xs) σ), l0 ↦ v0)
+    }}}.
+  Proof.
+    iIntros (-> Hlocs Hg Hacy Hsub Hpath Φ) "(Hr'&Hσ&Hg1&Hg2) HΦ".
+    iInduction xs as [|((r0,(l,v)),r1) ] "IH" using rev_ind forall (σ w r r' g1 g2  Hpath Hg Hlocs Hacy Hsub).
+    { wp_rec. simpl.
+      iStep 4. iModIntro.
+      inversion Hpath. subst. wp_store. iModIntro.
+      iApply "HΦ". iExists nil. rewrite !right_id_L. iFrame.
+      iPureIntro. eauto using undo_nil. }
+    { wp_rec. simpl. rewrite rev_unit. simpl.
+      iStep 4. iModIntro.
+      rewrite Hg list_to_set_app_L list_to_set_cons list_to_set_nil right_id_L.
+      rewrite Hg list_to_set_app_L in Hsub.
+      assert ((r0, (l, v), r1) ∉ (list_to_set xs : gset (loc * diff * loc))).
+      { intros ?. apply use_path in Hpath; last done. destruct Hpath as (?&Hpath&?).
+        apply Hacy in Hpath. congruence. set_solver. }
+      iDestruct (big_sepS_union with "Hg2") as "(Hg2&?)".
+      { set_solver. }
+      rewrite big_sepS_singleton. wp_load. iStep 4. iModIntro.
+
+      rewrite Hg list_to_set_app_L list_to_set_cons list_to_set_nil right_id_L in Hlocs.
+      assert (exists v', σ !! l = Some v') as (v',Hl).
+      { apply elem_of_dom. eapply Hlocs. rewrite /edge.
+
+        rewrite elem_of_union elem_of_singleton. right. reflexivity. }
+
+      apply path_snoc_inv in Hpath. destruct Hpath as (?&->&?).
+      wp_smart_apply assert_spec. rewrite bool_decide_eq_true_2 //.
+      iStep 4. iModIntro.
+
+      iDestruct (big_sepM_insert_acc with "Hσ") as "(?&Hσ)". done.
+      wp_load. wp_store. wp_store. iStep 4. iModIntro.
+
+      iSpecialize ("Hσ" with "[$]").
+      iSpecialize ("IH" with "[%//][%//][%][%//][%][$][$] Hg1 Hg2").
+      { rewrite dom_insert_lookup_L //. intros x1 x2 x3 x4.
+        specialize (Hlocs x1 x2 x3 x4). set_solver. }
+      { set_solver. }
+
+      rewrite fmap_app -apply_diffl_snoc. simpl.
+      iApply "IH". iModIntro.
+      iIntros "[%ys (%Hundo&?&?&?)]". iApply "HΦ".
+      iExists ((r',(l,v'),r0)::ys). iFrame.
+      iSplitR.
+      { iPureIntro. eauto using undo_cons. }
+      rewrite list_to_set_cons.
+      iAssert ⌜(r', (l, v'), r0) ∉ g1 ∪ list_to_set ys⌝%I as "%".
+      { iIntros (?). iDestruct (big_sepS_elem_of with "[$]") as "?". done.
+        iDestruct (pointsto_ne r' r' with "[$][$]") as "%". congruence. }
+      replace (g1 ∪ ({[(r', (l, v'), r0)]} ∪ list_to_set ys)) with ({[(r', (l, v'), r0)]} ∪ ((g1 ∪ list_to_set ys))). 2:set_solver.
+      iApply big_sepS_union. set_solver.
+      iFrame. rewrite big_sepS_singleton //. }
+  Qed.
+
+  Lemma pstore_revert_spec r t g xs r' w σ σ0 :
+    lst_model' t (fsts (rev xs)) ->
+    locs_of_edges_in g (dom σ) ->
+    g = list_to_set xs ->
+    acyclic g ->
+    path g r xs r' ->
+    {{{
+      r' ↦ w ∗
+      ([∗ map] l0↦v0 ∈ σ, l0 ↦ v0) ∗
+      ([∗ set] '(r, (l, v), r') ∈ g, r ↦ ’Diff{ #(l : loc), v, #(r' : loc) })
+    }}}
+      pstore_revert #r' t
+    {{{
+      RET ();
+      ∃ ys,
+      ⌜undo xs ys σ⌝ ∗
+      r ↦ §Root ∗
+      ([∗ set] '(r, (l, v), r') ∈ (list_to_set ys), r ↦ ’Diff{ #(l : loc), v, #(r' : loc) }) ∗
+      ([∗ map] l0↦v0 ∈ (apply_diffl (proj2 <$> xs) σ), l0 ↦ v0)
+    }}}.
+  Proof.
+    iIntros (->???? Φ) "(?&?&?) HΦ".
+    iApply (pstore_revert_spec_aux g ∅ with "[-HΦ]"); try done.
+    { rewrite big_sepS_empty. iFrame. }
+    { iModIntro. iIntros "[% ?]". iApply "HΦ". iExists _. rewrite left_id_L //. }
+  Qed.
+
+  Lemma rev_fsts xs :
+    rev (fsts xs) = fsts (rev xs).
+  Proof.
+    induction xs as [|((?,?),?)]; simpl; eauto.
+    rewrite IHxs /fsts fmap_app //.
+  Qed.
+
+  Lemma pstore_reroot_spec r (xs:list (loc*(loc*val)*loc)) r' g σ :
+    locs_of_edges_in g (dom σ) ->
+    g = list_to_set xs ->
+    acyclic g ->
+    path g r xs r' ->
+    {{{
+      r' ↦ §Root ∗
+      ([∗ map] l0↦v0 ∈ σ, l0 ↦ v0) ∗
+      ([∗ set] '(r, (l, v), r') ∈ g, r ↦ ’Diff{ #(l : loc), v, #(r' : loc) })
+    }}}
+      pstore_reroot #r
+    {{{
+      RET ();
+      ∃ ys,
+      ⌜undo xs ys σ⌝ ∗
+      r ↦ §Root ∗
+      ([∗ set] '(r, (l, v), r') ∈ (list_to_set ys), r ↦ ’Diff{ #(l : loc), v, #(r' : loc) }) ∗
+      ([∗ map] l0↦v0 ∈ (apply_diffl (proj2 <$> xs) σ), l0 ↦ v0)
+    }}}.
+  Proof.
+    iIntros (???? Φ) "(Hr'&Hσ&Hg) HΦ".
+    wp_rec. wp_apply (pstore_collect_spec with "[$]"). done.
+    iIntros (?) "(?&?&%Heq)". rewrite {}Heq.
+    wp_smart_apply (pstore_revert_spec with "[-HΦ]"); try done; first rewrite rev_fsts //.
+    iSteps.
+  Qed.
+
+  Lemma locs_of_edges_weak g1 g2 X :
+    locs_of_edges_in g1 X ->
+    g2 ⊆ g1 ->
+    locs_of_edges_in g2 X.
+  Proof.
+    intros Z ? a b c d ?. eapply (Z a b c d). set_solver.
+  Qed.
+
+  Lemma undo_same_fst_label xs ys r l v r' σ :
+    undo xs ys σ ->
+    (r, (l, v), r') ∈ (list_to_set ys :  gset (loc*(loc*val)*loc)) ->
+    l ∈ (list_to_set (proj2 <$> xs).*1 : gset loc).
+  Proof.
+    revert xs σ. induction ys as [|(?,?)]. set_solver.
+    intros xs σ. inversion 1. subst.
+    simpl. rewrite !fmap_app list_to_set_app_L. simpl in *. subst.
+    destruct_decide (decide ((r, (l, v), r') = (r'0, (l1, v'), l0))) as Heq.
+    { inversion Heq. subst. intros _. set_solver. }
+    intros ?. simpl. apply elem_of_union. left. eapply IHys. done. set_solver.
+  Qed.
+
+  Definition diff_last {A:Type} (ys1 ys2:list A) :=
+    match last ys1, last ys2 with
+    | Some x, Some y =>
+        x ≠ y
+    | _, _ =>
+        True
+    end.
+
+  Lemma path_extract_suffix (g:gset (loc*(loc*val)*loc)) a1 a2 xs1 r xs2 :
+    unaliased g ->
+    path g a1 xs1 r ->
+    path g a2 xs2 r  ->
+    exists ys1 ys2 xs,
+      xs1 = ys1 ++ xs /\
+      xs2 = ys2 ++ xs /\ diff_last ys1 ys2.
+  Proof.
+    intros Hinj.
+    revert r a1 a2 xs2. induction xs1 using rev_ind; intros r a1 a2 xs2.
+    { inversion 1. subst. intros. exists nil,xs2,nil.
+      simpl. rewrite right_id_L. set_solver. }
+    intros Hp1 Hp2. apply path_inv_r in Hp1.
+    destruct Hp1 as [? | (bs'&b'&y&X1&X2&X3)].
+    { destruct xs1; naive_solver. }
+    apply app_inj_tail in X1. destruct X1 as (<-&->).
+
+    apply path_inv_r in Hp2. destruct Hp2 as [(->&->) | (bs'&b&y'&->&?&?)].
+    { exists (xs1 ++ [(y, b', r)]),nil,nil. rewrite right_id. split_and !; try done.
+      unfold diff_last. destruct (last (xs1 ++ [(y, b', r)])); try done. }
+
+    destruct_decide (decide (y'=y)); last first.
+    { eexists _,_,nil. rewrite !right_id_L. split_and!; try done.
+      unfold diff_last. rewrite !last_app. simpl. naive_solver. }
+    subst.
+
+    destruct (IHxs1 _ _ _ _ X2 H) as (ys1&ys2&xs&->&->&Hdiff).
+    destruct (Hinj _ _ _ _ _ X3 H0) as (->&_).
+    eexists _,_,(xs++[(y, b, r)]). rewrite !assoc_L. done.
+  Qed.
+
+  Lemma diff_last_app_middle {A:Type} x (l1' l2' l1 l2:list A) :
+    diff_last (l1' ++ x :: l2') (l1 ++ x :: l2) ->
+    diff_last (x :: l2') (x :: l2).
+  Proof.
+    unfold diff_last. rewrite !last_app !last_cons.
+    destruct (last l2),(last l2'); eauto.
+  Qed.
+
+  Lemma diff_last_irrefl {A:Type} (l:list A) :
+    l ≠ nil ->
+    ¬ (diff_last l l).
+  Proof.
+    destruct (list_case_r l) as [|(?&?&->)]. naive_solver.
+    intros _. unfold diff_last.
+    rewrite !last_app //. simpl. naive_solver.
+  Qed.
+
+  Lemma path_use_diff_last (g:gset (loc*(loc*val)*loc)) a1 a2 ys1 ys2 xs r :
+    acyclic g ->
+    unaliased g ->
+    path g a1 (ys1 ++ xs) r ->
+    path g a2 (ys2 ++ xs) r  ->
+    diff_last ys1 ys2 ->
+    forall x, x ∈ ys2 -> x ∉ (ys1 ++ xs).
+  Proof.
+    intros Hacy Hroot Hp1 Hp2 Hdiff x Hx Hx'.
+    apply elem_of_app in Hx'. destruct Hx' as [Hx'|Hx'].
+    (* contradicts diff_last. *)
+    { apply elem_of_middle in Hx,Hx'.
+      destruct Hx as (l1&l2&->).
+      destruct Hx' as (l1'&l2'&->).
+      rewrite -!assoc_L in Hp1,Hp2.
+      apply path_app_inv in Hp1,Hp2.
+      destruct Hp1 as (x1&_&Hp1).
+      destruct Hp2 as (x2&_&Hp2).
+      rewrite -!app_comm_cons in Hp1,Hp2.
+      assert (x1=proj1 x).
+      { inversion Hp1. subst. done. }
+      assert (x2=proj1 x).
+      { inversion Hp2. subst. done. }
+      subst.
+      eapply acyclic_unaliased_impl_uniq_path in Hp2; eauto.
+      apply Hp2 in Hp1.
+      rewrite !app_comm_cons in Hp1.
+      apply app_inv_tail in Hp1.
+      apply diff_last_app_middle in Hdiff.
+      rewrite Hp1 in Hdiff.
+      eapply diff_last_irrefl; last done. done. }
+    (* There is a loop. *)
+    { apply elem_of_middle in Hx,Hx'.
+      destruct Hx as (l1&l2&->).
+      destruct Hx' as (l1'&l2'&->).
+      rewrite -assoc_L in Hp2.
+      apply path_app_inv in Hp2.
+      destruct Hp2 as (?&_&Hp2).
+      rewrite assoc_L  in Hp2.
+      apply path_app_inv in Hp2.
+      destruct Hp2 as (?&Hp2&Hp2').
+      assert (x0 = proj1 x) as ->.
+      { inversion Hp2. subst. done. }
+      assert (x1 = proj1 x) as ->.
+      { inversion Hp2'. subst. done. }
+      rewrite -app_comm_cons in Hp2.
+      eapply Hacy in Hp2. congruence. }
+  Qed.
+
+  Lemma diff_last_comm {A:Type} (l1 l2:list A) :
+    diff_last l1 l2 <-> diff_last l2 l1.
+  Proof.
+    unfold diff_last.
+    destruct (last l1),(last l2); naive_solver.
+  Qed.
+
+  Lemma path_union_inv (g1: graph loc (loc*val)) g2 a1 xs a2 :
+    path (g1 ∪ g2) a1 xs a2 ->
+    path g1 a1 xs a2 \/ exists a' x xs1 xs2, path g1 a1 xs1 a' /\ x ∈ g2 /\ path (g1 ∪ g2) a' (x::xs2) a2 /\ xs=xs1++x::xs2.
+  Proof.
+    induction 1.
+    left. eauto using path_nil.
+    destruct IHpath as [|(x&?&?&?&?&?&?&->)].
+    { destruct_decide (decide ((a1,b,a2) ∈ g1)).
+      { left. apply path_cons; eauto. }
+      { right. exists a1,(a1,b,a2),nil. eexists. split_and !. apply path_nil. set_solver.
+        apply path_cons. set_solver. eauto. done. } }
+    { right.
+      destruct_decide (decide ((a1,b,a2) ∈ g1)).
+      { eexists _,_,_,_. split_and !;eauto.
+        2:{ rewrite app_comm_cons. reflexivity. }
+        apply path_cons. set_solver. done. }
+      eexists _,_,_,_. split_and !. apply path_nil.
+      3:{ simpl. reflexivity. }
+      set_solver. apply path_cons. set_solver. done. }
+  Qed.
+
+  Lemma path_cannot_escape (x:(loc * diff * loc)) (xs ys:list (loc * diff * loc)) (g1: graph loc (loc*val)) a a' r :
+    (forall x l', ¬ (r,x,l') ∈ (g1 ∪ list_to_set ys)) ->
+    unaliased (g1 ∪ list_to_set ys) ->
+    x ∈ (list_to_set ys : gset _) ->
+    pathlike ys r ->
+    path (g1 ∪ list_to_set ys) a (x :: xs) a' ->
+    path (list_to_set ys) a (x::xs) a'.
+  Proof.
+    intros ? X1 X2 X3. remember (x::xs) as zs.
+    revert a a' x xs Heqzs X1 X2 X3.
+    induction zs; intros a0 a' x xs Heqzs X1 X2 X3. congruence.
+    inversion 1. subst. inversion Heqzs. subst. apply path_cons. eauto.
+    destruct xs as [|((?,?),?)].
+    { inversion H6. subst. eauto using path_nil. }
+    eapply IHzs; eauto. inversion H6. subst.
+    apply elem_of_list_to_set in X2. apply X3 in X2.
+    destruct X2 as [|(?&?&?)]. naive_solver.
+    assert ((l, x, x0) ∈  g1 ∪ list_to_set ys) as Z. set_solver.
+    destruct (X1 _ _ _ _ _ H9 Z). set_solver.
+  Qed.
+
+  Lemma path_in_seg_complete (r a a':loc) (x:(loc * diff * loc)) (xs0 xs1 ys: list (loc * diff * loc)) (g1:graph loc (loc*val)) :
+    (forall x l', ¬ (r,x,l') ∈ (g1 ∪ list_to_set ys)) -> (* root has no succ *)
+    unaliased (g1 ∪ list_to_set ys) ->
+    pathlike ys r ->
+    path (g1 ∪ list_to_set ys) a xs0 a' ->
+    path (list_to_set ys) a' (x :: xs1) a ->
+    exists zs, path (list_to_set ys) a zs a'.
+  Proof.
+    intros Hroot Hinj Hclosed Hp1 Hp2.
+    inversion Hp1.
+    { subst. exists nil. apply path_nil. }
+    subst. eapply path_cannot_escape in Hp1; eauto.
+    apply path_inv_r in Hp2.
+    destruct Hp2 as [|(?&?&?&Heq&Hp2&Hys)].
+    { exfalso. destruct xs1; naive_solver. }
+    apply elem_of_list_to_set in Hys.
+    apply Hclosed in Hys. destruct Hys as [->|(?&?&Hys)].
+    { naive_solver. }
+    assert ((a, x3, x4) ∈  g1 ∪ list_to_set ys) as Z. set_solver.
+    destruct (Hinj _ _ _ _ _ H Z). set_solver.
+  Qed.
+
+  Lemma undo_preserves_rooted_dag (g:graph loc (loc*val)) xs ys rs r :
+    (forall x l', ¬ (rs,x,l') ∈ (list_to_set ys ∪ g ∖ list_to_set xs)) -> (* root has no succ *)
+    unaliased g ->
+    unaliased (list_to_set ys ∪ g ∖ list_to_set xs) ->
+    path g rs xs r ->
+    mirror xs ys ->
+    rooted_dag g r ->
+    rooted_dag (list_to_set ys ∪ g ∖ list_to_set xs) rs.
+  Proof.
+    intros Hnr Hinj Hinj' Hpath Hmirror Hroot. inversion Hroot as [X1 X2].
+    assert (vertices (list_to_set ys ∪ g ∖ list_to_set xs) = vertices g) as Hvg.
+    { apply mirror_vertices in Hmirror.
+      rewrite vertices_union Hmirror -vertices_union -union_difference_L //.
+      eauto using path_all_in. }
+
+    constructor.
+    { intros a. rewrite Hvg => Ha.
+      apply X1 in Ha. destruct Ha as (zs&Ha).
+      edestruct (path_extract_suffix g a rs) as (ys1&ys2&us&?&?&Hlast); eauto. subst.
+
+      apply path_middle in Ha. destruct Ha as (y&Hy1&Hy2).
+      apply path_middle in Hpath. destruct Hpath as (y'&Hy'1&Hy'2).
+      assert (y'=y) as ->.
+      { inversion Hy'2; subst; inversion Hy2; naive_solver. }
+      eapply use_mirror_subset in Hmirror. 3:apply Hy'1. 2:set_solver.
+      destruct Hmirror as (zs&Hzs&_).
+      exists (ys1++zs). eapply path_app.
+      2:{ eapply path_weak. done. set_solver. }
+      clear X2. induction Hy1.
+      { apply path_nil. }
+      apply path_cons.
+      { rewrite elem_of_union elem_of_difference. right. split. set_solver.
+        apply not_elem_of_list_to_set.
+        eapply path_use_diff_last. 1,2: eauto using ti2.
+        3:{ apply diff_last_comm. done. }
+        { eapply path_app; eauto. }
+        { rewrite -app_comm_cons. eapply path_cons. done.
+          eapply path_app; eauto. }
+        { set_solver. } }
+      { apply IHHy1; eauto.  unfold diff_last in *. rewrite last_cons in Hlast.
+        destruct (last bs), (last ys2); try done. } }
+    { intros a zs Hzs. rewrite comm_L in Hzs.
+      apply path_union_inv in Hzs. destruct Hzs as [Hsz|Hsz].
+      (* The cycle is only in g, easy. *)
+      { eapply X2. eapply path_weak. done. set_solver. }
+      (* There is at least a vertex in ys.
+         We are going to construct a cycle in ys, implying a cycle in xs. *)
+      exfalso. destruct Hsz as (a'&x&l1&l2&E1&Hx&E2&->).
+
+      apply path_cannot_escape with (r:=rs) in E2; last first.
+      { eapply path_pathlike. eapply use_mirror; eauto. }
+      { done. }
+      { rewrite comm_L //. }
+      { set_solver. }
+
+      eapply path_weak in E1.
+      eapply path_in_seg_complete with (r:=rs) in E1; last first. done.
+      { eapply path_pathlike. eapply use_mirror; eauto. }
+      { rewrite comm_L //. }
+      { set_solver. }
+      2:{ set_solver. }
+      destruct E1 as (?&E1).
+
+      assert (path (list_to_set ys) a (x0 ++ x::l2) a ) as Hcycle.
+      { eapply path_app. done. done. }
+
+      eapply use_mirror_subset with (ys:=xs) in Hcycle.
+      3:{ by apply mirror_symm. }
+      2:{ apply path_all_in in Hcycle. set_solver. }
+      destruct Hcycle as (?&Hcycle&F).
+      eapply path_weak in Hcycle. 2:eapply path_all_in; done.
+      eapply ti2 in Hcycle; eauto. subst. destruct x0; simpl in *; lia. }
+  Qed.
+
+  Lemma undo_app_inv xs ys1 ys2 σ :
+    undo xs (ys1 ++ ys2) σ ->
+    exists xs1 xs2, xs = xs2 ++ xs1 /\ undo xs2 ys2 (apply_diffl (proj2 <$> xs1) σ) /\ undo xs1 ys1 σ.
+  Proof.
+    revert xs ys2 σ. induction ys1; intros xs ys2 σ Hundo.
+    { exists nil,xs. rewrite right_id_L. split; eauto using undo_nil. }
+    rewrite -app_comm_cons in Hundo. inversion Hundo. subst.
+    apply IHys1 in H4. destruct H4 as (xs1&xs2&->&?&?).
+    eexists _,xs2. split_and !.
+    { rewrite -assoc_L //. }
+    { rewrite fmap_app apply_diffl_app. done. }
+    { apply undo_cons. done. done. }
+  Qed.
+
+  Lemma construct_middlepoint (g:graph loc (loc*val)) a1 xs ys a2 a2' :
+    unaliased g ->
+    (forall x l', ¬ (a2,x,l') ∈ g) -> (* root has no succ *)
+    path g a1 xs a2 ->
+    path g a1 ys a2' ->
+    exists zs, xs = ys ++ zs.
+  Proof.
+    intros Hinj Hroot Hpath. revert ys. induction Hpath; intros ys.
+    { intros Hpath. inversion Hpath. eauto. subst. set_solver. }
+    { intros X. inversion X; subst.
+      { exists ((a2', b, a2) :: bs ). done. }
+      destruct (Hinj _ _ _ _ _ H H0). subst.
+      apply IHHpath in H1. destruct H1 as (?&?).
+      eexists. rewrite -app_comm_cons H1 //.
+      intros ??. apply Hroot. }
+  Qed.
+
+
+  Lemma undo_preserves_model g (M:map_model) (xs ys:list (loc* (loc*val)*loc)) rs σ0 r:
+    dom M = vertices g ∪ {[r]} ->
+    correct_path_diff M g ->
+    (forall x l', ¬ (rs,x,l') ∈ (list_to_set ys ∪ g ∖ list_to_set xs)) -> (* root has no succ *)
+    unaliased (g ∖ list_to_set xs ∪ list_to_set ys) ->
+    path g rs xs r ->
+    undo xs ys σ0 ->
+    M !! r = Some σ0 ->
+    correct_path_diff M (list_to_set ys ∪ g ∖ list_to_set xs).
+  Proof.
+    intros Hdom Hinv Hroot Hinj' Hrs Hundo E0.
+    intros r1 zs r2 σ1 σ2 Hpath E1 E2. rewrite comm_L in Hpath.
+    apply path_union_inv in Hpath. destruct Hpath as [Hpath|Hpath].
+
+    (* If the path is entirely in g, easy. *)
+    { eapply Hinv; eauto. eapply path_weak. done. set_solver. }
+
+    assert (mirror xs ys) as Hmirror by eauto using undo_mirror.
+
+    destruct Hpath as (a'&x&l1&l2&X1&Hx&X2&Hzs).
+    eapply path_cannot_escape with (r:=rs) in X2; eauto; last first.
+    { eapply path_pathlike. eapply use_mirror; eauto. }
+    { set_solver. }
+
+    (* otherwise the path includes a part in g, and a part in ys. *)
+
+    assert (vertices (list_to_set ys ∪ g ∖ list_to_set xs) = vertices g) as Hvg.
+    { apply mirror_vertices in Hmirror.
+      rewrite vertices_union Hmirror -vertices_union -union_difference_L //.
+      eauto using path_all_in. }
+
+    assert (a' ∈ dom M) as Ha'.
+    { rewrite Hdom -Hvg elem_of_union. left. apply elem_of_vertices.
+      inversion X2. set_solver. }
+    apply elem_of_dom in Ha'. destruct Ha' as (σ',Ea').
+    assert (σ1 = (apply_diffl (proj2 <$> l1) σ')).
+    { eapply path_weak in X1.
+      eapply (Hinv _ _ _ _ _ X1 E1 Ea'). set_solver. }
+
+    (* The part in g is preserved. *)
+
+    etrans. done. rewrite Hzs. rewrite fmap_app apply_diffl_app.
+    f_equal. clear dependent σ1 l1.
+
+    (* XXX facto a lemma. *)
+    assert (exists u1 u2, ys = u1 ++ (x::l2) ++ u2) as (u1&u2&Hys).
+    { eapply use_mirror in Hrs. 2:done.
+      apply elem_of_list_to_set, elem_of_middle in Hx.
+      destruct Hx as (p1&p2&->).
+      apply path_app_inv in Hrs. destruct Hrs as (?&Hp1&Hp2).
+      inversion Hp2; inversion X2. subst. inversion H5. subst.
+      eapply construct_middlepoint in H10. 4:apply H4.
+      2:{ intros z1 z2 z3 z4 z5 ??. eapply (Hinj' z1 z2 z3 z4 z5); try done.
+          all:apply elem_of_union; right. all:set_solver. }
+      2:{ intros x l' X. eapply (Hroot x l').
+          apply elem_of_union. left. set_solver. }
+      destruct H10.
+      eexists _,_. f_equal. rewrite -app_comm_cons. f_equal. done. }
+
+    rewrite Hys assoc_L in Hundo. apply undo_app_inv in Hundo.
+    destruct Hundo as (xs1&xs2&->&Hundo1&Hundo2).
+    apply undo_app_inv in Hundo2.
+    destruct Hundo2 as (xs4&xs3&->&Hundo2&Hundo3).
+
+    eapply use_mirror in Hmirror. 2:done.
+    rewrite {2}Hys in Hmirror.
+    apply path_app_inv in Hmirror. destruct Hmirror as (n1&T1&T2).
+    apply path_app_inv in T2. destruct T2 as (n2&T2&T3).
+    edestruct (same_path (list_to_set ys) (x::l2) n1 n2 a') as (?&?); try done.
+    subst n1 n2.
+
+    assert (path g a' xs4 r) as R1.
+    { eapply path_weak.
+      eapply use_mirror. eapply mirror_symm. eauto using undo_mirror. done.
+      apply path_all_in in Hrs. set_solver. }
+    apply (Hinv _ _ _ σ' σ0) in R1; try done.
+
+    assert (path g r2 xs3 a') as R2.
+    { eapply path_weak.
+      eapply use_mirror. eapply mirror_symm. eauto using undo_mirror. done.
+      apply path_all_in in Hrs. set_solver. }
+    eapply (Hinv _ _ _ σ2 σ') in R2; try done.
+    rewrite R2. rewrite -apply_diffl_app -fmap_app.
+    eapply use_undo. rewrite R1. done.
+  Qed.
+
+  Lemma pstore_restore_spec γ t σ s σ' :
+    {{{
+      pstore γ t σ ∗
+      pstore_snapshot γ t s σ'
+    }}}
+      pstore_restore t s
+    {{{
+      RET ();
+      pstore γ t σ'
+    }}}.
+  Proof.
+    iIntros (Φ) "(HI&Hsnap) HΦ".
+    iDestruct "HI" as open_inv.
+    iDestruct "Hsnap" as "(%rs&%&->&Hsnap)".
+    wp_rec. iStep 20.
+
+    iDestruct (extract_unaliased with "Hg") as "%".
+
+    iDestruct (mono_map_elem_valid with "[$][$]") as "%Hrs".
+    apply Hsnap in Hrs. destruct Hrs as (σ1&HMrs&?).
+
+    destruct_decide (decide (rs=r)).
+    { subst.
+      subst.
+      wp_load. iStep 4. iModIntro.
+      iExists _,_,_,_,_,_. iFrame. iPureIntro. split_and!; eauto.
+      { destruct Hinv as [X1 X2 X3 X4]. constructor; eauto. naive_solver. } }
+
+    assert (rs ∈ vertices g) as Hrs.
+    { destruct Hinv. apply elem_of_dom_2 in HMrs. set_solver. }
+
+    eapply ti1 in Hrs; eauto. destruct Hrs as (ds,Hrs).
+    inversion Hrs. congruence. subst. rename a2 into r'. destruct b.
+    iDestruct (big_sepS_elem_of_acc with "[$]") as "(?&Hg)". done. simpl.
+    wp_load. iStep 2. iModIntro.
+    iSpecialize ("Hg" with "[$]").
+
+    remember ((rs, (l, v), r') :: bs) as xs.
+    assert (list_to_set xs ⊆ g).
+    { eauto using path_all_in. }
+
+    rewrite (union_difference_L (list_to_set xs) g) //.
+
+    iDestruct (big_sepS_union with "Hg") as "(Hxs&Hg)". set_solver.
+    wp_apply (pstore_reroot_spec with "[Hr Hxs Hσ0]").
+    4:{ eapply path_restrict. done. }
+    2:done.
+    { destruct Hcoh as [_ X]. eapply locs_of_edges_weak; eauto. }
+    { eapply acyclic_weak; eauto using ti2. }
+    { iFrame. }
+
+    iIntros "[%ys (%Hundo&?&?&?)]".
+    assert (mirror xs ys) as Hmirror by eauto using undo_mirror.
+    iStep 8. do 2 iModIntro.
+    iApply "HΦ".
+    iDestruct (big_sepS_union_2 with "[$][$]") as "Hs".
+
+    remember ((rs, (l, v), r') :: bs) as xs.
+
+    iDestruct (extract_unaliased with "Hs") as "%".
+
+    assert (({[(rs, (l, v), r')]} ∪ list_to_set bs) = (list_to_set xs : gset _)) as Hbs.
+    { subst xs. reflexivity. }
+    rewrite Hbs. rewrite Hbs in H5.
+
+    iAssert ⌜forall x y, (rs,x,y) ∉ (list_to_set ys ∪ g ∖ list_to_set xs)⌝%I as "%".
+    { iIntros (???). destruct a. iDestruct (big_sepS_elem_of with "Hs") as "?". done.
+      iDestruct (pointsto_ne rs rs with "[$][$]") as "%". congruence. }
+
+    iExists _,_,_,_,M,_. iFrame.
+
+    assert (vertices (list_to_set ys ∪ g ∖ list_to_set xs) = vertices g) as Hvg.
+    { apply mirror_vertices in Hmirror.
+      rewrite vertices_union Hmirror -vertices_union -union_difference_L //. }
+
+    assert (σ1 = (apply_diffl (proj2 <$> xs) σ0)).
+    { destruct Hinv as [X1 X2 X3 X4]. eauto. }
+
+    assert (rooted_dag (list_to_set ys ∪ g ∖ list_to_set xs) rs) as Hroot.
+    { eapply undo_preserves_rooted_dag; eauto. }
+
+    iPureIntro. split_and !; try done.
+    { destruct Hinv as [X1 X2 X3 X4]. constructor.
+      { rewrite X1 Hvg.
+        apply elem_of_dom_2 in X3,HMrs.
+        apply path_ends_vertices in Hrs.
+        set_solver. }
+      { subst xs. set_solver. }
+      { set_solver. }
+      { intros. eapply undo_preserves_model; eauto. rewrite comm_L //. }
+    } {
+      rewrite /apply_diffl.
+      replace (<[l:=v]> (foldr (λ '(l0, v0) σ2, <[l0:=v0]> σ2) σ0 (list_fmap (loc * diff * loc)%type diff proj2 bs))) with (apply_diffl (proj2 <$> xs) σ0).
+      2:{ subst xs. reflexivity. }
+
+      destruct Hcoh as [X1 X2]. constructor.
+      { intros ???. rewrite dom_apply_diffl. apply X1 in H8.
+        eapply use_locs_of_edges_in in Hrs. 2:done.
+        set_solver.
+      } {
+        rewrite dom_apply_diffl. intros ???? Hedge.
+        rewrite /edge elem_of_union in Hedge. rewrite elem_of_union.
+        destruct Hedge as [Hedge|Hedge].
+        { right. eauto using undo_same_fst_label. }
+        { left. eapply (X2 r0). eapply elem_of_subseteq. 2:done. set_solver. }
+      }
+    }
+  Qed.
 End pstore_G.
 
 #[global] Opaque pstore_create.
 #[global] Opaque pstore_ref.
 #[global] Opaque pstore_get.
 #[global] Opaque pstore_set.
+#[global] Opaque pstore_capture.
+#[global] Opaque pstore_restore.
 
-#[global] Opaque pstore_inv.
-#[global] Opaque pstore_model.
+#[global] Opaque pstore.
+#[global] Opaque pstore_snapshot.
