theories/persistent/pstore_2.v
@@ -2,8 +2,8 @@
    https://gitlab.com/basile.clement/store/-/blob/main/src/store.ml?ref_type=heads
 *)
 
-From iris.algebra Require Import
-  gmap.
+From iris.base_logic Require Import
+  lib.ghost_map.
 
 From zebre Require Import
   prelude.
@@ -15,21 +15,42 @@ From zebre.language Require Import
 From zebre.std Require Import
   assert
   lst.
-From zebre.persistent Require Export
-  base.
 From zebre Require Import
   options.
 
-Implicit Types l : loc.
+Implicit Types l r node cnode base root dst : loc.
+Implicit Types nodes : list loc.
 Implicit Types v t s : val.
 Implicit Types σ : gmap loc val.
+
+#[local] Notation "'gen'" := (
+  in_type "t" 0
+)(in custom zebre_field
+).
+#[local] Notation "'root'" := (
+  in_type "t" 1
+)(in custom zebre_field
+).
+
+#[local] Notation "'ref_gen'" := (
+  in_type "ref" 0
+)(in custom zebre_field
+).
+#[local] Notation "'ref_value'" := (
+  in_type "ref" 1
+)(in custom zebre_field
+).
 
 #[local] Notation "'snap_store'" := (
   in_type "snap" 0
 )(in custom zebre_proj
 ).
-#[local] Notation "'snap_root'" := (
+#[local] Notation "'snap_gen'" := (
   in_type "snap" 1
+)(in custom zebre_proj
+).
+#[local] Notation "'snap_root'" := (
+  in_type "snap" 2
 )(in custom zebre_proj
 ).
 
@@ -42,60 +63,58 @@ Implicit Types σ : gmap loc val.
 )(in custom zebre_tag
 ).
 
-(* ------------------------------------------------------------------------ *)
-(* Code. *)
-
 Definition pstore_create : val :=
   λ: <>,
-    ref (ref §Root).
+    { #0; ref §Root }.
 
 Definition pstore_ref : val :=
-  λ: "v",
-    ref "v".
+  λ: "t" "v",
+    { #0; "v" }.
 
 Definition pstore_get : val :=
   λ: "t" "r",
-    !"r".
+    "r".{ref_value}.
 
 Definition pstore_set : val :=
   λ: "t" "r" "v",
-    let: "root" := ref §Root in
-    !"t" <- ‘Diff{ "r", !"r", "root" } ;;
-    "r" <- "v" ;;
-    "t" <- "root".
+    let: "g_t" := "t".{gen} in
+    let: "g_r" := "r".{ref_gen} in
+    if: "g_t" = "g_r" then (
+      "r" <-{ref_value} "v"
+    ) else (
+      let: "root" := ref §Root in
+      "t".{root} <- ‘Diff{ "r", "g_r", "r".{ref_value}, "root" } ;;
+      "r" <-{ref_gen} "g_t" ;;
+      "r" <-{ref_value} "v" ;;
+      "t" <-{root} "root"
+    ).
 
 Definition pstore_capture : val :=
   λ: "t",
-    ("t", !"t").
+    let: "g" := "t".{gen} in
+    "t" <-{gen} #1 + "g" ;;
+    ("t", "g", "t".{root}).
 
-Definition pstore_collect : val :=
-  rec: "pstore_collect" "node" "acc" :=
+#[local] Definition pstore_reroot_aux : val :=
+  rec: "pstore_reroot_aux" "node" :=
     match: !"node" with
     | Root =>
-        ("node", "acc")
-    | Diff <> <> "node'" =>
-        "pstore_collect" "node'" ‘Cons{ "node", "acc" }
+        ()
+    | Diff "r" "v" "gen" "node'" =>
+        "pstore_reroot_opt_aux" "node'" ;;
+        "node'" <- ‘Diff{ "r", "r".{ref_gen}, "r".{ref_value}, "node" } ;;
+        "r" <-{ref_gen} "gen" ;;
+        "r" <-{ref_value} "v"
     end.
-Definition pstore_revert : val :=
-  rec: "pstore_revert" "node" "seg" :=
-    match: "seg" with
-    | Nil =>
-        "node" <- §Root
-    | Cons "node'" "seg" =>
-        match: !"node'" with
-        | Root =>
-            Fail
-        | Diff "r" "v" "node_" =>
-            assert ("node_" = "node") ;;
-            "node" <- ‘Diff{ "r", !"r", "node'" } ;;
-            "r" <- "v" ;;
-            "pstore_revert" "node'" "seg"
-        end
-    end.
-Definition pstore_reroot : val :=
+#[local] Definition pstore_reroot : val :=
   λ: "node",
-    let: "root", "nodes" := pstore_collect "node" §Nil in
-    pstore_revert "root" "nodes".
+    match: !"node" with
+    | Root =>
+        ()
+    | Diff <> <> <> <> =>
+        pstore_reroot_aux "node" ;;
+        "node" <- §Root
+    end.
 
 Definition pstore_restore : val :=
   λ: "t" "s",
@@ -106,549 +125,623 @@ Definition pstore_restore : val :=
       match: !"root" with
       | Root =>
           ()
-      | Diff <> <> <> =>
+      | Diff <> <> <> <> =>
           pstore_reroot "root" ;;
-          "t" <- "root"
+          "t" <-{gen} #1 + "s".<snap_gen> ;;
+          "t" <-{root} "root"
       end
     ).
 
-(* ------------------------------------------------------------------------ *)
-(* Lemmas on maps and lists. *)
+Module raw.
+  #[local] Definition generation :=
+    nat.
+  Implicit Types g : generation.
 
-Section map.
-  Context `{Countable K}.
-  Context {V : Type}.
+  #[local] Definition store :=
+    gmap loc (generation * val).
+  Implicit Types ς : store.
+  Implicit Types data : generation * val.
 
-  Lemma gmap_included_insert (σ1 σ2:gmap K V) (l:K) (v:V) :
-    σ1 ⊆ σ2 ->
-    <[l:=v]>σ1 ⊆ <[l:=v]>σ2.
+  #[local] Definition descriptor : Set :=
+    generation * store.
+  Implicit Types descr : descriptor.
+  Implicit Types descrs : gmap loc descriptor.
+
+  Class PstoreG Σ `{zebre_G : !ZebreG Σ} := {
+    #[local] pstore_G_nodes_G :: ghost_mapG Σ loc descriptor ;
+  }.
+
+  Definition pstore_Σ := #[
+    ghost_mapΣ loc descriptor
+  ].
+  #[global] Instance subG_pstore_Σ Σ `{zebre_G : !ZebreG Σ} :
+    subG pstore_Σ Σ →
+    PstoreG Σ.
   Proof.
-    intros ? l'. destruct_decide (decide (l=l')).
-    { subst. rewrite !lookup_insert //. }
-    { rewrite !lookup_insert_ne //. }
+    solve_inG.
   Qed.
 
-  Lemma gmap_included_insert_notin (σ1 σ2:gmap K V) (l:K) (v:V) :
-    l ∉ dom σ1 ->
-    σ1 ⊆ σ2 ->
-    σ1 ⊆ <[l:=v]>σ2.
-  Proof.
-    intros ?? l'. destruct_decide (decide (l=l')).
-    { subst. rewrite lookup_insert // not_elem_of_dom_1 //. }
-    { rewrite !lookup_insert_ne //. }
-  Qed.
+  Section pstore_G.
+    Context `{pstore_G : PstoreG Σ}.
 
-  Lemma incl_dom_incl (σ1 σ2:gmap K V)  :
-    σ1 ⊆ σ2 ->
-    dom σ1 ⊆ dom σ2.
-  Proof.
-    intros X1.
-    intros l Hl. apply elem_of_dom in Hl. destruct Hl as (?&Hl).
-    eapply map_subseteq_spec in X1; last done. by eapply elem_of_dom.
-  Qed.
-End map.
+    #[local] Definition store_on σ0 ς :=
+      ς ∪ (pair 0 <$> σ0).
+    #[local] Definition store_generation g ς :=
+      map_Forall (λ r data, data.1 ≤ g) ς.
 
-Section list.
-  Context {A : Type}.
+    #[local] Definition descriptor_wf σ0 descr :=
+      dom descr.2 ⊆ dom σ0 ∧
+      store_generation descr.1 descr.2.
 
-  Lemma list_case_r (l:list A) :
-    l = nil \/ exists (l':list A) x, l = l' ++ [x].
-  Proof.
-    induction l using rev_ind.
-    naive_solver. right.
-    destruct IHl as [-> | (?&?&->)]; eauto.
-  Qed.
+    #[local] Definition delta : Set :=
+      loc * (generation * val).
+    Implicit Types δ : delta.
+    Implicit Types δs : list delta.
 
-  Lemma elem_of_middle (x:A) (xs:list A) :
-    x ∈ xs ->
-    exists (l1 l2:list A), xs = l1 ++ x::l2.
-  Proof.
-    intros Hx. apply elem_of_list_lookup_1 in Hx.
-    destruct Hx as (?&?).
-    eexists _,_. symmetry. eapply take_drop_middle. done.
-  Qed.
-End list.
+    #[local] Definition deltas_apply δs ς :=
+      list_to_map δs ∪ ς.
+    #[local] Fixpoint deltas_chain node nodes δs dst : iProp Σ :=
+      match nodes, δs with
+      | [], [] =>
+          ⌜node = dst⌝
+      | node' :: nodes, δ :: δs =>
+          node ↦ ’Diff{ #δ.1, #δ.2.1, δ.2.2, #node' } ∗
+          deltas_chain node' nodes δs dst
+      | _, _ =>
+          False
+      end.
 
-(* ------------------------------------------------------------------------ *)
-(* Define a labeled graph as a set of edges. *)
+    #[local] Definition edge : Set :=
+      loc * (list loc * list delta).
+    Implicit Types edg : edge.
+    Implicit Types edgs : gmap loc edge.
 
-Section graph.
-  Definition graph (A B : Type) `{Countable A} `{Countable B} :=
-    gset (A * B * A).
+    #[local] Definition descriptors_auth γ descrs :=
+      ghost_map_auth γ 1 descrs.
+    #[local] Definition descriptors_elem γ cnode descr :=
+      ghost_map_elem γ cnode DfracDiscarded descr.
 
-  Context `{Countable A} `{Countable B}.
-  Definition vertices (g:graph A B) : gset A :=
-    set_fold (fun '(x,_,y) acc => {[x;y]} ∪ acc) ∅ g.
+    #[local] Definition cnode_model is_base γ σ0 cnode descr edg ς : iProp Σ :=
+      let node := edg.1 in
+      let nodes := edg.2.1 in
+      let δs := edg.2.2 in
+      ⌜descriptor_wf σ0 descr⌝ ∗
+      descriptors_elem γ cnode descr ∗
+      ⌜NoDup δs.*1⌝ ∗
+      ⌜ if is_base is Some g then
+          Forall (λ δ, ∃ data, ς !! δ.1 = Some data ∧ data.1 = g) δs
+        else
+          0 < length δs
+      ⌝ ∗
+      ⌜store_on σ0 descr.2 = store_on σ0 $ deltas_apply δs ς⌝ ∗
+      deltas_chain cnode nodes δs node.
+    Definition pstore_model t σ0 σ : iProp Σ :=
+      ∃ l γ g root ς,
+      ⌜t = #l⌝ ∗
+      ⌜σ = snd <$> ς⌝ ∗
+      meta l (nroot.@"impl") γ ∗
+      l.[gen] ↦ #g ∗
+      l.[root] ↦ #root ∗
+      root ↦ §Root ∗
+      ( [∗ map] r ↦ data ∈ store_on σ0 ς,
+        r.[ref_gen] ↦ #data.1 ∗
+        r.[ref_value] ↦ data.2
+      ) ∗
+      ⌜descriptor_wf σ0 (g, ς)⌝ ∗
+      if decide (g = 0) then
+        descriptors_auth γ ∅
+      else
+        ∃ descrs edgs base descr nodes δs,
+        descriptors_auth γ descrs ∗
+        (* base cnode *)
+        ⌜descrs !! base = Some descr⌝ ∗
+        ⌜descr.1 < g⌝ ∗
+        cnode_model (Some g) γ σ0 base descr (root, (nodes, δs)) ς ∗
+        (* other cnodes *)
+        ( [∗ map] cnode ↦ descr; edg ∈ delete base descrs; edgs,
+          ∃ descr',
+          ⌜descrs !! edg.1 = Some descr'⌝ ∗
+          cnode_model None γ σ0 cnode descr edg descr'.2
+        ).
 
-  Lemma vertices_empty :
-    vertices ∅ = ∅.
-  Proof.
-    compute_done.
-  Qed.
+    Definition pstore_snapshot_model s t σ : iProp Σ :=
+      ∃ l γ g node descr,
+      ⌜t = #l ∧ s = (t, #g, #node)%V⌝ ∗
+      meta l (nroot.@"impl") γ ∗
+      descriptors_elem γ node descr ∗
+      ⌜descr.1 ≤ g⌝.
 
-  Definition proj1 {A B C:Type} (x:(A*B*C)) : A :=
-    match x with (x,_,_) => x end.
-  Definition proj2 {A B C:Type} (x:(A*B*C)) : B :=
-    match x with (_,x,_) => x end.
-  Definition proj3 {A B C:Type} (x:(A*B*C)) : C :=
-    match x with (_,_,x) => x end.
+    #[global] Instance pstore_model_timeless t σ0 σ :
+      Timeless (pstore_model t σ0 σ).
+    Proof.
+    Admitted.
+    #[global] Instance pstore_snapshot_persistent s t σ :
+      Persistent (pstore_snapshot_model s t σ).
+    Proof.
+      apply _.
+    Qed.
 
-  Lemma elem_of_vertices x (g:graph A B) :
-    x ∈ vertices g <-> exists b y, ((x,b,y) ∈ g \/ (y,b,x) ∈ g).
-  Proof.
-    apply set_fold_ind_L with (P := fun f g => x ∈ f  <-> exists b y, ((x,b,y) ∈ g \/ (y,b,x) ∈ g)).
-    set_solver.
-    intros ((?,?),?). set_solver.
-  Qed.
+    #[local] Lemma store_on_dom σ0 ς :
+      dom (store_on σ0 ς) = dom σ0 ∪ dom ς.
+    Proof.
+      set_solver.
+    Qed.
+    #[local] Lemma store_on_dom' σ0 ς :
+      dom ς ⊆ dom σ0 →
+      dom (store_on σ0 ς) = dom σ0.
+    Proof.
+      set_solver.
+    Qed.
+    #[local] Lemma store_on_lookup {σ0 ς} r data :
+      store_on σ0 ς !! r = Some data ↔
+          ς !! r = Some data
+        ∨ ς !! r = None ∧
+          data.1 = 0 ∧
+          σ0 !! r = Some data.2.
+    Proof.
+      destruct data as (g, v).
+      rewrite lookup_union_Some_raw lookup_fmap_Some. naive_solver.
+    Qed.
+    #[local] Lemma store_on_lookup' {σ0 ς} r data :
+      ς !! r = Some data →
+      store_on σ0 ς !! r = Some data.
+    Proof.
+      apply lookup_union_Some_l.
+    Qed.
+    #[local] Lemma store_on_insert r data σ0 ς :
+      store_on σ0 (<[r := data]> ς) = <[r := data]> (store_on σ0 ς).
+    Proof.
+      rewrite insert_union_l //.
+    Qed.
+    #[local] Lemma store_on_insert_support r v σ0 ς :
+      σ0 !! r = None →
+      dom ς ⊆ dom σ0 →
+      store_on (<[r := v]> σ0) ς = <[r := (0, v)]> (store_on σ0 ς).
+    Proof.
+      intros Hr%not_elem_of_dom Hς_dom.
+      assert (ς !! r = None).
+      { apply not_elem_of_dom. set_solver. }
+      rewrite insert_union_r // -fmap_insert //.
+    Qed.
 
-  Lemma vertices_singleton (x:(A*B*A)) :
-    vertices {[x]} = {[proj1 x; proj3 x]}.
-  Proof.
-    rewrite /vertices set_fold_singleton. destruct x as ((?&?)&?); set_solver.
-  Qed.
+    #[local] Lemma deltas_apply_nil ς :
+      deltas_apply [] ς = ς.
+    Proof.
+      rewrite /deltas_apply list_to_map_nil left_id //.
+    Qed.
+    #[local] Lemma deltas_apply_cons δ δs ς :
+      deltas_apply (δ :: δs) ς = <[δ.1 := δ.2]> (deltas_apply δs ς).
+    Proof.
+      destruct δ as (r, data).
+      rewrite /deltas_apply list_to_map_cons insert_union_l //.
+    Qed.
+    #[local] Lemma deltas_apply_singleton δ ς :
+      deltas_apply [δ] ς = <[δ.1 := δ.2]> ς.
+    Proof.
+      rewrite deltas_apply_cons deltas_apply_nil //.
+    Qed.
+    #[local] Lemma deltas_apply_app δs1 δs2 ς :
+      deltas_apply (δs1 ++ δs2) ς = deltas_apply δs1 (deltas_apply δs2 ς).
+    Proof.
+      rewrite /deltas_apply list_to_map_app assoc //.
+    Qed.
+    #[local] Lemma deltas_apply_snoc δs δ ς :
+      deltas_apply (δs ++ [δ]) ς = deltas_apply δs (<[δ.1 := δ.2]> ς).
+    Proof.
+      rewrite deltas_apply_app deltas_apply_singleton //.
+    Qed.
+    #[local] Lemma deltas_apply_snoc' δs r data ς :
+      deltas_apply (δs ++ [(r, data)]) ς = deltas_apply δs (<[r := data]> ς).
+    Proof.
+      apply (deltas_apply_snoc _ (r, data)).
+    Qed.
+    #[local] Lemma deltas_apply_dom δs ς :
+      dom (deltas_apply δs ς) = list_to_set δs.*1 ∪ dom ς.
+    Proof.
+      rewrite dom_union_L. f_equal. apply dom_list_to_map_L.
+    Qed.
+    #[local] Lemma deltas_apply_lookup r data δs ς :
+      NoDup δs.*1 →
+      (r, data) ∈ δs →
+      deltas_apply δs ς !! r = Some data.
+    Proof.
+      intros Hδs_nodup Hδ.
+      apply lookup_union_Some_l, elem_of_list_to_map_1; done.
+    Qed.
+    #[local] Lemma deltas_apply_lookup_ne r δs ς :
+      NoDup δs.*1 →
+      r ∉ δs.*1 →
+      deltas_apply δs ς !! r = ς !! r.
+    Proof.
+      intros Hδs_nodup Hr.
+      apply lookup_union_r, not_elem_of_list_to_map_1. done.
+    Qed.
+    #[local] Lemma deltas_apply_permutation {δs1} δs2 ς :
+      NoDup δs1.*1 →
+      δs1 ≡ₚ δs2 →
+      deltas_apply δs1 ς = deltas_apply δs2 ς.
+    Proof.
+      intros. rewrite /deltas_apply (list_to_map_proper _ δs2) //.
+    Qed.
 
-  Lemma vertices_union (g1 g2:graph A B) :
-    vertices (g1 ∪ g2) = vertices g1 ∪ vertices g2.
-  Proof.
-    revert g2. induction g1 using set_ind_L; intros g2.
-    { rewrite /vertices set_fold_empty !left_id_L //. }
-    replace ({[x]} ∪ X ∪ g2) with (X ∪ ({[x]} ∪ g2)) by set_solver.
-    rewrite (union_comm_L _  X).
-    rewrite !IHg1. rewrite -union_assoc_L. f_equal.
-    destruct_decide (decide (x ∈ g2)).
-    { replace ({[x]} ∪ g2) with g2 by set_solver.
-      rewrite vertices_singleton.
-      assert ({[proj1 x; proj3 x]} ⊆ vertices g2); last by set_solver.
-      intros l Hl. apply elem_of_vertices.
-      rewrite elem_of_union !elem_of_singleton in Hl. destruct x as ((?,?),?). set_solver. }
-    rewrite {1}/vertices /set_fold. simpl.
-    rewrite (foldr_permutation _ _ _ _ (x::elements g2)).
-    { intros. destruct a1 as ((?,?),?),a2 as ((?,?),?); set_solver. }
-    { by apply elements_union_singleton. }
-    { simpl. rewrite vertices_singleton. destruct x as ((?,?),?). set_solver. }
-  Qed.
+    #[local] Lemma deltas_chain_nil_inv node nodes dst :
+      deltas_chain node nodes [] dst ⊢
+      ⌜nodes = [] ∧ node = dst⌝.
+    Proof.
+      destruct nodes; iSteps.
+    Qed.
+    #[local] Lemma deltas_chain_cons_inv node nodes δ δs dst :
+      deltas_chain node nodes (δ :: δs) dst ⊢
+        ∃ node' nodes',
+        ⌜nodes = node' :: nodes'⌝ ∗
+        node ↦ ’Diff{ #δ.1, #δ.2.1, δ.2.2, #node' } ∗
+        deltas_chain node' nodes' δs dst.
+    Proof.
+      destruct nodes; iSteps.
+    Qed.
+    #[local] Lemma deltas_chain_snoc {node nodes δs dst} r g v dst' :
+      deltas_chain node nodes δs dst -∗
+      dst ↦ ’Diff{ #r, #g, v, #dst' } -∗
+      deltas_chain node (nodes ++ [dst']) (δs ++ [(r, (g, v))]) dst'.
+    Proof.
+      iInduction nodes as [] "IH" forall (node δs); destruct δs; iSteps.
+    Qed.
 
-  Definition edge (g:graph A B) x c y :=
-    (x,c,y) ∈ g.
+    #[local] Definition descriptors_alloc root :
+      ⊢ |==>
+        ∃ γ,
+        descriptors_auth γ ∅.
+    Proof.
+      iMod ghost_map_alloc as "(%γ & Hauth & _)".
+      iSteps.
+    Qed.
+    #[local] Lemma descriptors_insert {γ descrs} cnode descr :
+      descrs !! cnode = None →
+      descriptors_auth γ descrs ⊢ |==>
+        descriptors_auth γ (<[cnode := descr]> descrs) ∗
+        descriptors_elem γ cnode descr.
+    Proof.
+      iIntros "%Hdescrs_lookup Hauth".
+      iMod (ghost_map_insert with "Hauth") as "($ & Helem)"; first done.
+      iApply (ghost_map_elem_persist with "Helem").
+    Qed.
 
-  Inductive path (g:graph A B) : A -> list (A*B*A) -> A -> Prop :=
-  | path_nil : forall a, path g a [] a
-  | path_cons : forall a1 b a2 bs a3,
-      (a1,b,a2) ∈ g ->
-      path g a2 bs a3 ->
-      path g a1 ((a1,b,a2)::bs) a3.
+    Lemma pstore_model_valid t σ0 σ :
+      pstore_model t σ0 σ ⊢
+      ⌜dom σ ⊆ dom σ0⌝.
+    Proof.
+      iIntros "(%l & %γ & %g & %root & %ς & -> & -> & #Hmeta & Hl_gen & Hl_root & Hroot & Hς & (%Hς_dom & %Hς_gen) & _)".
+      rewrite dom_fmap //.
+    Qed.
 
-  Lemma path_app_inv g a1 a2 xs ys :
-    path g a1 (xs ++ ys) a2 ->
-    exists a, path g a1 xs a /\ path g a ys a2.
-  Proof.
-    revert a1 ys a2. induction xs as [| ((?,?),?)].
-    { eauto using path_nil. }
-    { intros. rewrite -app_comm_cons in H1. inversion H1. subst.
-      apply IHxs in H9. destruct H9 as (?&?&?).
-      eauto using path_cons. }
-  Qed.
+    Lemma pstore_create_spec :
+      {{{ True }}}
+        pstore_create ()
+      {{{ t,
+        RET t;
+        (∃ l, ⌜t = #l⌝ ∗ meta_token l (↑nroot.@"user")) ∗
+        pstore_model t ∅ ∅
+      }}}.
+    Proof.
+      iIntros "%Φ _ HΦ".
+      wp_rec.
+      wp_alloc root as "Hroot".
+      wp_record l as "Hmeta" "(Hl_gen & Hl_root & _)".
+      iMod (descriptors_alloc root) as "(%γ & Hauth)".
+      iDestruct (meta_token_difference _ (↑nroot.@"user") with "Hmeta") as "(Hmeta_user & Hmeta)"; first done.
+      iDestruct (meta_token_difference _ (↑nroot.@"impl") with "Hmeta") as "(Hmeta & _)"; first solve_ndisj.
+      iMod (meta_set with "Hmeta") as "Hmeta"; first done.
+      iApply "HΦ".
+      iStep. iExists l, γ, 0, root, ∅. iFrame. rewrite big_sepM_empty. iSteps.
+    Qed.
 
-  Lemma path_snoc_inv g a1 a2 a3 a4 b xs :
-    path g a1 (xs ++ [(a2,b,a3)]) a4 ->
-    path g a1 xs a2 /\ a3 = a4 /\ (a2,b,a3) ∈ g.
-  Proof.
-    intros Hpath. apply path_app_inv in Hpath. destruct Hpath as (?&?&Hpath).
-    inversion Hpath. subst. inversion H9. naive_solver.
-  Qed.
+    Lemma pstore_ref_spec t σ0 σ v :
+      {{{
+        pstore_model t σ0 σ
+      }}}
+        pstore_ref t v
+      {{{ r,
+        RET #r;
+        ⌜σ0 !! r = None⌝ ∗
+        pstore_model t (<[r := v]> σ0) σ
+      }}}.
+    Proof.
+      iIntros "%Φ (%l & %γ & %g & %root & %ς & -> & -> & #Hmeta & Hl_gen & Hl_root & Hroot & Hς & (%Hς_dom & %Hς_gen) & Hmodel) HΦ".
+      wp_rec. wp_record r as "(Hr_gen & Hr_value & _)".
+      iAssert ⌜σ0 !! r = None⌝%I as %Hr.
+      { rewrite -not_elem_of_dom. iIntros "%Hr".
+        iDestruct (big_sepM_lookup with "Hς") as "(_Hr_gen & _)".
+        { apply lookup_lookup_total_dom. rewrite store_on_dom' //. }
+        iDestruct (pointsto_ne with "Hr_gen _Hr_gen") as %?. done.
+      }
+      iApply "HΦ".
+      iSplitR; first iSteps. iExists l, γ, g, root, ς. iFrame "#∗". iStep 2.
+      iSplitL "Hς Hr_gen Hr_value".
+      { rewrite store_on_insert_support //.
+        iApply (big_sepM_insert_2 with "[Hr_gen Hr_value] Hς").
+        iSteps.
+      }
+      iSplitR. { iPureIntro. split; [set_solver | done]. }
+      case_decide as Hg; first iSteps.
+      iStep 3 as (descrs edgs base descr nodes δs Hdescrs_lookup_base Hgen (Hstore_dom & Hstore_gen) Hδs_nodup Hδs_gen Hδs) "Helem_base Hδs Hdescrs".
+      iExists edgs, nodes, δs. iSteps.
+      { iPureIntro. set_solver. }
+      { iPureIntro.
+        rewrite !store_on_insert_support //; last congruence.
+        apply (f_equal dom) in Hδs. set_solver.
+      } {
+        iClear "Helem_base". clear dependent descr nodes δs.
+        iApply (big_sepM2_impl with "Hdescrs"). iIntros "!> !>" (cnode descr (cnode' & (nodes & δs))) "%Hdescrs_lookup %Hedgs_lookup (%descr' & %Hdescrs_lookup' & ((%Hcnode_store_dom & %Hcnode_store_gen) & #Helem_cnode & %Hδs_nodup & %Hδs_length & %Hδs' & Hδs'))".
+        simpl in *.
+        iSteps; iPureIntro; first set_solver.
+        rewrite !store_on_insert_support //; last congruence.
+        apply (f_equal dom) in Hδs'. set_solver.
+      }
+    Qed.
 
-  Definition acyclic g := forall a xs, path g a xs a -> xs = nil.
+    Lemma pstore_get_spec {t σ0 σ r} v :
+      (σ ∪ σ0) !! r = Some v →
+      {{{
+        pstore_model t σ0 σ
+      }}}
+        pstore_get t #r
+      {{{
+        RET v;
+        pstore_model t σ0 σ
+      }}}.
+    Proof.
+      iIntros "%Hσ_lookup %Φ (%l & %γ & %g & %root & %ς & -> & -> & #Hmeta & Hl_gen & Hl_root & Hroot & Hς & (%Hς_dom & %Hς_gen) & Hmodel) HΦ".
+      wp_rec.
+      assert (∃ g_r, store_on σ0 ς !! r = Some (g_r, v)) as (g_r & Hς_lookup).
+      { setoid_rewrite store_on_lookup.
+        apply lookup_union_Some_raw in Hσ_lookup as [Hσ_lookup | (Hσ_lookup & Hσ0_lookup)].
+        - apply lookup_fmap_Some in Hσ_lookup as ((g_r & _v) & ? & Hς_lookup).
+          naive_solver.
+        - rewrite lookup_fmap fmap_None in Hσ_lookup.
+          naive_solver.
+      }
+      iDestruct (big_sepM_lookup_acc with "Hς") as "((Hr_gen & Hr_value) & Hς)"; first done.
+      wp_load.
+      iSteps.
+    Qed.
 
-  Record rooted_dag g (r:A) :=
-    { ti1 : forall a, a ∈ vertices g -> exists xs, path g a xs r;
-      ti2 : acyclic g
-    }.
+    Lemma pstore_set_spec t σ0 σ r v :
+      r ∈ dom σ0 →
+      {{{
+        pstore_model t σ0 σ
+      }}}
+        pstore_set t #r v
+      {{{
+        RET ();
+        pstore_model t σ0 (<[r := v]> σ)
+      }}}.
+    Proof.
+      iIntros "%Hr %Φ (%l & %γ & %g & %root & %ς & -> & -> & #Hmeta & Hl_gen & Hl_root & Hroot & Hς & (%Hς_dom & %Hς_gen) & Hmodel) HΦ".
+      pose proof Hr as (w0 & Hσ0_lookup)%elem_of_dom.
+      wp_rec. wp_load.
+      assert (∃ g_r w, store_on σ0 ς !! r = Some (g_r, w) ∧ g_r ≤ g) as (g_r & w & Hς_lookup & Hg_r).
+      { setoid_rewrite store_on_lookup.
+        destruct (ς !! r) as [(g_r, w) |] eqn:Hς_lookup.
+        - exists g_r, w. split; first naive_solver.
+          opose proof* map_Forall_lookup_1; done.
+        - exists 0, w0. split; first naive_solver. lia.
+      }
+      iDestruct (big_sepM_insert_acc with "Hς") as "((Hr_gen & Hr_value) & Hς)"; first done.
+      wp_load. wp_pures.
+      destruct (decide (g = 0)) as [-> | Hg].
+      - assert (g_r = 0) as -> by lia.
+        rewrite bool_decide_eq_true_2 //. wp_pures.
+        wp_store.
+        iDestruct ("Hς" $! (0, v) with "[$Hr_gen $Hr_value]") as "Hς".
+        iApply "HΦ".
+        iExists l, γ, 0, root, (<[r := (0, v)]> ς). iFrame "#∗". iStep.
+        iSplitR. { rewrite fmap_insert //. }
+        iSplitL. { rewrite insert_union_l //. }
+        iPureIntro. split; first set_solver. apply map_Forall_insert_2; done.
+      - destruct (decide (g = g_r)) as [<- | Hcase].
+        + rewrite bool_decide_eq_true_2 //.
+          wp_store.
+          iDestruct ("Hς" $! (g, v) with "[$Hr_gen $Hr_value]") as "Hς".
+          iApply "HΦ".
+          iExists l, γ, g, root, (<[r := (g, v)]> ς). iFrame "#∗". iStep.
+          iSplitR. { rewrite fmap_insert //. }
+          iSplitL "Hς". { rewrite insert_union_l //. }
+          iSplitR. { iPureIntro. split; first set_solver. apply map_Forall_insert_2; done. }
+          rewrite decide_False //.
+          iStep 3 as (descrs edgs base descr nodes δs Hdescrs_lookup_base Hgen (Hstore_dom & Hstore_gen) Hδs_nodup Hδs_gen Hδs) "Helem_base Hδs Hdescrs". iSteps; iPureIntro.
+          { eapply Forall_impl; first done. intros (r' & (g' & v')) H.
+            destruct (decide (r = r')) as [<- | Hr'].
+            - rewrite lookup_insert. naive_solver.
+            - rewrite lookup_insert_ne //.
+          } {
+            clear Hδs_gen. generalize dependent ς.
+            induction δs as [| (r' & (g' & v')) δs IH] using rev_ind.
+            all: intros ς Hς_dom Hς_gen Hς_lookup Hδs.
+            - exfalso.
+              rewrite deltas_apply_nil in Hδs.
+              rewrite -Hδs store_on_lookup in Hς_lookup.
+              destruct Hς_lookup as [Hstore_lookup |]; last naive_solver.
+              opose proof* (map_Forall_lookup_1 _ descr.2); [done.. |].
+              naive_solver lia.
+            - rewrite deltas_apply_snoc /=.
+              destruct (decide (r = r')) as [<- | Hr'].
+              + rewrite deltas_apply_snoc /= in Hδs.
+                rewrite insert_insert //.
+              + rewrite insert_commute //.
+                apply IH; simpl.
+                * rewrite fmap_app NoDup_app in Hδs_nodup. naive_solver.
+                * rewrite dom_insert union_subseteq singleton_subseteq_l.
+                  split; last done.
+                  apply (f_equal dom) in Hδs.
+                  rewrite store_on_dom' // store_on_dom in Hδs.
+                  rewrite Hδs deltas_apply_dom. set_solver.
+                * apply map_Forall_insert_2; last done.
+                  trans descr.1; last lia.
+                  assert (store_on σ0 descr.2 !! r' = Some (g', v')) as [Hstore_lookup | (_ & ? & _)]%store_on_lookup; last lia.
+                  { rewrite Hδs.
+                    apply store_on_lookup', deltas_apply_lookup; first done.
+                    set_solver.
+                  }
+                  eapply map_Forall_lookup_1 in Hstore_gen; done.
+                * rewrite /store_on -insert_union_l lookup_insert_ne //.
+                * rewrite deltas_apply_snoc // in Hδs.
+          }
+        + rewrite bool_decide_eq_false_2; first naive_solver. wp_pures.
+          wp_alloc root' as "Hroot'". do 2 wp_load. do 4 wp_store.
+          iDestruct ("Hς" $! (g, v) with "[$Hr_gen $Hr_value]") as "Hς".
+          iApply "HΦ".
+          iExists l, γ, g, root', (<[r := (g, v)]> ς). iFrame "#∗". iStep.
+          iSplitR. { rewrite fmap_insert //. }
+          iSplitL "Hς". { rewrite insert_union_l //. }
+          iSplitR. { iPureIntro. split; first set_solver. apply map_Forall_insert_2; done. }
+          rewrite decide_False //.
+          iStep 3 as (descrs edgs base descr nodes δs Hdescrs_lookup_base Hgen (Hstore_dom & Hstore_gen) Hδs_nodup Hδs_gen Hδs) "Helem_base Hδs Hdescrs".
+          assert (r ∉ δs.*1) as Hr_notin_δs.
+          { intros (i & ((? & data) & -> & Hδs_lookup)%list_lookup_fmap_inv)%elem_of_list_lookup.
+            opose proof* Forall_lookup_1 as H; [done.. |].
+            apply store_on_lookup in Hς_lookup. naive_solver.
+          }
+          assert (store_on σ0 descr.2 !! r = Some (g_r, w)) as Hstore_lookup.
+          { rewrite Hδs store_on_lookup deltas_apply_lookup_ne //.
+            rewrite store_on_lookup // in Hς_lookup.
+          }
+          iExists edgs, (nodes ++ [root']), (δs ++ [(r, (g_r, w))]). iFrame. iSteps; [iPureIntro.. |].
+          { rewrite fmap_app NoDup_app. split_and!; first done.
+            - set_solver.
+            - apply NoDup_singleton.
+          } {
+            rewrite Forall_app Forall_singleton. split.
+            - rewrite Forall_forall => δ Hδ. rewrite lookup_insert_ne.
+              { rewrite elem_of_list_fmap in Hr_notin_δs. naive_solver. }
+              rewrite Forall_forall in Hδs_gen. naive_solver.
+            - rewrite lookup_insert. naive_solver.
+          } {
+            rewrite deltas_apply_snoc insert_insert -deltas_apply_snoc'.
+            rewrite (deltas_apply_permutation ((r, (g_r, w)) :: δs)).
+            { rewrite fmap_app NoDup_app. split_and!; first done.
+              - set_solver.
+              - apply NoDup_singleton.
+            } {
+              solve_Permutation.
+            }
+            rewrite deltas_apply_cons store_on_insert -Hδs insert_id //.
+          } {
+            iApply (deltas_chain_snoc with "Hδs Hroot").
+          }
+    Qed.
 
-  Definition unaliased (g:graph A B) :=
-      forall r x1 r1 x2 r2,
-      (r,x1,r1) ∈ g ->
-      (r,x2,r2) ∈ g ->
-      x1 = x2 /\ r1 = r2.
+    Lemma pstore_capture_spec t σ0 σ :
+      {{{
+        pstore_model t σ0 σ
+      }}}
+        pstore_capture t
+      {{{ s,
+        RET s;
+        pstore_model t σ0 σ ∗
+        pstore_snapshot_model s t σ
+      }}}.
+    Proof.
+      iIntros "%Φ (%l & %γ & %g & %root & %ς & -> & -> & #Hmeta & Hl_gen & Hl_root & Hroot & Hς & (%Hς_dom & %Hς_gen) & Hmodel) HΦ".
+      wp_rec. wp_load. wp_store. wp_load. wp_pures.
+      iApply "HΦ".
+      case_decide as Hg; first subst.
+      - pose descr := (0, ς).
+        iMod (descriptors_insert root descr with "Hmodel") as "(Hauth & #Helem)"; first done.
+        iSplitL; last iSteps.
+        iExists l, γ, 1, root, ς. iFrame "#∗". iStep 2. iSplitR.
+        { iPureIntro. split; first set_solver.
+          eapply map_Forall_impl; first done. naive_solver.
+        }
+        iStep. iExists ∅, root, descr, [], []. iSplitR.
+        { iPureIntro. rewrite lookup_insert //. }
+        iSteps.
+        { rewrite NoDup_nil //. }
+        { rewrite deltas_apply_nil //. }
+        rewrite insert_empty delete_singleton.
+        iApply (big_sepM2_empty with "[//]").
+      - iDestruct "Hmodel" as "(%descrs & %edgs & %base & %descr & %nodes & %δs & Hauth & %Hdescrs_lookup_base & %Hgen & ((%Hstore_dom & %Hstore_gen) & #Helem_base & %Hδs_nodup & %Hδs_gen & %Hδs & Hδs) & Hdescrs)".
+        destruct δs as [| δ δs]; simpl.
+        + iDestruct (deltas_chain_nil_inv with "Hδs") as %(-> & <-).
+          iSplitL; iSteps.
+          { iPureIntro. eapply map_Forall_impl; first done. naive_solver lia. }
+          rewrite decide_False; first lia.
+          iSteps. iExists []. iSteps.
+        + iAssert ⌜edgs !! base = None⌝%I as %Hedgs_lookup_base.
+          { rewrite -eq_None_ne_Some. iIntros "%edg %Hedgs_lookup".
+            iDestruct (big_sepM2_lookup_r with "Hdescrs") as "(%descr' & %Hdescrs_lookup & _)"; first done.
+            rewrite lookup_delete // in Hdescrs_lookup.
+          }
+          iAssert ⌜descrs !! root = None⌝%I as %Hdescrs_lookup_root.
+          { destruct (decide (root = base)) as [-> | Hcase].
+            - iDestruct (deltas_chain_cons_inv with "Hδs") as "(%node & %nodes' & -> & Hbase & _)".
+              iDestruct (pointsto_ne with "Hroot Hbase") as %?. done.
+            - rewrite -eq_None_ne_Some. iIntros "%descr' %Hdescrs_lookup".
+              iDestruct (big_sepM2_lookup_l with "Hdescrs") as ((cnode' & (nodes' & δs'))) "(_ & %descr'' & _ & _ & _ & _ & %Hδs'_length & _ & Hδs') /=".
+              { rewrite lookup_delete_Some //. }
+              destruct δs' as [| δ' δs']; first naive_solver lia.
+              iDestruct (deltas_chain_cons_inv with "Hδs'") as "(%node & %nodes'' & -> & _Hroot & _)".
+              iDestruct (pointsto_ne with "Hroot _Hroot") as %?. done.
+          }
+          pose root_descr := (g, ς).
+          iMod (descriptors_insert root root_descr with "Hauth") as "(Hauth & #Helem_root)"; first done.
+          iSplitL; last iSteps.
+          iExists l, γ, (S g), root, ς. iFrame "#∗". iSteps as (_ | _) "" | "".
+          { iPureIntro. eapply map_Forall_impl; first done. naive_solver. }
+          iExists root, root_descr. iSplitR.
+          { rewrite lookup_insert //. }
+          set edg := (root, (nodes, δ :: δs)).
+          iExists (<[base := edg]> edgs), [], []. iSteps.
+          { rewrite NoDup_nil //. }
+          { rewrite deltas_apply_nil //. }
+          rewrite delete_insert //.
+          iApply big_sepM2_delete_l; first done.
+          iExists edg. iSteps.
+          { rewrite lookup_insert //. }
+          iExists root_descr. iSteps.
+          { iPureIntro. rewrite lookup_insert //. }
+          rewrite delete_insert //.
+          iClear "Helem_base". clear dependent descr nodes δs.
+          iApply (big_sepM2_impl with "Hdescrs"). iIntros "!>" (cnode descr (cnode' & (nodes & δs))) "%Hdescrs_lookup %Hedgs_lookup_cnode (%descr' & %Hdescrs_lookup' & ((%Hcnode_store_dom & %Hcnode_store_gen) & #Helem_cnode & %Hδs_nodup & %Hδs_length & %Hδs' & Hδs'))".
+          simpl in *.
+          iExists descr'. iSteps.
+          rewrite lookup_insert_ne //. congruence.
+    Qed.
 
-  Lemma path_app (g:graph A B) x3 x1 xs ys x2 :
-    path g x1 xs x3 ->
-    path g x3 ys x2 ->
-    path g x1 (xs++ys) x2.
-  Proof.
-    intros Hp.
-    revert x2 ys. induction Hp. eauto.
-    intros. rewrite -app_comm_cons. apply path_cons. set_solver.
-    eauto.
-  Qed.
+    Lemma pstore_restore_spec t σ0 σ s σ' :
+      {{{
+        pstore_model t σ0 σ ∗
+        pstore_snapshot_model s t σ'
+      }}}
+        pstore_restore t s
+      {{{
+        RET ();
+        pstore_model t σ0 σ'
+      }}}.
+    Proof.
+    Admitted.
+  End pstore_G.
 
-  Definition all_uniq_path g :=
-    forall a1 a2 xs ys, path g a1 xs a2 -> path g a1 ys a2 -> xs = ys.
+  #[global] Opaque pstore_model.
+  #[global] Opaque pstore_snapshot_model.
+End raw.
 
-  Lemma rooted_tree_impl_acyclic_unaliased g r :
-    (forall a, a ∈ vertices g -> exists xs, path g a xs r) -> (* If every vertex can reach the root, *)
-    all_uniq_path g -> (* then the property of uniq path *)
-    acyclic g /\ unaliased g. (* implies acyclicity + unalising *)
-  Proof.
-    intros Hroot  Huniq. split.
-    { intros ?? Hpath.
-      assert (path g a (xs++xs) a) as Hloop.
-      { by eapply path_app. }
-      specialize (Huniq a a xs (xs++xs) Hpath Hloop).
-      apply (@f_equal _ _ length) in Huniq. rewrite app_length in Huniq.
-      assert (length xs = 0) by lia. destruct xs; simpl in *; try done; lia. }
-    { intros ????? X1 X2.
-      destruct (Hroot r1) as (xs1&Hxs1).
-      { eapply elem_of_vertices. eauto. }
-      destruct (Hroot r2) as (xs2&Hxs2).
-      { eapply elem_of_vertices. eauto. }
-      assert (path g r0 ((r0,x1,r1)::xs1) r) as Hp1. by eapply path_cons.
-      assert (path g r0 ((r0,x2,r2)::xs2) r) as Hp2. by eapply path_cons.
-      specialize (Huniq _ _ _ _ Hp1 Hp2). naive_solver. }
-  Qed.
-
-  Lemma acyclic_unaliased_impl_uniq_path g :
-    acyclic g ->
-    unaliased g ->
-    all_uniq_path g.
-  Proof.
-    intros Hacy Hinj. intros ???? Hpath.
-    revert ys. induction Hpath; intros ys.
-    { intros Hpath. apply Hacy in Hpath. done. }
-    { inversion 1; subst.
-      { exfalso.
-        assert (path g a3 ((a3, b, a2)::bs) a3) as Z.
-        { apply path_cons. done. eauto. }
-        apply Hacy in Z. congruence. }
-      destruct (Hinj _ _ _ _ _ H1 H3). subst.
-      f_equal. eapply IHHpath. done. }
-  Qed.
-
-  Lemma rooted_dag_empty (r:A) :
-      rooted_dag (∅ : graph A B) r.
-  Proof.
-    constructor.
-    { intros ?. rewrite vertices_empty. set_solver. }
-    { intros ??. inversion 1; set_solver. }
-  Qed.
-
-  Lemma path_cycle_end_inv_aux g (r r':A) b ds x1 x2 :
-    r ≠ r' ->
-    x2 ≠ r' ->
-    r' ∉ vertices g ->
-    path ({[(r, b, r')]} ∪ g) x1 ds x2 ->
-    path g x1 ds x2.
-  Proof.
-    induction 4.
-    { apply path_nil. }
-    { eapply path_cons.
-      { rewrite /edge elem_of_union elem_of_singleton in H4.
-        destruct H4 as [|]; last done.
-        inversion H4. subst. inversion H5. congruence. subst.
-        exfalso. apply H3. apply elem_of_vertices. set_solver. }
-      by eapply IHpath. }
-  Qed.
-
-  Lemma path_cycle_end_inv g (r r':A) b ds x :
-    r ≠ r' ->
-    r' ∉ vertices g ->
-    path ({[(r, b, r')]} ∪ g) x ds x ->
-    path g x ds x.
-  Proof.
-    intros.
-    destruct_decide (decide (x=r')).
-    { subst. inversion H3. apply path_nil. subst. exfalso. apply H2. apply elem_of_vertices. set_solver. }
-    eapply path_cycle_end_inv_aux; last done. all:done.
-  Qed.
-
-  Lemma path_snoc g a1 b a2 bs a3 :
-    path g a1 bs a2 ->
-    (a2,b,a3) ∈ g ->
-    path g a1 (bs++[(a2,b,a3)]) a3.
-  Proof.
-    induction 1.
-    { intros. apply path_cons. done. apply path_nil. }
-    { intros. rewrite -app_comm_cons. eauto using path_cons. }
-  Qed.
-
-  Lemma path_weak g1 g2 x bs y :
-    path g1 x bs y ->
-    g1 ⊆ g2 ->
-    path g2 x bs y.
-  Proof.
-    induction 1; intros Hi. apply path_nil. eapply path_cons.
-    by apply Hi. by apply IHpath.
-  Qed.
-
-  Lemma rooted_dag_add (r r':A) g x:
-    r ≠ r' ->
-    r' ∉ vertices g ->
-    rooted_dag g r ->
-    rooted_dag ({[(r, x, r')]} ∪ g) r'.
-  Proof.
-    intros Hne Hg Hroot. inversion Hroot as [X1 X2].
-    constructor.
-    { rewrite vertices_union vertices_singleton. intros a.
-      rewrite !elem_of_union !elem_of_singleton.
-      intros [[-> | ->] | Hx].
-      { exists [(r, x, r')]. simpl. eapply path_cons. set_solver. apply path_nil. }
-      { exists nil. apply path_nil. }
-      { apply X1 in Hx. destruct Hx as (ds,Hx). exists (ds++[(r, x, r')]).
-        eapply path_snoc.
-        { eapply path_weak; eauto. set_solver. }
-        { set_solver. } } }
-    { intros ?? Hpath. apply  path_cycle_end_inv in Hpath; eauto. }
-  Qed.
-
-  Lemma acyclic_weak (g1 g2:graph A B) :
-    acyclic g1 ->
-    g2 ⊆ g1 ->
-    acyclic g2.
-  Proof.
-    intros Hacy ? ???. eapply Hacy. by eapply path_weak.
-  Qed.
-
-  Lemma path_all_in (g:graph A B) a1 xs a2 :
-    path g a1 xs a2 ->
-    list_to_set xs ⊆ g.
-  Proof.
-    induction 1; simpl; set_solver.
-  Qed.
-
-  Lemma path_restrict (g:graph A B) r xs r' :
-    path g r xs r' ->
-    path (list_to_set xs) r xs r'.
-  Proof.
-    induction 1; eauto using path_nil.
-    apply path_cons. set_solver.
-    eapply path_weak. done. set_solver.
-  Qed.
-
-  Lemma path_inv_r (g:graph A B) x bs z :
-    path g x bs z ->
-    (x = z /\ bs = nil) ∨ ∃ bs' b y, bs = bs' ++ [(y,b,z)] /\ path g x bs' y ∧ (y,b,z) ∈ g.
-  Proof.
-    induction 1.
-    { naive_solver.  }
-    right. destruct IHpath as [(->&->)|(bs'&b'&y&->&?&?)].
-    { exists nil. eexists _,_. split; first done. split. eauto using path_nil. naive_solver. }
-    { exists ((a1, b, a2) :: bs'). eexists _,_. rewrite app_comm_cons //. split_and !; try done.
-      apply path_cons; eauto. }
-  Qed.
-
-  Lemma path_add_inv_r (r r':A) b x xs g :
-    r ≠ r' ->
-    r' ∉ vertices g ->
-    path ({[(r, b, r')]} ∪ g) x xs r' ->
-    (xs = nil /\ x = r') \/ (exists xs', xs = xs' ++ [(r, b, r')] /\ path g x xs' r).
-  Proof.
-    intros Hrr' Hr' Hreach. apply path_inv_r in Hreach.
-    destruct Hreach as [(->&->)|(bs'&b0&y&->&Hreach&Hedge)].
-    { eauto. }
-    right.
-    assert (b0=b /\ y=r) as (->&->).
-    { rewrite /edge elem_of_union elem_of_singleton in Hedge.
-      destruct Hedge. naive_solver. exfalso. apply Hr', elem_of_vertices. eauto. }
-    eexists. split; first done.
-    eauto using path_cycle_end_inv_aux.
-  Qed.
-
-  (* [mirror xs ys] asserts that, up-to labels, the path xs is the reverse of ys *)
-  Inductive mirror :
-    list (A*B*A) -> list (A*B*A) -> Prop :=
-  | mirror_nil :
-    mirror [] []
-  | mirror_cons :
-    forall r x x' r' xs ys,
-      mirror xs ys  ->
-      mirror (xs++[(r,x,r')]) ((r',x',r)::ys).
-
-  Lemma mirror_snoc ys xs a a' x x' :
-    mirror ys xs ->
-    mirror ((a,x,a') :: ys) (xs ++ [(a',x',a)]).
-  Proof.
-    induction 1.
-    { apply (mirror_cons _ _ _ _ nil nil). apply mirror_nil. }
-    rewrite -!app_comm_cons app_comm_cons. by apply mirror_cons.
-  Qed.
-
-  Lemma mirror_symm xs ys :
-    mirror xs ys -> mirror ys xs.
-  Proof.
-    induction 1. eauto using mirror_nil.
-    apply mirror_snoc; eauto.
-  Qed.
-
-  Lemma use_mirror xs ys (g:graph A B) r y :
-    mirror xs ys ->
-    path g r xs y ->
-    path (list_to_set ys) y ys r.
-  Proof.
-    intros Hu. revert r y. induction Hu; intros r0 y.
-    { inversion 1. subst. apply path_nil. }
-    intros Hp. apply path_snoc_inv in Hp. destruct Hp as (?&?&?). subst.
-    apply path_cons. set_solver. eapply path_weak. apply IHHu; eauto. set_solver.
-  Qed.
-
-  Lemma mirror_vertices (xs ys:list (A*B*A)) :
-    mirror xs ys ->
-    vertices (list_to_set ys) = vertices (list_to_set xs).
-  Proof.
-    revert xs. induction ys; intros xs; inversion 1; subst. done.
-    simpl. rewrite list_to_set_app_L !vertices_union !vertices_singleton. simpl.
-    erewrite IHys; last done. rewrite vertices_empty. set_solver.
-  Qed.
-
-  Lemma mirror_same_length (xs ys:list (A*B*A)):
-    mirror xs ys ->
-    length xs = length ys.
-  Proof. induction 1. done. rewrite app_length. simpl. lia. Qed.
-
-  Lemma mirror_mirrored_edges xs ys r x r' :
-    mirror xs ys ->
-    (r,x,r') ∈ xs -> exists x', (r',x',r) ∈ ys.
-  Proof.
-    induction 1. intros ?. set_solver.
-    rewrite elem_of_app elem_of_list_singleton.
-    intros [X|X].
-    { apply IHmirror in X. set_solver. }
-    { set_solver. }
-  Qed.
-
-  Lemma path_middle (g:graph A B) x xs ys z :
-    path g x (xs ++ ys) z ->
-    exists y, path g x xs y /\ path g y ys z.
-  Proof.
-    revert g x ys z. induction xs; intros g x ys z.
-    { simpl. eauto using path_nil. }
-    inversion 1; simpl in *; subst.
-    apply IHxs in H7. destruct H7 as (y,(?&?)).
-    exists y. split; last done. eauto using path_cons.
-  Qed.
-
-  Lemma use_mirror_subset xs ys xs' g r y :
-    xs' ⊆ xs ->
-    mirror xs ys ->
-    path g r xs' y ->
-    exists zs, path (list_to_set ys) y zs r /\ length xs' = length zs.
-  Proof.
-    intros Hincl Hundo Hpath.
-    induction Hpath.
-    { exists nil. split. apply path_nil. done. }
-    { destruct IHHpath as (zs&Hzs&?).
-      { set_solver. }
-      eapply (mirror_mirrored_edges _ _ a1 b a2) in Hundo. 2:set_solver.
-      destruct Hundo as (b'&?).
-      exists (zs ++ [(a2, b', a1)]). split.
-      { eapply path_app. done.
-        apply path_cons.  set_solver. apply path_nil. }
-      { rewrite app_length. simpl. lia. } }
-  Qed.
-
-  Definition pathlike (ys:list (A*B*A)) r :=
-    forall a b a', (a,b,a') ∈ ys -> a' = r \/ exists b' a'', (a',b',a'') ∈ ys.
-
-  Lemma path_pathlike g r ys y :
-    path g y ys r ->
-    pathlike ys r.
-  Proof.
-    intros Hpath a b a' Hedge.
-    apply elem_of_middle in Hedge. destruct Hedge as (?&?&->).
-    rewrite cons_middle assoc_L in Hpath.
-    apply path_app_inv in Hpath. destruct Hpath as (?&Hpath&Hp').
-    apply path_snoc_inv in Hpath. destruct Hpath as (?&?&?). subst.
-    inversion Hp'; set_solver.
-  Qed.
-
-  Lemma same_path g (xs:list (A*B*A)) a1 a2 a3 a4 :
-    path g a1 xs a2 ->
-    path g a3 xs a4 ->
-    xs ≠ nil ->
-    a1 = a3 /\ a2=a4.
-  Proof.
-    intros Hp1. revert a3 a4. induction Hp1.
-    { intros. congruence. }
-    intros a3' a4'. inversion 1. subst. intros _. destruct bs.
-    { inversion Hp1; inversion H10. subst. done. }
-    apply IHHp1 in H10. 2:done. naive_solver.
-  Qed.
-
-  Lemma path_ends_vertices g x1 xs x2 :
-    path g x1 xs x2 ->
-    (x1 = x2) \/ (x1 ∈ vertices g /\ x2 ∈ vertices g).
-  Proof.
-     inversion 1. eauto. subst. right.
-     split. apply elem_of_vertices. eauto.
-     apply path_inv_r in H3. destruct H3 as [(->&->)|(?&?&?&->&?&?)].
-     all:apply elem_of_vertices; eauto.
-  Qed.
-End graph.
-
-(* ------------------------------------------------------------------------ *)
-(* Define apply_diffl, a function applying a list of diff. *)
-
-Section adiffl.
-  Notation diff := (
-    (* loc and its old value *)
-    loc*val
-  )%type.
-
-  Definition apply_diffl (ds:list diff) (σ:gmap loc val) : gmap loc val :=
-    foldr (fun '(l,v) σ => <[l:=v]> σ) σ ds.
-
-  Lemma dom_apply_diffl ds σ :
-    dom (apply_diffl ds σ) = dom σ ∪ (list_to_set ds.*1).
-  Proof.
-    induction ds as [|(?&?)]; set_solver.
-  Qed.
-
-  Lemma apply_diffl_insert_ne ds l v σ :
-    l ∉ ds.*1 ->
-    apply_diffl ds (<[l:=v]> σ) = <[l:=v]> (apply_diffl ds σ).
-  Proof.
-    induction ds as [|(?&?)].
-    { intros ?. reflexivity. }
-    { intros. simpl. rewrite IHds. set_solver.
-      rewrite insert_commute //. set_solver. }
-  Qed.
-
-  Lemma apply_diffl_app ds ds' σ :
-    apply_diffl (ds++ds') σ = apply_diffl ds (apply_diffl ds' σ).
-  Proof.
-    rewrite /apply_diffl foldr_app //.
-  Qed.
-
-  Lemma apply_diffl_snoc xs l v σ :
-    apply_diffl (xs ++ [(l,v)]) σ = apply_diffl xs (<[l:=v]> σ).
-  Proof.
-    rewrite apply_diffl_app //.
-  Qed.
-
-  Lemma apply_diffl_cons l v xs σ :
-    apply_diffl ((l,v)::xs) σ = <[l:=v]> (apply_diffl xs σ).
-  Proof.
-    done.
-  Qed.
-
-  Lemma apply_diffl_included xs σ1 σ2 :
-    σ1 ⊆ σ2 ->
-    apply_diffl xs σ1 ⊆ apply_diffl xs σ2.
-  Proof.
-    revert σ1 σ2. induction xs as [|(?,?)]; intros;
-      [ done | eauto using gmap_included_insert ].
-  Qed.
-End adiffl.
-
-(* ------------------------------------------------------------------------ *)
-(* Proof. *)
+#[global] Opaque pstore_create.
+#[global] Opaque pstore_ref.
+#[global] Opaque pstore_get.
+#[global] Opaque pstore_set.
+#[global] Opaque pstore_capture.
+#[global] Opaque pstore_restore.
 
 Class PstoreG Σ `{zebre_G : !ZebreG Σ} := {
-  #[local] pstore_G_map_G :: MonoMapG Σ nat (loc * gmap loc val)%type ;
+  #[local] pstore_G_raw_G :: raw.PstoreG Σ ;
+  #[local] pstore_G_support_G :: MonoMapG Σ loc val ;
 }.
 
 Definition pstore_Σ := #[
-  mono_map_Σ nat (loc * gmap loc val)%type
+  raw.pstore_Σ ;
+  mono_map_Σ loc val
 ].
-#[global] Instance subG_pstore_Σ Σ `{zebre_G : !ZebreG Σ} :
+Lemma subG_pstore_Σ Σ `{zebre_G : !ZebreG Σ} :
   subG pstore_Σ Σ →
   PstoreG Σ.
 Proof.
@@ -658,88 +751,29 @@ Qed.
 Section pstore_G.
   Context `{pstore_G : PstoreG Σ}.
 
-  Notation diff := (
-    (* loc and its old value. *)
-    loc*val
-  )%type.
-  Notation graph_store := (
-    graph loc diff
-  ).
-  Notation map_model := (
-    gmap loc (gmap loc val)
-  ).
+  Definition pstore_model t σ : iProp Σ :=
+    ∃ l γ σ0 ς,
+    ⌜t = #l⌝ ∗
+    ⌜σ ⊆ ς ∪ σ0⌝ ∗
+    meta l (nroot.@"user") γ ∗
+    mono_map_auth γ σ0 ∗
+    raw.pstore_model t σ0 ς.
 
-  Definition correct_path_diff (M:map_model) (g:graph_store) :=
-    forall r1 ds r2 σ1 σ2,
-      path g r1 ds r2 -> M !! r1 = Some σ1 -> M !! r2 = Some σ2 ->
-      σ1 = (apply_diffl (proj2 <$> ds) σ2).
+  Definition pstore_snapshot_model s t σ : iProp Σ :=
+    ∃ l γ σ0 ς,
+    ⌜t = #l⌝ ∗
+    ⌜σ ⊆ ς ∪ σ0⌝ ∗
+    meta l (nroot.@"user") γ ∗
+    mono_map_lb γ σ0 ∗
+    raw.pstore_snapshot_model s t ς.
 
-  Record store_inv (M:map_model) (g:graph_store) (r:loc) (σ σ0:gmap loc val) :=
-    { si1 : dom M = vertices g ∪ {[r]};
-      si2 : σ ⊆ σ0;
-      si3 : M !! r = Some σ0 ;
-      si4 : correct_path_diff M g
-    }.
-
-  Definition locs_of_edges_in g (X:gset loc) :=
-    forall (r:loc) l v r', edge g r (l,v) r' -> l ∈ X.
-
-  Record coherent (M:map_model) (σ0:gmap loc val) (g:graph_store) :=
-    { coh1 : forall r σ, M !! r = Some σ -> dom σ = dom σ0;
-      coh2 : locs_of_edges_in g (dom σ0);
-    }.
-
-  Definition snap_inv (M:map_model) (C:gmap nat (loc * gmap loc val)) :=
-    forall n l σ, C !! n = Some (l,σ) -> exists σ', M !! l = Some σ' /\ σ ⊆ σ'.
-
-  #[local] Definition pstore_map_auth γ map :=
-    mono_map_auth γ map.
-  #[local] Definition pstore_map_elem γ n l σ :=
-    mono_map_elem γ n (l, σ).
-
-  Lemma extract_unaliased (g : graph_store) :
-    ([∗ set] '(r, (l, v), r') ∈ g, r ↦ ’Diff{ #(l : loc), v, #(r' : loc) }) -∗
-    ⌜unaliased g⌝.
-  Proof.
-    iIntros "Hg" (???????).
-    destruct_decide (decide (a0 = a2 ∧ a1 = a3)). done.
-    rewrite (big_sepS_delete _ _ (a, a0, a1)). set_solver.
-    rewrite (big_sepS_delete _ _ (a, a2, a3)). set_solver.
-    iDestruct "Hg" as "(?&?&_)". destruct a0,a2.
-    iDestruct (pointsto_ne with "[$][$]") as "%". congruence.
-  Qed.
-
-  (* NB our invariant asserts that g is indeed a rooted tree: a rooted DAG
-     with unicity of paths. Indeed, from the set of pointsto we can extract [unaliased],
-     (see [extract_unaliased]), and a DAG with unaliased guarantees unicity of paths
-     (see [acyclic_unaliased_impl_uniq_path] ) *)
-
-  #[local] Definition pstore (γ:gname) (t:val) (σ:gmap loc val) : iProp Σ :=
-    ∃ (t0 r:loc)
-      (σ0:gmap loc val) (* the global map, with all the points-to ever allocated *)
-      (g:graph_store) (* the global graph *)
-      (M:map_model) (* the map model, associating to each node its model *)
-      (C:gmap nat (loc * gmap loc val)), (* the model of snapshots *)
-    ⌜t=#t0 /\ store_inv M g r σ σ0 /\ coherent M σ0 g /\ rooted_dag g r /\ snap_inv M C⌝ ∗
-    t0 ↦ #r ∗
-    r ↦ §Root ∗
-    pstore_map_auth γ C ∗
-    ([∗ map] l ↦ v ∈ σ0, l ↦ v) ∗
-    ([∗ set] x ∈ g, let '(r,(l,v),r') := x in r ↦ ’Diff{ #(l : loc), v, #(r' : loc) }) .
-
-  Definition open_inv : string :=
-    "[%t0 [%r [%σ0 [%g [%M [%C ((->&%Hinv&%Hcoh&%Hgraph&%Hsnap)&Ht0&Hr&HC&Hσ0&Hg)]]]]]]".
-
-  Definition pstore_snapshot γ t s σ : iProp Σ :=
-    ∃ l n, ⌜s=ValTuple [t;#l]⌝ ∗ pstore_map_elem γ n l σ.
-
-  #[global] Instance pstore_snapshot_timeless γ t s σ :
-    Timeless (pstore_snapshot γ t s σ).
+  #[global] Instance pstore_model_timeless t σ :
+    Timeless (pstore_model t σ).
   Proof.
     apply _.
   Qed.
-  #[global] Instance pstore_snapshot_persistent γ t s σ :
-    Persistent (pstore_snapshot γ t s σ).
+  #[global] Instance pstore_snapshot_persistent s t σ :
+    Persistent (pstore_snapshot_model s t σ).
   Proof.
     apply _.
   Qed.
@@ -747,974 +781,118 @@ Section pstore_G.
   Lemma pstore_create_spec :
     {{{ True }}}
       pstore_create ()
-    {{{ t γ,
+    {{{ t,
       RET t;
-        pstore γ t ∅
+      pstore_model t ∅
     }}}.
   Proof.
     iIntros "%Φ _ HΦ".
-    wp_rec.
-    wp_alloc r as "Hroot".
-    wp_alloc t0 as "Ht0".
-    iMod (mono_map_alloc ∅) as "[%γ ?]".
-    iApply "HΦ". iModIntro.
-    iExists t0,r,∅,∅,{[r := ∅]},∅. iFrame.
-    rewrite !big_sepM_empty big_sepS_empty !right_id.
-    iPureIntro. split_and!; first done.
-    { constructor.
-      { rewrite dom_singleton_L vertices_empty //. set_solver. }
-      { set_solver. }
-      { rewrite lookup_insert //. }
-      { intros ????? Hr.
-        rewrite !lookup_singleton_Some.
-        inversion Hr; set_solver. } }
-    { constructor.
-      { intros ??. rewrite lookup_singleton_Some. intros (->&->). reflexivity. }
-      { intros ????. set_solver. } }
-    { eauto using rooted_dag_empty. }
-    { intros ??. set_solver. }
+    iApply wp_fupd.
+    wp_apply (raw.pstore_create_spec with "[//]") as (t) "((%l & -> & Hmeta) & Ht)".
+    iMod mono_map_alloc as "(%γ & Hauth)".
+    iMod (meta_set with "Hmeta") as "Hmeta"; first done.
+    iSteps. iExists ∅, ∅. iSteps.
   Qed.
 
-  Lemma use_locs_of_edges_in g r xs r' X :
-    locs_of_edges_in g X ->
-    path g r xs r' ->
-    (list_to_set (proj2 <$> xs).*1) ⊆ X.
-  Proof.
-    intros He.
-    induction 1. set_solver.
-    apply He in H. set_solver.
-  Qed.
-
-  Lemma pstore_ref_spec γ t σ v :
+  Lemma pstore_ref_spec t σ v :
     {{{
-      pstore γ t σ
+      pstore_model t σ
     }}}
-      pstore_ref v
-    {{{ l,
-      RET #l;
-      ⌜l ∉ dom σ⌝ ∗
-      pstore γ t (<[l := v]> σ)
+      pstore_ref t v
+    {{{ r,
+      RET #r;
+      ⌜σ !! r = None⌝ ∗
+      pstore_model t (<[r := v]> σ)
     }}}.
   Proof.
-    iIntros (ϕ) open_inv. iIntros "HΦ".
-
-    wp_rec. wp_alloc l as "Hl".
+    iIntros "%Φ (%l & %γ & %σ0 & %ς & -> & %Hσ & #Hmeta & Hauth & Ht) HΦ".
+    iDestruct (raw.pstore_model_valid with "Ht") as %Hς_dom.
+    iApply wp_fupd.
+    wp_apply (raw.pstore_ref_spec with "Ht") as (r) "(%Hσ0_lookup & Ht)".
+    assert (ς !! r = None) as Hς_lookup.
+    { rewrite -!not_elem_of_dom in Hσ0_lookup |- *. set_solver. }
+    assert (σ !! r = None) as Hσ_lookup.
+    { eapply lookup_weaken_None; last done. apply lookup_union_None_2; done. }
+    iMod (mono_map_insert with "Hauth") as "Hauth"; first done.
     iApply "HΦ".
-
-    iAssert ⌜σ0 !! l = None⌝%I as %Hl0.
-    { rewrite -not_elem_of_dom. iIntros (Hl).
-      apply elem_of_dom in Hl. destruct Hl.
-      iDestruct (big_sepM_lookup with "Hσ0") as "Hl_"; first done.
-      iDestruct (pointsto_ne with "Hl Hl_") as %?. done. }
-    assert (σ !! l = None).
-    { eapply not_elem_of_dom. apply not_elem_of_dom in Hl0.  destruct Hinv as [_ X].
-      apply incl_dom_incl in X. set_solver. }
-    iDestruct (pointsto_ne with "Hl Hr") as %Hlr.
-
-    iModIntro. iSplitR. iPureIntro. by eapply not_elem_of_dom.
-    iExists t0,r, (<[l:=v]>σ0),g,((fun σ => <[l:=v]>σ)<$> M),C.
-
-    rewrite big_sepM_insert //. iFrame.
-    iPureIntro. split_and !; eauto.
-    { destruct Hinv as [X1 X2 X3 X4].
-      constructor.
-      { rewrite dom_fmap_L; set_solver. }
-      { eauto using gmap_included_insert. }
-      { rewrite lookup_fmap X3 //. }
-      { intros r1 ds r2 σ1 σ2 Hr. rewrite !lookup_fmap. generalize Hr. intros Hreach.
-        intros Hr1 Hr2.
-        destruct (M !! r1) eqn:Hor1. 2:simpl in *; congruence.
-        inversion Hr1. subst.
-        destruct (M !! r2) eqn:Hor2. 2:simpl in *; congruence.
-        inversion Hr2. subst.
-        destruct Hcoh as [Z1 Z2].
-        eapply use_locs_of_edges_in in Z2. 2:done.
-        rewrite apply_diffl_insert_ne.
-        { apply not_elem_of_dom in Hl0. set_solver. }
-        { f_equal. eauto. } } }
-    { destruct Hcoh as [X1 X2].
-      constructor.
-      { intros r' ?. rewrite lookup_fmap. intros E.
-        destruct (M !! r') eqn:Hor. 2:simpl in *; congruence.
-        inversion E. subst. rewrite !dom_insert_L. set_solver. }
-      { intros. rewrite dom_insert_L. intros ??. set_solver. } }
-    { intros ? r' ? HC. apply Hsnap in HC. destruct HC as (x&Hx&?).
-      exists (<[l:=v]>x). rewrite lookup_fmap Hx. split. done.
-      apply gmap_included_insert_notin; last done.
-      apply incl_dom_incl in H0. intros X. apply H0 in X.
-      destruct Hcoh as [X1 X2]. apply X1 in Hx.
-      apply not_elem_of_dom in Hl0. set_solver. }
+    iStep. iExists l, γ, (<[r := v]> σ0), ς. iSteps. iPureIntro.
+    rewrite -insert_union_r //. apply insert_mono. done.
   Qed.
 
-  Lemma pstore_get_spec {γ t σ l} v :
-    σ !! l = Some v →
+  Lemma pstore_get_spec {t σ r} v :
+    σ !! r = Some v →
     {{{
-      pstore γ t σ
+      pstore_model t σ
     }}}
-      pstore_get t #l
+      pstore_get t #r
     {{{
       RET v;
-      pstore γ t σ
+      pstore_model t σ
     }}}.
   Proof.
-    iIntros (Hl ϕ) open_inv. iIntros "HΦ".
-    wp_rec. iStep 4. iModIntro.
-
-    iDestruct (big_sepM_lookup_acc _ _ l v with "[$]") as "(?&Hσ0)".
-    { destruct Hinv as [_ Hincl _ _].
-      specialize (Hincl l). rewrite Hl in Hincl. destruct (σ0!!l); naive_solver. }
-
+    iIntros "%Hσ_lookup %Φ (%l & %γ & %σ0 & %ς & -> & %Hσ & #Hmeta & Hauth & Ht) HΦ".
+    wp_apply (raw.pstore_get_spec with "Ht") as "Ht".
+    { eapply lookup_weaken; done. }
     iSteps.
   Qed.
 
-  Lemma pstore_set_spec γ t σ l v :
-    l ∈ dom σ →
+  Lemma pstore_set_spec t σ r v :
+    r ∈ dom σ →
     {{{
-      pstore γ t σ
+      pstore_model t σ
     }}}
-      pstore_set t #l v
+      pstore_set t #r v
     {{{
       RET ();
-      pstore γ t (<[l := v]> σ)
+      pstore_model t (<[r := v]> σ)
     }}}.
   Proof.
-    iIntros (Hl Φ) open_inv. iIntros "HΦ".
-    wp_rec. iStep 8. iModIntro.
-    wp_alloc r' as "Hr'".
-
-    assert (exists w, σ0 !! l = Some w) as (w&Hl0).
-    { apply elem_of_dom. destruct Hinv as [_ Hincl].
-      apply incl_dom_incl in Hincl.
-      set_solver. }
-
-    iDestruct (big_sepM_insert_acc with "Hσ0") as "(?&Hσ0)". done.
-    wp_load. wp_load. wp_store. iStep 4. iModIntro.
-    wp_store. wp_store. iApply "HΦ".
-
-    iSpecialize ("Hσ0" with "[$]").
-
-    iAssert ⌜r ≠ r'⌝%I as %?.
-    { iClear "Ht0". iDestruct (pointsto_ne with "[$][$]") as %?. done. }
-
-    iAssert ⌜r' ∉ vertices g⌝%I as %Hr'.
-    { iIntros (Hr'). destruct Hgraph as [X1 X2].
-      apply X1 in Hr'. destruct Hr' as (?&Hr'). inversion Hr'; subst.
-      { done. }
-      { destruct b. iDestruct (big_sepS_elem_of with "[$]") as "?". done.
-        iDestruct (pointsto_ne r' r' with "[$][$]") as %?. congruence. } }
-
-    iModIntro. iExists t0,r',(<[l:=v]> σ0),({[(r,(l,w),r')]} ∪ g), (<[r':=<[l:=v]> σ0]>M),C.
-    rewrite big_sepS_union.
-    { apply disjoint_singleton_l. intros ?. apply Hr'.
-      apply elem_of_vertices. eauto. }
-    rewrite big_sepS_singleton. iFrame. iPureIntro.
-    split_and!; first done.
-    { destruct Hinv as [X1 X2 X3 X4].
-      constructor.
-      { rewrite dom_insert_L vertices_union vertices_singleton //. set_solver. }
-      { apply gmap_included_insert. done. }
-      { rewrite lookup_insert //. }
-      { intros r1 ds r2 σ1 σ2 Hreach.
-        destruct_decide (decide (r'=r1)).
-        { subst. rewrite lookup_insert. inversion_clear 1.
-          inversion Hreach. subst.
-          2:{ exfalso. subst. rewrite /edge elem_of_union in H0.
-              destruct H0. set_solver. apply Hr'. apply elem_of_vertices. set_solver. }
-          rewrite lookup_insert. inversion 1. done. }
-        rewrite lookup_insert_ne //. intros E1.
-        destruct_decide (decide (r2=r')).
-        { subst. rewrite lookup_insert. inversion 1. subst.
-          apply path_add_inv_r in Hreach; try done.
-          destruct Hreach as [(->&->)|(ds'&->&Hreach)].
-          { congruence. }
-          specialize (X4 _ _ _ _ _ Hreach E1 X3).
-          rewrite fmap_app apply_diffl_snoc insert_insert insert_id //. }
-        { rewrite lookup_insert_ne //. intros. eapply X4; eauto.
-          apply path_cycle_end_inv_aux in Hreach; eauto. } } }
-    { destruct Hcoh as [X1 X2].
-      constructor.
-      { intros r0 ?. destruct_decide (decide (r0=r')).
-        { subst. rewrite lookup_insert. inversion 1. done. }
-        rewrite lookup_insert_ne //. intros HM.
-        apply X1 in HM. rewrite dom_insert_lookup_L //. }
-      { intros ?. set_solver. } }
-    { eauto using rooted_dag_add. }
-    { intros ? r0 ? HC. apply Hsnap in HC. destruct HC as (?&HC&?).
-      destruct_decide (decide (r0=r')).
-      { exfalso. subst. destruct Hinv as [X1 X2 X3].
-        assert (r' ∉ dom M) as F by set_solver. apply F. by eapply elem_of_dom. }
-      rewrite lookup_insert_ne //. eauto. }
+    iIntros "%Hr %Φ (%l & %γ & %σ0 & %ς & -> & %Hσ & #Hmeta & Hauth & Ht) HΦ".
+    iDestruct (raw.pstore_model_valid with "Ht") as %Hς_dom.
+    wp_apply (raw.pstore_set_spec with "Ht") as "Ht".
+    { apply subseteq_dom in Hσ. set_solver. }
+    iApply "HΦ".
+    iExists l, γ, σ0, (<[r := v]> ς). iSteps. iPureIntro.
+    rewrite -insert_union_l. apply insert_mono. done.
   Qed.
 
-  Lemma pstore_capture_spec γ t σ :
+  Lemma pstore_capture_spec t σ :
     {{{
-      pstore γ t σ
+      pstore_model t σ
     }}}
       pstore_capture t
     {{{ s,
       RET s;
-      pstore γ t σ ∗
-      pstore_snapshot γ t s σ
+      pstore_model t σ ∗
+      pstore_snapshot_model s t σ
     }}}.
   Proof.
-    iIntros (Φ) open_inv. iIntros "HΦ".
-    wp_rec. wp_load. do 5 iStep.
-
-    iMod (mono_map_insert' (fresh (dom C)) (r,σ) with "HC") as "(HC&Hsnap)".
-    { apply not_elem_of_dom. apply is_fresh. }
-    iModIntro.
-    iSplitR "Hsnap". 2:iSteps.
-    iExists _,_,_,_,_,_. iFrame.
-    iPureIntro. split_and!; eauto.
-    intros ? r' ? HC.
-    destruct_decide (decide (n=fresh (dom C))).
-    { subst. rewrite lookup_insert in HC. inversion HC. subst.
-      destruct Hinv. eauto. }
-    { rewrite lookup_insert_ne // in HC. eauto. }
-  Qed.
-
-  Definition fsts  (ys:list (loc*(loc*val)*loc)) : list val :=
-    (fun '(x,_,_) => ValLoc x) <$> ys.
-
-  Lemma pstore_collect_spec_aux (r r':loc) t' (xs:list val) (ys:list (loc*(loc*val)*loc)) (g:graph_store) :
-    lst_model' t' xs ->
-    path g r ys r' ->
-    {{{
-      r' ↦ §Root ∗
-      ([∗ set] '(r, (l, v), r') ∈ g, r ↦ ’Diff{ #(l : loc), v, #(r' : loc) })
-    }}}
-      pstore_collect #r t'
-    {{{ t,
-      RET (#r',t);
-      r' ↦ §Root ∗
-      ([∗ set] '(r, (l, v), r') ∈ g, r ↦ ’Diff{ #(l : loc), v, #(r' : loc) }) ∗
-      lst_model t (rev_append (fsts ys) xs)
-    }}}.
-  Proof.
-    iIntros (-> Hpath Φ) "(Hr'&Hg) HΦ".
-    iInduction ys as [|] "IH" forall (r xs r' Hpath); wp_rec.
-    { inversion Hpath. subst. iSteps. }
-    { inversion Hpath. subst.
-      iDestruct (big_sepS_elem_of_acc _ _ (r,b,a2) with "[$]") as "(?&Hg)".
-      { set_solver. } destruct b.
-      wp_load.
-      iSpecialize ("Hg" with "[$]").
-      iSpecialize ("IH" with "[%//][$][$][$]").
-      iSteps.
-    }
-  Qed.
-
-  Lemma pstore_collect_spec (r r':loc) (ys:list (loc*(loc*val)*loc)) (g:graph_store) :
-    path g r ys r' ->
-    {{{
-      r' ↦ §Root ∗
-      ([∗ set] '(r, (l, v), r') ∈ g, r ↦ ’Diff{ #(l : loc), v, #(r' : loc) })
-    }}}
-      pstore_collect #r §Nil
-    {{{ t,
-      RET (#r',t);
-      r' ↦ §Root ∗
-      ([∗ set] '(r, (l, v), r') ∈ g, r ↦ ’Diff{ #(l : loc), v, #(r' : loc) }) ∗
-      lst_model t (rev (fsts ys))
-    }}}.
-  Proof.
-    iIntros (? Φ) "(?&?) HΦ".
-    iDestruct (pstore_collect_spec_aux with "[$]") as "Go"; [done.. |].
-    rewrite -lst_to_val_nil.
-    iApply "Go". rewrite -rev_alt //.
-  Qed.
-
-  Lemma use_path r g (xs:list (loc*(loc*val)*loc)) r0 x r1 r':
-    list_to_set xs ⊆ g ->
-    path g r (xs ++ [(r0, x, r1)]) r' ->
-    (r0, x, r1) ∈ (list_to_set xs : gset(loc*(loc*val)*loc) ) ->
-    exists ds, path g r0 ds r0 /\ ds ≠ nil.
-  Proof.
-    revert r r0 r1 r' x. induction xs; intros r r0 r1 r' x ?.
-    { set_solver. }
-    rewrite -app_comm_cons. inversion 1. subst.
-    rewrite list_to_set_cons.
-    destruct_decide (decide ((r0, x, r1) = (r, b, a2))) as X.
-    { inversion X. subst. intros _. clear IHxs.
-      rewrite app_comm_cons in H0. apply path_snoc_inv in H0.
-      destruct H0 as (?&?&?). subst a2.
-      exists (((r, b, r') :: xs)). done. }
-    { intros ?. apply IHxs in H6. 2,3:set_solver.
-      destruct H6 as (?&?&?). eexists. split; last done.
-      eapply path_weak. done. set_solver. }
-  Qed.
-
-  (* [undo xs ys σ] asserts [mirror xs ys] and that [σ = apply_diffl (proj2 <$> ys ++ xs) σ],
-     ie, ys undo the changes of xs *)
-  Inductive undo :
-    list (loc*(loc*val)*loc) -> list (loc*(loc*val)*loc) -> gmap loc val -> Prop :=
-  | undo_nil :
-    forall σ, undo [] [] σ
-  | undo_cons :
-    forall σ r l v v' r' xs ys,
-      σ !! l = Some v' ->
-      undo xs ys (<[l:=v]> σ) ->
-      undo (xs++[(r,(l,v),r')]) ((r',(l,v'),r)::ys) σ.
-
-  Lemma use_undo xs ys σ :
-    undo xs ys σ ->
-    σ = apply_diffl (proj2 <$> ys ++ xs) σ.
-  Proof.
-    induction 1.
-    { done. }
-    rewrite !assoc_L fmap_app apply_diffl_snoc.
-    rewrite -app_comm_cons fmap_cons apply_diffl_cons.
-    rewrite -IHundo insert_insert insert_id //.
-  Qed.
-
-  Lemma undo_mirror xs ys g :
-    undo xs ys g ->
-    mirror xs ys.
-  Proof.
-    induction 1; eauto using mirror_cons,mirror_nil.
-  Qed.
-
-  Lemma pstore_revert_spec_aux g g1 r t g2 xs r' w σ σ0 :
-    lst_model' t (fsts (rev xs)) ->
-    locs_of_edges_in g2 (dom σ) ->
-    g2 = list_to_set xs ->
-    acyclic g ->
-    g2 ⊆ g ->
-    path g r xs r' ->
-    {{{
-      r' ↦ w ∗
-      ([∗ map] l0↦v0 ∈ σ, l0 ↦ v0) ∗
-      ([∗ set] '(r, (l, v), r') ∈ g1, r ↦ ’Diff{ #(l : loc), v, #(r' : loc) }) ∗
-      ([∗ set] '(r, (l, v), r') ∈ g2, r ↦ ’Diff{ #(l : loc), v, #(r' : loc) })
-    }}}
-      pstore_revert #r' t
-    {{{
-      RET ();
-      ∃ ys,
-      ⌜undo xs ys σ⌝ ∗
-      r ↦ §Root ∗
-      ([∗ set] '(r, (l, v), r') ∈ (g1 ∪ list_to_set ys), r ↦ ’Diff{ #(l : loc), v, #(r' : loc) }) ∗
-      ([∗ map] l0↦v0 ∈ (apply_diffl (proj2 <$> xs) σ), l0 ↦ v0)
-    }}}.
-  Proof.
-    iIntros (-> Hlocs Hg Hacy Hsub Hpath Φ) "(Hr'&Hσ&Hg1&Hg2) HΦ".
-    iInduction xs as [|((r0,(l,v)),r1) ] "IH" using rev_ind forall (σ w r r' g1 g2  Hpath Hg Hlocs Hacy Hsub).
-    { wp_rec. simpl.
-      iStep 4. iModIntro.
-      inversion Hpath. subst. wp_store. iModIntro.
-      iApply "HΦ". iExists nil. rewrite !right_id_L. iFrame.
-      iPureIntro. eauto using undo_nil. }
-    { wp_rec. simpl. rewrite rev_unit. simpl.
-      iStep 4. iModIntro.
-      rewrite Hg list_to_set_app_L list_to_set_cons list_to_set_nil right_id_L.
-      rewrite Hg list_to_set_app_L in Hsub.
-      assert ((r0, (l, v), r1) ∉ (list_to_set xs : gset (loc * diff * loc))).
-      { intros ?. apply use_path in Hpath; last done. destruct Hpath as (?&Hpath&?).
-        apply Hacy in Hpath. congruence. set_solver. }
-      iDestruct (big_sepS_union with "Hg2") as "(Hg2&?)".
-      { set_solver. }
-      rewrite big_sepS_singleton. wp_load. iStep 4. iModIntro.
-
-      rewrite Hg list_to_set_app_L list_to_set_cons list_to_set_nil right_id_L in Hlocs.
-      assert (exists v', σ !! l = Some v') as (v',Hl).
-      { apply elem_of_dom. eapply Hlocs. rewrite /edge.
-
-        rewrite elem_of_union elem_of_singleton. right. reflexivity. }
-
-      apply path_snoc_inv in Hpath. destruct Hpath as (?&->&?).
-      wp_smart_apply assert_spec. rewrite bool_decide_eq_true_2 //.
-      iStep 4. iModIntro.
-
-      iDestruct (big_sepM_insert_acc with "Hσ") as "(?&Hσ)". done.
-      wp_load. wp_store. wp_store. iStep 4. iModIntro.
-
-      iSpecialize ("Hσ" with "[$]").
-      iSpecialize ("IH" with "[%//][%//][%][%//][%][$][$] Hg1 Hg2").
-      { rewrite dom_insert_lookup_L //. intros x1 x2 x3 x4.
-        specialize (Hlocs x1 x2 x3 x4). set_solver. }
-      { set_solver. }
-
-      rewrite fmap_app -apply_diffl_snoc. simpl.
-      iApply "IH". iModIntro.
-      iIntros "[%ys (%Hundo&?&?&?)]". iApply "HΦ".
-      iExists ((r',(l,v'),r0)::ys). iFrame.
-      iSplitR.
-      { iPureIntro. eauto using undo_cons. }
-      rewrite list_to_set_cons.
-      iAssert ⌜(r', (l, v'), r0) ∉ g1 ∪ list_to_set ys⌝%I as "%".
-      { iIntros (?). iDestruct (big_sepS_elem_of with "[$]") as "?". done.
-        iDestruct (pointsto_ne r' r' with "[$][$]") as "%". congruence. }
-      replace (g1 ∪ ({[(r', (l, v'), r0)]} ∪ list_to_set ys)) with ({[(r', (l, v'), r0)]} ∪ ((g1 ∪ list_to_set ys))). 2:set_solver.
-      iApply big_sepS_union. set_solver.
-      iFrame. rewrite big_sepS_singleton //. }
-  Qed.
-
-  Lemma pstore_revert_spec r t g xs r' w σ σ0 :
-    lst_model' t (fsts (rev xs)) ->
-    locs_of_edges_in g (dom σ) ->
-    g = list_to_set xs ->
-    acyclic g ->
-    path g r xs r' ->
-    {{{
-      r' ↦ w ∗
-      ([∗ map] l0↦v0 ∈ σ, l0 ↦ v0) ∗
-      ([∗ set] '(r, (l, v), r') ∈ g, r ↦ ’Diff{ #(l : loc), v, #(r' : loc) })
-    }}}
-      pstore_revert #r' t
-    {{{
-      RET ();
-      ∃ ys,
-      ⌜undo xs ys σ⌝ ∗
-      r ↦ §Root ∗
-      ([∗ set] '(r, (l, v), r') ∈ (list_to_set ys), r ↦ ’Diff{ #(l : loc), v, #(r' : loc) }) ∗
-      ([∗ map] l0↦v0 ∈ (apply_diffl (proj2 <$> xs) σ), l0 ↦ v0)
-    }}}.
-  Proof.
-    iIntros (->???? Φ) "(?&?&?) HΦ".
-    iApply (pstore_revert_spec_aux g ∅ with "[-HΦ]"); try done.
-    { rewrite big_sepS_empty. iFrame. }
-    { iModIntro. iIntros "[% ?]". iApply "HΦ". iExists _. rewrite left_id_L //. }
-  Qed.
-
-  Lemma rev_fsts xs :
-    rev (fsts xs) = fsts (rev xs).
-  Proof.
-    induction xs as [|((?,?),?)]; simpl; eauto.
-    rewrite IHxs /fsts fmap_app //.
-  Qed.
-
-  Lemma pstore_reroot_spec r (xs:list (loc*(loc*val)*loc)) r' g σ :
-    locs_of_edges_in g (dom σ) ->
-    g = list_to_set xs ->
-    acyclic g ->
-    path g r xs r' ->
-    {{{
-      r' ↦ §Root ∗
-      ([∗ map] l0↦v0 ∈ σ, l0 ↦ v0) ∗
-      ([∗ set] '(r, (l, v), r') ∈ g, r ↦ ’Diff{ #(l : loc), v, #(r' : loc) })
-    }}}
-      pstore_reroot #r
-    {{{
-      RET ();
-      ∃ ys,
-      ⌜undo xs ys σ⌝ ∗
-      r ↦ §Root ∗
-      ([∗ set] '(r, (l, v), r') ∈ (list_to_set ys), r ↦ ’Diff{ #(l : loc), v, #(r' : loc) }) ∗
-      ([∗ map] l0↦v0 ∈ (apply_diffl (proj2 <$> xs) σ), l0 ↦ v0)
-    }}}.
-  Proof.
-    iIntros (???? Φ) "(Hr'&Hσ&Hg) HΦ".
-    wp_rec. wp_apply (pstore_collect_spec with "[$]"). done.
-    iIntros (?) "(?&?&%Heq)". rewrite {}Heq.
-    wp_smart_apply (pstore_revert_spec with "[-HΦ]"); try done; first rewrite rev_fsts //.
+    iIntros "%Φ (%l & %γ & %σ0 & %ς & -> & %Hσ & #Hmeta & Hauth & Ht) HΦ".
+    iMod (mono_map_lb_get with "Hauth") as "(Hauth & #Hlb)".
+    wp_apply (raw.pstore_capture_spec with "Ht") as (s) "(Ht & Hs)".
     iSteps.
   Qed.
 
-  Lemma locs_of_edges_weak g1 g2 X :
-    locs_of_edges_in g1 X ->
-    g2 ⊆ g1 ->
-    locs_of_edges_in g2 X.
-  Proof.
-    intros Z ? a b c d ?. eapply (Z a b c d). set_solver.
-  Qed.
-
-  Lemma undo_same_fst_label xs ys r l v r' σ :
-    undo xs ys σ ->
-    (r, (l, v), r') ∈ (list_to_set ys :  gset (loc*(loc*val)*loc)) ->
-    l ∈ (list_to_set (proj2 <$> xs).*1 : gset loc).
-  Proof.
-    revert xs σ. induction ys as [|(?,?)]. set_solver.
-    intros xs σ. inversion 1. subst.
-    simpl. rewrite !fmap_app list_to_set_app_L. simpl in *. subst.
-    destruct_decide (decide ((r, (l, v), r') = (r'0, (l1, v'), l0))) as Heq.
-    { inversion Heq. subst. intros _. set_solver. }
-    intros ?. simpl. apply elem_of_union. left. eapply IHys. done. set_solver.
-  Qed.
-
-  Definition diff_last {A:Type} (ys1 ys2:list A) :=
-    match last ys1, last ys2 with
-    | Some x, Some y =>
-        x ≠ y
-    | _, _ =>
-        True
-    end.
-
-  Lemma path_extract_suffix (g:gset (loc*(loc*val)*loc)) a1 a2 xs1 r xs2 :
-    unaliased g ->
-    path g a1 xs1 r ->
-    path g a2 xs2 r  ->
-    exists ys1 ys2 xs,
-      xs1 = ys1 ++ xs /\
-      xs2 = ys2 ++ xs /\ diff_last ys1 ys2.
-  Proof.
-    intros Hinj.
-    revert r a1 a2 xs2. induction xs1 using rev_ind; intros r a1 a2 xs2.
-    { inversion 1. subst. intros. exists nil,xs2,nil.
-      simpl. rewrite right_id_L. set_solver. }
-    intros Hp1 Hp2. apply path_inv_r in Hp1.
-    destruct Hp1 as [? | (bs'&b'&y&X1&X2&X3)].
-    { destruct xs1; naive_solver. }
-    apply app_inj_tail in X1. destruct X1 as (<-&->).
-
-    apply path_inv_r in Hp2. destruct Hp2 as [(->&->) | (bs'&b&y'&->&?&?)].
-    { exists (xs1 ++ [(y, b', r)]),nil,nil. rewrite right_id. split_and !; try done.
-      unfold diff_last. destruct (last (xs1 ++ [(y, b', r)])); try done. }
-
-    destruct_decide (decide (y'=y)); last first.
-    { eexists _,_,nil. rewrite !right_id_L. split_and!; try done.
-      unfold diff_last. rewrite !last_app. simpl. naive_solver. }
-    subst.
-
-    destruct (IHxs1 _ _ _ _ X2 H) as (ys1&ys2&xs&->&->&Hdiff).
-    destruct (Hinj _ _ _ _ _ X3 H0) as (->&_).
-    eexists _,_,(xs++[(y, b, r)]). rewrite !assoc_L. done.
-  Qed.
-
-  Lemma diff_last_app_middle {A:Type} x (l1' l2' l1 l2:list A) :
-    diff_last (l1' ++ x :: l2') (l1 ++ x :: l2) ->
-    diff_last (x :: l2') (x :: l2).
-  Proof.
-    unfold diff_last. rewrite !last_app !last_cons.
-    destruct (last l2),(last l2'); eauto.
-  Qed.
-
-  Lemma diff_last_irrefl {A:Type} (l:list A) :
-    l ≠ nil ->
-    ¬ (diff_last l l).
-  Proof.
-    destruct (list_case_r l) as [|(?&?&->)]. naive_solver.
-    intros _. unfold diff_last.
-    rewrite !last_app //. simpl. naive_solver.
-  Qed.
-
-  Lemma path_use_diff_last (g:gset (loc*(loc*val)*loc)) a1 a2 ys1 ys2 xs r :
-    acyclic g ->
-    unaliased g ->
-    path g a1 (ys1 ++ xs) r ->
-    path g a2 (ys2 ++ xs) r  ->
-    diff_last ys1 ys2 ->
-    forall x, x ∈ ys2 -> x ∉ (ys1 ++ xs).
-  Proof.
-    intros Hacy Hroot Hp1 Hp2 Hdiff x Hx Hx'.
-    apply elem_of_app in Hx'. destruct Hx' as [Hx'|Hx'].
-    (* contradicts diff_last. *)
-    { apply elem_of_middle in Hx,Hx'.
-      destruct Hx as (l1&l2&->).
-      destruct Hx' as (l1'&l2'&->).
-      rewrite -!assoc_L in Hp1,Hp2.
-      apply path_app_inv in Hp1,Hp2.
-      destruct Hp1 as (x1&_&Hp1).
-      destruct Hp2 as (x2&_&Hp2).
-      rewrite -!app_comm_cons in Hp1,Hp2.
-      assert (x1=proj1 x).
-      { inversion Hp1. subst. done. }
-      assert (x2=proj1 x).
-      { inversion Hp2. subst. done. }
-      subst.
-      eapply acyclic_unaliased_impl_uniq_path in Hp2; eauto.
-      apply Hp2 in Hp1.
-      rewrite !app_comm_cons in Hp1.
-      apply app_inv_tail in Hp1.
-      apply diff_last_app_middle in Hdiff.
-      rewrite Hp1 in Hdiff.
-      eapply diff_last_irrefl; last done. done. }
-    (* There is a loop. *)
-    { apply elem_of_middle in Hx,Hx'.
-      destruct Hx as (l1&l2&->).
-      destruct Hx' as (l1'&l2'&->).
-      rewrite -assoc_L in Hp2.
-      apply path_app_inv in Hp2.
-      destruct Hp2 as (?&_&Hp2).
-      rewrite assoc_L  in Hp2.
-      apply path_app_inv in Hp2.
-      destruct Hp2 as (?&Hp2&Hp2').
-      assert (x0 = proj1 x) as ->.
-      { inversion Hp2. subst. done. }
-      assert (x1 = proj1 x) as ->.
-      { inversion Hp2'. subst. done. }
-      rewrite -app_comm_cons in Hp2.
-      eapply Hacy in Hp2. congruence. }
-  Qed.
-
-  Lemma diff_last_comm {A:Type} (l1 l2:list A) :
-    diff_last l1 l2 <-> diff_last l2 l1.
-  Proof.
-    unfold diff_last.
-    destruct (last l1),(last l2); naive_solver.
-  Qed.
-
-  Lemma path_union_inv (g1: graph loc (loc*val)) g2 a1 xs a2 :
-    path (g1 ∪ g2) a1 xs a2 ->
-    path g1 a1 xs a2 \/ exists a' x xs1 xs2, path g1 a1 xs1 a' /\ x ∈ g2 /\ path (g1 ∪ g2) a' (x::xs2) a2 /\ xs=xs1++x::xs2.
-  Proof.
-    induction 1.
-    left. eauto using path_nil.
-    destruct IHpath as [|(x&?&?&?&?&?&?&->)].
-    { destruct_decide (decide ((a1,b,a2) ∈ g1)).
-      { left. apply path_cons; eauto. }
-      { right. exists a1,(a1,b,a2),nil. eexists. split_and !. apply path_nil. set_solver.
-        apply path_cons. set_solver. eauto. done. } }
-    { right.
-      destruct_decide (decide ((a1,b,a2) ∈ g1)).
-      { eexists _,_,_,_. split_and !;eauto.
-        2:{ rewrite app_comm_cons. reflexivity. }
-        apply path_cons. set_solver. done. }
-      eexists _,_,_,_. split_and !. apply path_nil.
-      3:{ simpl. reflexivity. }
-      set_solver. apply path_cons. set_solver. done. }
-  Qed.
-
-  Lemma path_cannot_escape (x:(loc * diff * loc)) (xs ys:list (loc * diff * loc)) (g1: graph loc (loc*val)) a a' r :
-    (forall x l', ¬ (r,x,l') ∈ (g1 ∪ list_to_set ys)) ->
-    unaliased (g1 ∪ list_to_set ys) ->
-    x ∈ (list_to_set ys : gset _) ->
-    pathlike ys r ->
-    path (g1 ∪ list_to_set ys) a (x :: xs) a' ->
-    path (list_to_set ys) a (x::xs) a'.
-  Proof.
-    intros ? X1 X2 X3. remember (x::xs) as zs.
-    revert a a' x xs Heqzs X1 X2 X3.
-    induction zs; intros a0 a' x xs Heqzs X1 X2 X3. congruence.
-    inversion 1. subst. inversion Heqzs. subst. apply path_cons. eauto.
-    destruct xs as [|((?,?),?)].
-    { inversion H6. subst. eauto using path_nil. }
-    eapply IHzs; eauto. inversion H6. subst.
-    apply elem_of_list_to_set in X2. apply X3 in X2.
-    destruct X2 as [|(?&?&?)]. naive_solver.
-    assert ((l, x, x0) ∈  g1 ∪ list_to_set ys) as Z. set_solver.
-    destruct (X1 _ _ _ _ _ H9 Z). set_solver.
-  Qed.
-
-  Lemma path_in_seg_complete (r a a':loc) (x:(loc * diff * loc)) (xs0 xs1 ys: list (loc * diff * loc)) (g1:graph loc (loc*val)) :
-    (forall x l', ¬ (r,x,l') ∈ (g1 ∪ list_to_set ys)) -> (* root has no succ *)
-    unaliased (g1 ∪ list_to_set ys) ->
-    pathlike ys r ->
-    path (g1 ∪ list_to_set ys) a xs0 a' ->
-    path (list_to_set ys) a' (x :: xs1) a ->
-    exists zs, path (list_to_set ys) a zs a'.
-  Proof.
-    intros Hroot Hinj Hclosed Hp1 Hp2.
-    inversion Hp1.
-    { subst. exists nil. apply path_nil. }
-    subst. eapply path_cannot_escape in Hp1; eauto.
-    apply path_inv_r in Hp2.
-    destruct Hp2 as [|(?&?&?&Heq&Hp2&Hys)].
-    { exfalso. destruct xs1; naive_solver. }
-    apply elem_of_list_to_set in Hys.
-    apply Hclosed in Hys. destruct Hys as [->|(?&?&Hys)].
-    { naive_solver. }
-    assert ((a, x3, x4) ∈  g1 ∪ list_to_set ys) as Z. set_solver.
-    destruct (Hinj _ _ _ _ _ H Z). set_solver.
-  Qed.
-
-  Lemma undo_preserves_rooted_dag (g:graph loc (loc*val)) xs ys rs r :
-    (forall x l', ¬ (rs,x,l') ∈ (list_to_set ys ∪ g ∖ list_to_set xs)) -> (* root has no succ *)
-    unaliased g ->
-    unaliased (list_to_set ys ∪ g ∖ list_to_set xs) ->
-    path g rs xs r ->
-    mirror xs ys ->
-    rooted_dag g r ->
-    rooted_dag (list_to_set ys ∪ g ∖ list_to_set xs) rs.
-  Proof.
-    intros Hnr Hinj Hinj' Hpath Hmirror Hroot. inversion Hroot as [X1 X2].
-    assert (vertices (list_to_set ys ∪ g ∖ list_to_set xs) = vertices g) as Hvg.
-    { apply mirror_vertices in Hmirror.
-      rewrite vertices_union Hmirror -vertices_union -union_difference_L //.
-      eauto using path_all_in. }
-
-    constructor.
-    { intros a. rewrite Hvg => Ha.
-      apply X1 in Ha. destruct Ha as (zs&Ha).
-      edestruct (path_extract_suffix g a rs) as (ys1&ys2&us&?&?&Hlast); eauto. subst.
-
-      apply path_middle in Ha. destruct Ha as (y&Hy1&Hy2).
-      apply path_middle in Hpath. destruct Hpath as (y'&Hy'1&Hy'2).
-      assert (y'=y) as ->.
-      { inversion Hy'2; subst; inversion Hy2; naive_solver. }
-      eapply use_mirror_subset in Hmirror. 3:apply Hy'1. 2:set_solver.
-      destruct Hmirror as (zs&Hzs&_).
-      exists (ys1++zs). eapply path_app.
-      2:{ eapply path_weak. done. set_solver. }
-      clear X2. induction Hy1.
-      { apply path_nil. }
-      apply path_cons.
-      { rewrite elem_of_union elem_of_difference. right. split. set_solver.
-        apply not_elem_of_list_to_set.
-        eapply path_use_diff_last. 1,2: eauto using ti2.
-        3:{ apply diff_last_comm. done. }
-        { eapply path_app; eauto. }
-        { rewrite -app_comm_cons. eapply path_cons. done.
-          eapply path_app; eauto. }
-        { set_solver. } }
-      { apply IHHy1; eauto.  unfold diff_last in *. rewrite last_cons in Hlast.
-        destruct (last bs), (last ys2); try done. } }
-    { intros a zs Hzs. rewrite comm_L in Hzs.
-      apply path_union_inv in Hzs. destruct Hzs as [Hsz|Hsz].
-      (* The cycle is only in g, easy. *)
-      { eapply X2. eapply path_weak. done. set_solver. }
-      (* There is at least a vertex in ys.
-         We are going to construct a cycle in ys, implying a cycle in xs. *)
-      exfalso. destruct Hsz as (a'&x&l1&l2&E1&Hx&E2&->).
-
-      apply path_cannot_escape with (r:=rs) in E2; last first.
-      { eapply path_pathlike. eapply use_mirror; eauto. }
-      { done. }
-      { rewrite comm_L //. }
-      { set_solver. }
-
-      eapply path_weak in E1.
-      eapply path_in_seg_complete with (r:=rs) in E1; last first. done.
-      { eapply path_pathlike. eapply use_mirror; eauto. }
-      { rewrite comm_L //. }
-      { set_solver. }
-      2:{ set_solver. }
-      destruct E1 as (?&E1).
-
-      assert (path (list_to_set ys) a (x0 ++ x::l2) a ) as Hcycle.
-      { eapply path_app. done. done. }
-
-      eapply use_mirror_subset with (ys:=xs) in Hcycle.
-      3:{ by apply mirror_symm. }
-      2:{ apply path_all_in in Hcycle. set_solver. }
-      destruct Hcycle as (?&Hcycle&F).
-      eapply path_weak in Hcycle. 2:eapply path_all_in; done.
-      eapply ti2 in Hcycle; eauto. subst. destruct x0; simpl in *; lia. }
-  Qed.
-
-  Lemma undo_app_inv xs ys1 ys2 σ :
-    undo xs (ys1 ++ ys2) σ ->
-    exists xs1 xs2, xs = xs2 ++ xs1 /\ undo xs2 ys2 (apply_diffl (proj2 <$> xs1) σ) /\ undo xs1 ys1 σ.
-  Proof.
-    revert xs ys2 σ. induction ys1; intros xs ys2 σ Hundo.
-    { exists nil,xs. rewrite right_id_L. split; eauto using undo_nil. }
-    rewrite -app_comm_cons in Hundo. inversion Hundo. subst.
-    apply IHys1 in H4. destruct H4 as (xs1&xs2&->&?&?).
-    eexists _,xs2. split_and !.
-    { rewrite -assoc_L //. }
-    { rewrite fmap_app apply_diffl_app. done. }
-    { apply undo_cons. done. done. }
-  Qed.
-
-  Lemma construct_middlepoint (g:graph loc (loc*val)) a1 xs ys a2 a2' :
-    unaliased g ->
-    (forall x l', ¬ (a2,x,l') ∈ g) -> (* root has no succ *)
-    path g a1 xs a2 ->
-    path g a1 ys a2' ->
-    exists zs, xs = ys ++ zs.
-  Proof.
-    intros Hinj Hroot Hpath. revert ys. induction Hpath; intros ys.
-    { intros Hpath. inversion Hpath. eauto. subst. set_solver. }
-    { intros X. inversion X; subst.
-      { exists ((a2', b, a2) :: bs ). done. }
-      destruct (Hinj _ _ _ _ _ H H0). subst.
-      apply IHHpath in H1. destruct H1 as (?&?).
-      eexists. rewrite -app_comm_cons H1 //.
-      intros ??. apply Hroot. }
-  Qed.
-
-
-  Lemma undo_preserves_model g (M:map_model) (xs ys:list (loc* (loc*val)*loc)) rs σ0 r:
-    dom M = vertices g ∪ {[r]} ->
-    correct_path_diff M g ->
-    (forall x l', ¬ (rs,x,l') ∈ (list_to_set ys ∪ g ∖ list_to_set xs)) -> (* root has no succ *)
-    unaliased (g ∖ list_to_set xs ∪ list_to_set ys) ->
-    path g rs xs r ->
-    undo xs ys σ0 ->
-    M !! r = Some σ0 ->
-    correct_path_diff M (list_to_set ys ∪ g ∖ list_to_set xs).
-  Proof.
-    intros Hdom Hinv Hroot Hinj' Hrs Hundo E0.
-    intros r1 zs r2 σ1 σ2 Hpath E1 E2. rewrite comm_L in Hpath.
-    apply path_union_inv in Hpath. destruct Hpath as [Hpath|Hpath].
-
-    (* If the path is entirely in g, easy. *)
-    { eapply Hinv; eauto. eapply path_weak. done. set_solver. }
-
-    assert (mirror xs ys) as Hmirror by eauto using undo_mirror.
-
-    destruct Hpath as (a'&x&l1&l2&X1&Hx&X2&Hzs).
-    eapply path_cannot_escape with (r:=rs) in X2; eauto; last first.
-    { eapply path_pathlike. eapply use_mirror; eauto. }
-    { set_solver. }
-
-    (* otherwise the path includes a part in g, and a part in ys. *)
-
-    assert (vertices (list_to_set ys ∪ g ∖ list_to_set xs) = vertices g) as Hvg.
-    { apply mirror_vertices in Hmirror.
-      rewrite vertices_union Hmirror -vertices_union -union_difference_L //.
-      eauto using path_all_in. }
-
-    assert (a' ∈ dom M) as Ha'.
-    { rewrite Hdom -Hvg elem_of_union. left. apply elem_of_vertices.
-      inversion X2. set_solver. }
-    apply elem_of_dom in Ha'. destruct Ha' as (σ',Ea').
-    assert (σ1 = (apply_diffl (proj2 <$> l1) σ')).
-    { eapply path_weak in X1.
-      eapply (Hinv _ _ _ _ _ X1 E1 Ea'). set_solver. }
-
-    (* The part in g is preserved. *)
-
-    etrans. done. rewrite Hzs. rewrite fmap_app apply_diffl_app.
-    f_equal. clear dependent σ1 l1.
-
-    (* XXX facto a lemma. *)
-    assert (exists u1 u2, ys = u1 ++ (x::l2) ++ u2) as (u1&u2&Hys).
-    { eapply use_mirror in Hrs. 2:done.
-      apply elem_of_list_to_set, elem_of_middle in Hx.
-      destruct Hx as (p1&p2&->).
-      apply path_app_inv in Hrs. destruct Hrs as (?&Hp1&Hp2).
-      inversion Hp2; inversion X2. subst. inversion H5. subst.
-      eapply construct_middlepoint in H10. 4:apply H4.
-      2:{ intros z1 z2 z3 z4 z5 ??. eapply (Hinj' z1 z2 z3 z4 z5); try done.
-          all:apply elem_of_union; right. all:set_solver. }
-      2:{ intros x l' X. eapply (Hroot x l').
-          apply elem_of_union. left. set_solver. }
-      destruct H10.
-      eexists _,_. f_equal. rewrite -app_comm_cons. f_equal. done. }
-
-    rewrite Hys assoc_L in Hundo. apply undo_app_inv in Hundo.
-    destruct Hundo as (xs1&xs2&->&Hundo1&Hundo2).
-    apply undo_app_inv in Hundo2.
-    destruct Hundo2 as (xs4&xs3&->&Hundo2&Hundo3).
-
-    eapply use_mirror in Hmirror. 2:done.
-    rewrite {2}Hys in Hmirror.
-    apply path_app_inv in Hmirror. destruct Hmirror as (n1&T1&T2).
-    apply path_app_inv in T2. destruct T2 as (n2&T2&T3).
-    edestruct (same_path (list_to_set ys) (x::l2) n1 n2 a') as (?&?); try done.
-    subst n1 n2.
-
-    assert (path g a' xs4 r) as R1.
-    { eapply path_weak.
-      eapply use_mirror. eapply mirror_symm. eauto using undo_mirror. done.
-      apply path_all_in in Hrs. set_solver. }
-    apply (Hinv _ _ _ σ' σ0) in R1; try done.
-
-    assert (path g r2 xs3 a') as R2.
-    { eapply path_weak.
-      eapply use_mirror. eapply mirror_symm. eauto using undo_mirror. done.
-      apply path_all_in in Hrs. set_solver. }
-    eapply (Hinv _ _ _ σ2 σ') in R2; try done.
-    rewrite R2. rewrite -apply_diffl_app -fmap_app.
-    eapply use_undo. rewrite R1. done.
-  Qed.
-
-  Lemma pstore_restore_spec γ t σ s σ' :
+  Lemma pstore_restore_spec t σ s σ' :
     {{{
-      pstore γ t σ ∗
-      pstore_snapshot γ t s σ'
+      pstore_model t σ ∗
+      pstore_snapshot_model s t σ'
     }}}
       pstore_restore t s
     {{{
       RET ();
-      pstore γ t σ'
+      pstore_model t σ'
     }}}.
   Proof.
-    iIntros (Φ) "(HI&Hsnap) HΦ".
-    iDestruct "HI" as open_inv.
-    iDestruct "Hsnap" as "(%rs&%&->&Hsnap)".
-    wp_rec. iStep 20.
-
-    iDestruct (extract_unaliased with "Hg") as "%".
-
-    iDestruct (mono_map_elem_valid with "[$][$]") as "%Hrs".
-    apply Hsnap in Hrs. destruct Hrs as (σ1&HMrs&?).
-
-    destruct_decide (decide (rs=r)).
-    { subst.
-      subst.
-      wp_load. iStep 4. iModIntro.
-      iExists _,_,_,_,_,_. iFrame. iPureIntro. split_and!; eauto.
-      { destruct Hinv as [X1 X2 X3 X4]. constructor; eauto. naive_solver. } }
-
-    assert (rs ∈ vertices g) as Hrs.
-    { destruct Hinv. apply elem_of_dom_2 in HMrs. set_solver. }
-
-    eapply ti1 in Hrs; eauto. destruct Hrs as (ds,Hrs).
-    inversion Hrs. congruence. subst. rename a2 into r'. destruct b.
-    iDestruct (big_sepS_elem_of_acc with "[$]") as "(?&Hg)". done. simpl.
-    wp_load. iStep 2. iModIntro.
-    iSpecialize ("Hg" with "[$]").
-
-    remember ((rs, (l, v), r') :: bs) as xs.
-    assert (list_to_set xs ⊆ g).
-    { eauto using path_all_in. }
-
-    rewrite (union_difference_L (list_to_set xs) g) //.
-
-    iDestruct (big_sepS_union with "Hg") as "(Hxs&Hg)". set_solver.
-    wp_apply (pstore_reroot_spec with "[Hr Hxs Hσ0]").
-    4:{ eapply path_restrict. done. }
-    2:done.
-    { destruct Hcoh as [_ X]. eapply locs_of_edges_weak; eauto. }
-    { eapply acyclic_weak; eauto using ti2. }
-    { iFrame. }
-
-    iIntros "[%ys (%Hundo&?&?&?)]".
-    assert (mirror xs ys) as Hmirror by eauto using undo_mirror.
-    iStep 8. do 2 iModIntro.
+    iIntros "%Φ ((%l & %γ & %σ0 & %ς & -> & %Hσ & #Hmeta & Hauth & Ht) & (%_l & %_γ & %σ0' & %ς' & %Heq & %Hσ' & _Hmeta & #Hlb & Hs)) HΦ". injection Heq as <-.
+    iDestruct (meta_agree with "Hmeta _Hmeta") as %<-. iClear "_Hmeta".
+    wp_apply (raw.pstore_restore_spec with "[$Ht $Hs]") as "Ht".
+    iDestruct (mono_map_lb_valid with "Hauth Hlb") as %Hσ0'.
     iApply "HΦ".
-    iDestruct (big_sepS_union_2 with "[$][$]") as "Hs".
-
-    remember ((rs, (l, v), r') :: bs) as xs.
-
-    iDestruct (extract_unaliased with "Hs") as "%".
-
-    assert (({[(rs, (l, v), r')]} ∪ list_to_set bs) = (list_to_set xs : gset _)) as Hbs.
-    { subst xs. reflexivity. }
-    rewrite Hbs. rewrite Hbs in H5.
-
-    iAssert ⌜forall x y, (rs,x,y) ∉ (list_to_set ys ∪ g ∖ list_to_set xs)⌝%I as "%".
-    { iIntros (???). destruct a. iDestruct (big_sepS_elem_of with "Hs") as "?". done.
-      iDestruct (pointsto_ne rs rs with "[$][$]") as "%". congruence. }
-
-    iExists _,_,_,_,M,_. iFrame.
-
-    assert (vertices (list_to_set ys ∪ g ∖ list_to_set xs) = vertices g) as Hvg.
-    { apply mirror_vertices in Hmirror.
-      rewrite vertices_union Hmirror -vertices_union -union_difference_L //. }
-
-    assert (σ1 = (apply_diffl (proj2 <$> xs) σ0)).
-    { destruct Hinv as [X1 X2 X3 X4]. eauto. }
-
-    assert (rooted_dag (list_to_set ys ∪ g ∖ list_to_set xs) rs) as Hroot.
-    { eapply undo_preserves_rooted_dag; eauto. }
-
-    iPureIntro. split_and !; try done.
-    { destruct Hinv as [X1 X2 X3 X4]. constructor.
-      { rewrite X1 Hvg.
-        apply elem_of_dom_2 in X3,HMrs.
-        apply path_ends_vertices in Hrs.
-        set_solver. }
-      { subst xs. set_solver. }
-      { set_solver. }
-      { intros. eapply undo_preserves_model; eauto. rewrite comm_L //. }
-    } {
-      rewrite /apply_diffl.
-      replace (<[l:=v]> (foldr (λ '(l0, v0) σ2, <[l0:=v0]> σ2) σ0 (list_fmap (loc * diff * loc)%type diff proj2 bs))) with (apply_diffl (proj2 <$> xs) σ0).
-      2:{ subst xs. reflexivity. }
-
-      destruct Hcoh as [X1 X2]. constructor.
-      { intros ???. rewrite dom_apply_diffl. apply X1 in H8.
-        eapply use_locs_of_edges_in in Hrs. 2:done.
-        set_solver.
-      } {
-        rewrite dom_apply_diffl. intros ???? Hedge.
-        rewrite /edge elem_of_union in Hedge. rewrite elem_of_union.
-        destruct Hedge as [Hedge|Hedge].
-        { right. eauto using undo_same_fst_label. }
-        { left. eapply (X2 r0). eapply elem_of_subseteq. 2:done. set_solver. }
-      }
-    }
+    iExists l, γ, σ0, ς'. iSteps. iPureIntro.
+    trans (ς' ∪ σ0'); first done. apply map_union_mono_l. done.
   Qed.
 End pstore_G.
 
-#[global] Opaque pstore_create.
-#[global] Opaque pstore_ref.
-#[global] Opaque pstore_get.
-#[global] Opaque pstore_set.
-#[global] Opaque pstore_capture.
-#[global] Opaque pstore_restore.
-
-#[global] Opaque pstore.
-#[global] Opaque pstore_snapshot.
+#[global] Opaque pstore_model.
+#[global] Opaque pstore_snapshot_model.
